<?xml version="1.0" encoding="utf-8"?>
<rdf:RDF xmlns:dc="http://purl.org/dc/terms/" xmlns:foaf="http://xmlns.com/foaf/0.1/" xmlns:hxl="http://carsten.io/hxl/ns-2012-01-23#" xmlns:owl="http://www.w3.org/2002/07/owl#" xmlns:rdf="http://www.w3.org/1999/02/22-rdf-syntax-ns#" xmlns:rdfs="http://www.w3.org/2000/01/rdf-schema#" xmlns:skos="http://www.w3.org/2004/02/skos/core#" xmlns:xsd="http://www.w3.org/2001/XMLSchema#">
  <rdf:Description rdf:about="http://carsten.io/hxl/ns-2012-01-23">
    <rdf:type rdf:resource="http://www.w3.org/2002/07/owl#Ontology"/>
  </rdf:Description>
  <rdf:Description rdf:about="http://carsten.io/hxl/ns-2012-01-23">
    <dc:date>2012-01-23</dc:date>
  </rdf:Description>
  <rdf:Description rdf:about="http://carsten.io/hxl/ns-2012-01-23">
    <dc:creator rdf:resource="http://carsten.io/hxl/ns-2012-01-23#carsten"/>
  </rdf:Description>
  <rdf:Description rdf:about="http://carsten.io/hxl/ns-2012-01-23">
    <dc:creator rdf:resource="http://carsten.io/hxl/ns-2012-01-23#cj"/>
  </rdf:Description>
  <rdf:Description rdf:about="http://carsten.io/hxl/ns-2012-01-23">
    <dc:title xml:lang="en">Humanitarian eXchange Language (HXL) domain vocabulary</dc:title>
  </rdf:Description>
  <rdf:Description rdf:about="http://carsten.io/hxl/ns-2012-01-23">
    <dc:abstract xml:lang="en">&lt;p&gt;Draft specification of the Humanitarian eXchange Language (HXL) standard. This vocabulary specification is currently &lt;b&gt;under development&lt;/b&gt; and may change at any time without notice.&lt;/p&gt; &lt;p&gt;The porpuse of HXL is to facilitate data exchange within the humanitarian domain. It provides a core domain model that has been created bottom-up by inspecting a broad range of systems in use with different humanitarian organizations. As needs vary widely across organizations in this domain, this vocabulary does &lt;em&gt;not&lt;/em&gt; intend to be complete; in fact, it is the smallest common denominator. Any organizations that wish to publish &lt;em&gt;full&lt;/em&gt; exports of their data can do so by extending this domain model with application- or organization-specific models that reflect their internal data models (which may already be formalized in an XML schema or database schema). </dc:abstract>
  </rdf:Description>
  <rdf:Description rdf:about="http://carsten.io/hxl/ns-2012-01-23">
    <dc:license xml:lang="en">We still need to decide under which license this vocabulary should be published.</dc:license>
  </rdf:Description>
  <rdf:Description rdf:about="http://carsten.io/hxl/ns-2012-01-23">
    <dc:versionOf rdf:resource="http://carsten.io/hxl/ns"/>
  </rdf:Description>
  <rdf:Description rdf:about="http://carsten.io/hxl/ns-2012-01-23">
    <rdfs:seeAlso xml:lang="en">For further information about the HXL project, see &lt;a href='https://sites.google.com/site/hxlproject/'&gt;https://sites.google.com/site/hxlproject/&lt;/a&gt;.</rdfs:seeAlso>
  </rdf:Description>
  <rdf:Description rdf:about="http://carsten.io/hxl/ns-2012-01-23">
    <dc:replaces rdf:resource="http://carsten.io/hxl/ns-2012-01-21"/>
  </rdf:Description>
  <rdf:Description rdf:about="http://carsten.io/hxl/ns-2012-01-23">
    <skos:changeNote>&lt;ol&gt;&lt;li&gt;Classes &lt;a href='#NeedTarget'&gt;NeedTarget&lt;/a&gt; and &lt;a href='#NeedAchieved'&gt;NeedAchieved&lt;/a&gt; have been introduced.&lt;/li&gt;&lt;li&gt;The &lt;a href='#measures'&gt;measures&lt;/a&gt; property does not have &lt;a href='#Need'&gt;Need&lt;/a&gt; as range anymore: a need is &lt;a href='#basedOn'&gt;based on&lt;/a&gt; an indicator, which measures the progress in addressing this need. &lt;/li&gt;&lt;li&gt;&lt;a href='#Project'&gt;Project&lt;/a&gt; is now a subclass of &lt;a href='#Activity'&gt;Activity&lt;/a&gt;. This is more consistent, as Activity is the (more ambiguous) superclass now that is used in all property definitions (which still apply to Project). &lt;li&gt;Classes &lt;a href='#Need'&gt;Need&lt;/a&gt; , Gap, and Lack have been merged, since we only address actual needs, i.e., in the sense of a lack of food. These needs &lt;a href='requires'&gt;require&lt;/a&gt; some kind of &lt;a href='#'&lt;li&gt;Property &lt;em&gt;locatedAt&lt;/em&gt; removed for redundancy (see &lt;a href='#location'&gt;location&lt;/a&gt;).&lt;li&gt;Class &lt;a href='#Donor'&gt;Donor&lt;/a&gt; introduced, along with property &lt;a href='#contributesTo'&gt;contributesTo&lt;/a&gt;.&lt;li&gt;Class &lt;em&gt;BasicHumanNeed&lt;/em&gt; has been removed – design decision to stick to measurable or reportable classes for HXL.&lt;li&gt;Switched from &lt;em&gt;rdfs:label&lt;/em&gt; to &lt;em&gt;skos:prefLabel&lt;/em&gt; to be able to add alternative labels to the classes (via &lt;em&gt;skos:altLabel&lt;/em&gt;). &lt;/li&gt;&lt;li&gt;Merged classes Budget and Funding.&lt;/li&gt;&lt;li&gt;Added alternative labels to several classes.&lt;/li&gt;&lt;li&gt;Fixed a number of typos.&lt;/li&gt;&lt;/ol&gt;</skos:changeNote>
  </rdf:Description>
  <rdf:Description rdf:about="http://carsten.io/hxl/ns-2012-01-23#carsten">
    <foaf:name>Carsten Keßler</foaf:name>
  </rdf:Description>
  <rdf:Description rdf:about="http://carsten.io/hxl/ns-2012-01-23#carsten">
    <foaf:mbox>me@carsten.io</foaf:mbox>
  </rdf:Description>
  <rdf:Description rdf:about="http://carsten.io/hxl/ns-2012-01-23#carsten">
    <foaf:homepage rdf:resource="http://carsten.io"/>
  </rdf:Description>
  <rdf:Description rdf:about="http://carsten.io/hxl/ns-2012-01-23#cj">
    <foaf:name>CJ Hendrix</foaf:name>
  </rdf:Description>
  <rdf:Description rdf:about="http://carsten.io/hxl/ns-2012-01-23#cj">
    <foaf:mbox>hendrix@un.org</foaf:mbox>
  </rdf:Description>
  <rdf:Description rdf:about="http://carsten.io/hxl/ns-2012-01-23#Situation">
    <rdf:type rdf:resource="http://www.w3.org/2000/01/rdf-schema#Class"/>
  </rdf:Description>
  <rdf:Description rdf:about="http://carsten.io/hxl/ns-2012-01-23#Situation">
    <skos:prefLabel xml:lang="en">Situation</skos:prefLabel>
  </rdf:Description>
  <rdf:Description rdf:about="http://carsten.io/hxl/ns-2012-01-23#Situation">
    <rdfs:comment xml:lang="en">Generic situation.</rdfs:comment>
  </rdf:Description>
  <rdf:Description rdf:about="http://carsten.io/hxl/ns-2012-01-23#Activity">
    <rdf:type rdf:resource="http://www.w3.org/2000/01/rdf-schema#Class"/>
  </rdf:Description>
  <rdf:Description rdf:about="http://carsten.io/hxl/ns-2012-01-23#Activity">
    <skos:prefLabel xml:lang="en">Humanitarian Activity</skos:prefLabel>
  </rdf:Description>
  <rdf:Description rdf:about="http://carsten.io/hxl/ns-2012-01-23#Activity">
    <rdfs:comment xml:lang="en">An Activity generally addresses some kind of need given in a Humanitarian Situation. &lt;br /&gt;&lt;small&gt;Term origin: IATI, CAP OPS, Pakistan SRF, Sahana Project, Sigmah DB&lt;/small&gt;</rdfs:comment>
  </rdf:Description>
  <rdf:Description rdf:about="http://carsten.io/hxl/ns-2012-01-23#AffectedPopulation">
    <rdf:type rdf:resource="http://www.w3.org/2000/01/rdf-schema#Class"/>
  </rdf:Description>
  <rdf:Description rdf:about="http://carsten.io/hxl/ns-2012-01-23#AffectedPopulation">
    <skos:prefLabel xml:lang="en">Affected Population</skos:prefLabel>
  </rdf:Description>
  <rdf:Description rdf:about="http://carsten.io/hxl/ns-2012-01-23#AffectedPopulation">
    <rdfs:subClassOf rdf:resource="http://carsten.io/hxl/ns-2012-01-23#Population"/>
  </rdf:Description>
  <rdf:Description rdf:about="http://carsten.io/hxl/ns-2012-01-23#AffectedPopulation">
    <rdfs:comment xml:lang="en">The population affected by an emergency.&lt;br /&gt;&lt;small&gt;Term origin: Humanitarian Profile (&lt;em&gt;Affected&lt;/em&gt;);&lt;/small&gt;</rdfs:comment>
  </rdf:Description>
  <rdf:Description rdf:about="http://carsten.io/hxl/ns-2012-01-23#Cluster">
    <rdf:type rdf:resource="http://www.w3.org/2000/01/rdf-schema#Class"/>
  </rdf:Description>
  <rdf:Description rdf:about="http://carsten.io/hxl/ns-2012-01-23#Cluster">
    <skos:prefLabel xml:lang="en">Cluster</skos:prefLabel>
  </rdf:Description>
  <rdf:Description rdf:about="http://carsten.io/hxl/ns-2012-01-23#Cluster">
    <rdfs:comment xml:lang="en">An organizational unit responsible for one or more sectors during an emergency.&lt;br /&gt;&lt;small&gt;Term origin: CAP OPS, CCDI.&lt;/small&gt;</rdfs:comment>
  </rdf:Description>
  <rdf:Description rdf:about="http://carsten.io/hxl/ns-2012-01-23#Agency">
    <rdf:type rdf:resource="http://www.w3.org/2000/01/rdf-schema#Class"/>
  </rdf:Description>
  <rdf:Description rdf:about="http://carsten.io/hxl/ns-2012-01-23#Agency">
    <rdfs:subClassOf rdf:resource="http://carsten.io/hxl/ns-2012-01-23#Organization"/>
  </rdf:Description>
  <rdf:Description rdf:about="http://carsten.io/hxl/ns-2012-01-23#Agency">
    <skos:prefLabel xml:lang="en">Agency</skos:prefLabel>
  </rdf:Description>
  <rdf:Description rdf:about="http://carsten.io/hxl/ns-2012-01-23#Agency">
    <rdfs:comment xml:lang="en">An Agency is an official body of the United Nations. &lt;br /&gt;&lt;small&gt;Term origin: CCDI, CERF, Shelter Cluster&lt;/small&gt;</rdfs:comment>
  </rdf:Description>
  <rdf:Description rdf:about="http://carsten.io/hxl/ns-2012-01-23#ImplementingPartner">
    <rdf:type rdf:resource="http://www.w3.org/2000/01/rdf-schema#Class"/>
  </rdf:Description>
  <rdf:Description rdf:about="http://carsten.io/hxl/ns-2012-01-23#ImplementingPartner">
    <skos:prefLabel xml:lang="en">Implementing Partner</skos:prefLabel>
  </rdf:Description>
  <rdf:Description rdf:about="http://carsten.io/hxl/ns-2012-01-23#ImplementingPartner">
    <skos:altLabel xml:lang="en">IP</skos:altLabel>
  </rdf:Description>
  <rdf:Description rdf:about="http://carsten.io/hxl/ns-2012-01-23#ImplementingPartner">
    <rdfs:comment xml:lang="en">An external partner implenting (parts) of a project for an agency. &lt;br /&gt;&lt;small&gt;Term origin: CAP OPS, Pakistan SRF, HPM Ethiopia (&lt;em&gt;Partner&lt;/em&gt;), Sigmah DB (&lt;em&gt;Partner&lt;/em&gt;).&lt;/small&gt;</rdfs:comment>
  </rdf:Description>
  <rdf:Description rdf:about="http://carsten.io/hxl/ns-2012-01-23#ImplementingPartner">
    <rdfs:subClassOf rdf:resource="http://carsten.io/hxl/ns-2012-01-23#Organization"/>
  </rdf:Description>
  <rdf:Description rdf:about="http://carsten.io/hxl/ns-2012-01-23#Camp">
    <rdf:type rdf:resource="http://www.w3.org/2000/01/rdf-schema#Class"/>
  </rdf:Description>
  <rdf:Description rdf:about="http://carsten.io/hxl/ns-2012-01-23#Camp">
    <rdfs:subClassOf rdf:resource="http://carsten.io/hxl/ns-2012-01-23#Site"/>
  </rdf:Description>
  <rdf:Description rdf:about="http://carsten.io/hxl/ns-2012-01-23#Camp">
    <rdfs:subClassOf rdf:resource="http://carsten.io/hxl/ns-2012-01-23#Shelter"/>
  </rdf:Description>
  <rdf:Description rdf:about="http://carsten.io/hxl/ns-2012-01-23#Camp">
    <skos:prefLabel xml:lang="en">Camp</skos:prefLabel>
  </rdf:Description>
  <rdf:Description rdf:about="http://carsten.io/hxl/ns-2012-01-23#Camp">
    <rdfs:comment xml:lang="en">A site with temporary shelter for an affected population, such as refugees. &lt;br /&gt;&lt;small&gt;Term origin: UNHCR Camp DB, Pakistan SRF, Humanitarian Profile.&lt;/small&gt;</rdfs:comment>
  </rdf:Description>
  <rdf:Description rdf:about="http://carsten.io/hxl/ns-2012-01-23#Population">
    <rdf:type rdf:resource="http://www.w3.org/2000/01/rdf-schema#Class"/>
  </rdf:Description>
  <rdf:Description rdf:about="http://carsten.io/hxl/ns-2012-01-23#Population">
    <skos:prefLabel xml:lang="en">Population</skos:prefLabel>
  </rdf:Description>
  <rdf:Description rdf:about="http://carsten.io/hxl/ns-2012-01-23#Population">
    <rdfs:subClassOf rdf:resource="http://xmlns.com/foaf/0.1/Group"/>
  </rdf:Description>
  <rdf:Description rdf:about="http://carsten.io/hxl/ns-2012-01-23#Population">
    <rdfs:comment xml:lang="en">Generic class for any kind of population (e.g. total, affected, etc.); use the subclasses for the data annotation.</rdfs:comment>
  </rdf:Description>
  <rdf:Description rdf:about="http://carsten.io/hxl/ns-2012-01-23#TotalPopulation">
    <rdf:type rdf:resource="http://www.w3.org/2000/01/rdf-schema#Class"/>
  </rdf:Description>
  <rdf:Description rdf:about="http://carsten.io/hxl/ns-2012-01-23#TotalPopulation">
    <skos:prefLabel xml:lang="en">Total Population</skos:prefLabel>
  </rdf:Description>
  <rdf:Description rdf:about="http://carsten.io/hxl/ns-2012-01-23#TotalPopulation">
    <rdfs:subClassOf rdf:resource="http://carsten.io/hxl/ns-2012-01-23#Population"/>
  </rdf:Description>
  <rdf:Description rdf:about="http://carsten.io/hxl/ns-2012-01-23#TotalPopulation">
    <rdfs:comment xml:lang="en">Total population for a given administrative unit or geographic area. Instances can be created to make statements about this population.</rdfs:comment>
  </rdf:Description>
  <rdf:Description rdf:about="http://carsten.io/hxl/ns-2012-01-23#AgeGroup">
    <rdf:type rdf:resource="http://www.w3.org/2000/01/rdf-schema#Class"/>
  </rdf:Description>
  <rdf:Description rdf:about="http://carsten.io/hxl/ns-2012-01-23#AgeGroup">
    <skos:prefLabel xml:lang="en">Age Group</skos:prefLabel>
  </rdf:Description>
  <rdf:Description rdf:about="http://carsten.io/hxl/ns-2012-01-23#AgeGroup">
    <rdfs:subClassOf rdf:resource="http://carsten.io/hxl/ns-2012-01-23#Population"/>
  </rdf:Description>
  <rdf:Description rdf:about="http://carsten.io/hxl/ns-2012-01-23#AgeGroup">
    <rdfs:comment>Generic class for age groups; instances should be created for actual age groups (e.g. children under 5). </rdfs:comment>
  </rdf:Description>
  <rdf:Description rdf:about="http://carsten.io/hxl/ns-2012-01-23#Appeal">
    <rdf:type rdf:resource="http://www.w3.org/2000/01/rdf-schema#Class"/>
  </rdf:Description>
  <rdf:Description rdf:about="http://carsten.io/hxl/ns-2012-01-23#Appeal">
    <skos:prefLabel xml:lang="en">Appeal</skos:prefLabel>
  </rdf:Description>
  <rdf:Description rdf:about="http://carsten.io/hxl/ns-2012-01-23#Appeal">
    <rdfs:comment>An appeal is a request for aid in the form of money or goods from Donors. &lt;br /&gt;&lt;small&gt;Term origin: CAP OPS, Pakistan SRF.&lt;/small&gt;</rdfs:comment>
  </rdf:Description>
  <rdf:Description rdf:about="http://carsten.io/hxl/ns-2012-01-23#Budget">
    <rdf:type rdf:resource="http://www.w3.org/2000/01/rdf-schema#Class"/>
  </rdf:Description>
  <rdf:Description rdf:about="http://carsten.io/hxl/ns-2012-01-23#Budget">
    <skos:prefLabel xml:lang="en">Budget</skos:prefLabel>
  </rdf:Description>
  <rdf:Description rdf:about="http://carsten.io/hxl/ns-2012-01-23#Budget">
    <skos:altLabel xml:lang="en">Funding</skos:altLabel>
  </rdf:Description>
  <rdf:Description rdf:about="http://carsten.io/hxl/ns-2012-01-23#Budget">
    <rdfs:comment>The money allocated to a Project.&lt;br /&gt;&lt;small&gt;Term origin: IATI, Sigmah DB, Sahana Project (&lt;em&gt;Funding&lt;/em&gt;), EDXL (&lt;em&gt;Funding&lt;/em&gt;).&lt;/small&gt;</rdfs:comment>
  </rdf:Description>
  <rdf:Description rdf:about="http://carsten.io/hxl/ns-2012-01-23#Casualty">
    <rdf:type rdf:resource="http://www.w3.org/2000/01/rdf-schema#Class"/>
  </rdf:Description>
  <rdf:Description rdf:about="http://carsten.io/hxl/ns-2012-01-23#Casualty">
    <rdfs:subClassOf rdf:resource="http://carsten.io/hxl/ns-2012-01-23#AffectedPopulation"/>
  </rdf:Description>
  <rdf:Description rdf:about="http://carsten.io/hxl/ns-2012-01-23#Casualty">
    <skos:prefLabel xml:lang="en">Casualty</skos:prefLabel>
  </rdf:Description>
  <rdf:Description rdf:about="http://carsten.io/hxl/ns-2012-01-23#Casualty">
    <rdfs:comment>E.g. injured or dead.&lt;br /&gt;&lt;small&gt;Term origin: ACAPS DSS, Humanitarian Profile.&lt;/small&gt;</rdfs:comment>
  </rdf:Description>
  <rdf:Description rdf:about="http://carsten.io/hxl/ns-2012-01-23#Country">
    <rdf:type rdf:resource="http://www.w3.org/2000/01/rdf-schema#Class"/>
  </rdf:Description>
  <rdf:Description rdf:about="http://carsten.io/hxl/ns-2012-01-23#Country">
    <rdfs:subClassOf rdf:resource="http://carsten.io/hxl/ns-2012-01-23#Location"/>
  </rdf:Description>
  <rdf:Description rdf:about="http://carsten.io/hxl/ns-2012-01-23#Country">
    <skos:prefLabel xml:lang="en">Country</skos:prefLabel>
  </rdf:Description>
  <rdf:Description rdf:about="http://carsten.io/hxl/ns-2012-01-23#Country">
    <rdfs:comment>Geolocation admin level 0.&lt;br /&gt;&lt;small&gt;Term origin: CAP OPS, Sahana Project, ACAPS DSS, CERF, Sigmah DB.&lt;/small&gt;</rdfs:comment>
  </rdf:Description>
  <rdf:Description rdf:about="http://carsten.io/hxl/ns-2012-01-23#Damage">
    <rdf:type rdf:resource="http://www.w3.org/2000/01/rdf-schema#Class"/>
  </rdf:Description>
  <rdf:Description rdf:about="http://carsten.io/hxl/ns-2012-01-23#Damage">
    <skos:prefLabel xml:lang="en">Damage</skos:prefLabel>
  </rdf:Description>
  <rdf:Description rdf:about="http://carsten.io/hxl/ns-2012-01-23#Damage">
    <rdfs:comment>A (reported) damage.&lt;br /&gt;&lt;small&gt;Term origin: ACAPS DSS, Shelter Cluster.&lt;/small&gt;</rdfs:comment>
  </rdf:Description>
  <rdf:Description rdf:about="http://carsten.io/hxl/ns-2012-01-23#DataCollection">
    <rdf:type rdf:resource="http://www.w3.org/2000/01/rdf-schema#Class"/>
  </rdf:Description>
  <rdf:Description rdf:about="http://carsten.io/hxl/ns-2012-01-23#DataCollection">
    <skos:prefLabel xml:lang="en">Data Collection</skos:prefLabel>
  </rdf:Description>
  <rdf:Description rdf:about="http://carsten.io/hxl/ns-2012-01-23#DataCollection">
    <rdfs:comment>The process that leads to a NeedsAssessment of Report. &lt;br /&gt;&lt;small&gt;Term origin: MRM/MARA, HPM Ethiopia.&lt;/small&gt;</rdfs:comment>
  </rdf:Description>
  <rdf:Description rdf:about="http://carsten.io/hxl/ns-2012-01-23#Death">
    <rdf:type rdf:resource="http://www.w3.org/2000/01/rdf-schema#Class"/>
  </rdf:Description>
  <rdf:Description rdf:about="http://carsten.io/hxl/ns-2012-01-23#Death">
    <skos:prefLabel xml:lang="en">Death</skos:prefLabel>
  </rdf:Description>
  <rdf:Description rdf:about="http://carsten.io/hxl/ns-2012-01-23#Death">
    <skos:altLabel xml:lang="en">Dead</skos:altLabel>
  </rdf:Description>
  <rdf:Description rdf:about="http://carsten.io/hxl/ns-2012-01-23#Death">
    <rdfs:subClassOf rdf:resource="http://carsten.io/hxl/ns-2012-01-23#Casualty"/>
  </rdf:Description>
  <rdf:Description rdf:about="http://carsten.io/hxl/ns-2012-01-23#Death">
    <owl:disjointWith rdf:resource="http://carsten.io/hxl/ns-2012-01-23#Injured"/>
  </rdf:Description>
  <rdf:Description rdf:about="http://carsten.io/hxl/ns-2012-01-23#Death">
    <rdfs:comment>A (reported) death.&lt;br /&gt;&lt;small&gt;Term origin: ACAPS DSS, HPM Ethiopia, Shelter Cluster, Humanitarian Profile (&lt;em&gt;Dead&lt;/em&gt;).&lt;/small&gt;</rdfs:comment>
  </rdf:Description>
  <rdf:Description rdf:about="http://carsten.io/hxl/ns-2012-01-23#Displaced">
    <rdf:type rdf:resource="http://www.w3.org/2000/01/rdf-schema#Class"/>
  </rdf:Description>
  <rdf:Description rdf:about="http://carsten.io/hxl/ns-2012-01-23#Displaced">
    <skos:prefLabel xml:lang="en">Displaced</skos:prefLabel>
  </rdf:Description>
  <rdf:Description rdf:about="http://carsten.io/hxl/ns-2012-01-23#Displaced">
    <skos:altLabel xml:lang="en">Displacement</skos:altLabel>
  </rdf:Description>
  <rdf:Description rdf:about="http://carsten.io/hxl/ns-2012-01-23#Displaced">
    <rdfs:subClassOf rdf:resource="http://carsten.io/hxl/ns-2012-01-23#AffectedPopulation"/>
  </rdf:Description>
  <rdf:Description rdf:about="http://carsten.io/hxl/ns-2012-01-23#Displaced">
    <rdfs:comment>Refers to internally displaced persons, refugees, and others of concern.&lt;br /&gt;&lt;small&gt;Term origin: Humanitarian Profile, ACAPS DSS (&lt;em&gt;Displacement&lt;/em&gt;)&lt;/small&gt;</rdfs:comment>
  </rdf:Description>
  <rdf:Description rdf:about="http://carsten.io/hxl/ns-2012-01-23#Displaced">
    <owl:disjointWith rdf:resource="http://carsten.io/hxl/ns-2012-01-23#NonDisplaced"/>
  </rdf:Description>
  <rdf:Description rdf:about="http://carsten.io/hxl/ns-2012-01-23#Donor">
    <rdf:type rdf:resource="http://www.w3.org/2000/01/rdf-schema#Class"/>
  </rdf:Description>
  <rdf:Description rdf:about="http://carsten.io/hxl/ns-2012-01-23#Donor">
    <skos:prefLabel xml:lang="en">Donor</skos:prefLabel>
  </rdf:Description>
  <rdf:Description rdf:about="http://carsten.io/hxl/ns-2012-01-23#Donor">
    <rdfs:subClassOf rdf:resource="http://xmlns.com/foaf/0.1/Agent"/>
  </rdf:Description>
  <rdf:Description rdf:about="http://carsten.io/hxl/ns-2012-01-23#Donor">
    <rdfs:comment xml:lang="en">A donor is an individual or organization donating money for a project or a specific activity.</rdfs:comment>
  </rdf:Description>
  <rdf:Description rdf:about="http://carsten.io/hxl/ns-2012-01-23#NonDisplaced">
    <rdf:type rdf:resource="http://www.w3.org/2000/01/rdf-schema#Class"/>
  </rdf:Description>
  <rdf:Description rdf:about="http://carsten.io/hxl/ns-2012-01-23#NonDisplaced">
    <skos:prefLabel xml:lang="en">Non-Displaced</skos:prefLabel>
  </rdf:Description>
  <rdf:Description rdf:about="http://carsten.io/hxl/ns-2012-01-23#NonDisplaced">
    <rdfs:subClassOf rdf:resource="http://carsten.io/hxl/ns-2012-01-23#AffectedPopulation"/>
  </rdf:Description>
  <rdf:Description rdf:about="http://carsten.io/hxl/ns-2012-01-23#NonDisplaced">
    <rdfs:comment>Refers to the part of the affected population that is not displaced (i.e., host or non-host);.&lt;br /&gt;&lt;small&gt;Term origin: Humanitarian Profile.&lt;/small&gt;</rdfs:comment>
  </rdf:Description>
  <rdf:Description rdf:about="http://carsten.io/hxl/ns-2012-01-23#NonDisplaced">
    <owl:disjointWith rdf:resource="http://carsten.io/hxl/ns-2012-01-23#Displaced"/>
  </rdf:Description>
  <rdf:Description rdf:about="http://carsten.io/hxl/ns-2012-01-23#Emergency">
    <rdf:type rdf:resource="http://www.w3.org/2000/01/rdf-schema#Class"/>
  </rdf:Description>
  <rdf:Description rdf:about="http://carsten.io/hxl/ns-2012-01-23#Emergency">
    <skos:prefLabel xml:lang="en">Emergency</skos:prefLabel>
  </rdf:Description>
  <rdf:Description rdf:about="http://carsten.io/hxl/ns-2012-01-23#Emergency">
    <rdfs:subClassOf rdf:resource="http://carsten.io/hxl/ns-2012-01-23#Situation"/>
  </rdf:Description>
  <rdf:Description rdf:about="http://carsten.io/hxl/ns-2012-01-23#Emergency">
    <rdfs:comment>&lt;p&gt;Any situation in which ... life or well-being ... will be threatened  unless immediate  and  appropriate   action  is  taken,  and  which demands   an   extraordinary   response   and   exceptional measures” (UNHCR Handbook for Emergencies)&lt;/p&gt;&lt;p&gt;A sudden crisis situation or event requiring immediate action (WART) &lt;/p&gt;&lt;p&gt;Any situation in which there is an exceptional and widespread threat to life, health or basic  subsistence,  that  is  beyond  the  coping  capacity  of individuals and the community”  (Oxfam GB Emergency Response Manual). &lt;/p&gt;&lt;p&gt;Where and when a disaster provokes an immediate, exceptional and widespread threat to life, health or basic subsistence, which overwhelms the coping capacity of individual and community, implying need of external assistance” (source: ACFIN Emergency module)&lt;/p&gt;&lt;small&gt;Term origin: CAP OPS, Pakistan SRF, ACAPS DSS, CERF, MIRA.&lt;/small&gt;</rdfs:comment>
  </rdf:Description>
  <rdf:Description rdf:about="http://carsten.io/hxl/ns-2012-01-23#Female">
    <rdf:type rdf:resource="http://www.w3.org/2000/01/rdf-schema#Class"/>
  </rdf:Description>
  <rdf:Description rdf:about="http://carsten.io/hxl/ns-2012-01-23#Female">
    <skos:prefLabel xml:lang="en">Female</skos:prefLabel>
  </rdf:Description>
  <rdf:Description rdf:about="http://carsten.io/hxl/ns-2012-01-23#Female">
    <rdfs:subClassOf rdf:resource="http://xmlns.com/foaf/0.1/Agent"/>
  </rdf:Description>
  <rdf:Description rdf:about="http://carsten.io/hxl/ns-2012-01-23#Female">
    <rdfs:subClassOf rdf:resource="http://carsten.io/hxl/ns-2012-01-23#Gender"/>
  </rdf:Description>
  <rdf:Description rdf:about="http://carsten.io/hxl/ns-2012-01-23#Female">
    <rdfs:comment>A woman/girl or group of women/girls.&lt;br /&gt;&lt;small&gt;Term origin: CERF, EIMS Report.&lt;/small&gt;</rdfs:comment>
  </rdf:Description>
  <rdf:Description rdf:about="http://carsten.io/hxl/ns-2012-01-23#Female">
    <owl:disjointWith rdf:resource="http://carsten.io/hxl/ns-2012-01-23#Male"/>
  </rdf:Description>
  <rdf:Description rdf:about="http://carsten.io/hxl/ns-2012-01-23#Male">
    <rdf:type rdf:resource="http://www.w3.org/2000/01/rdf-schema#Class"/>
  </rdf:Description>
  <rdf:Description rdf:about="http://carsten.io/hxl/ns-2012-01-23#Male">
    <skos:prefLabel xml:lang="en">Male</skos:prefLabel>
  </rdf:Description>
  <rdf:Description rdf:about="http://carsten.io/hxl/ns-2012-01-23#Male">
    <rdfs:subClassOf rdf:resource="http://xmlns.com/foaf/0.1/Agent"/>
  </rdf:Description>
  <rdf:Description rdf:about="http://carsten.io/hxl/ns-2012-01-23#Male">
    <rdfs:subClassOf rdf:resource="http://carsten.io/hxl/ns-2012-01-23#Gender"/>
  </rdf:Description>
  <rdf:Description rdf:about="http://carsten.io/hxl/ns-2012-01-23#Male">
    <rdfs:comment>A man/boy or group of men/boys.&lt;br /&gt;&lt;small&gt;Term origin: CERF, EIMS Report.&lt;/small&gt;</rdfs:comment>
  </rdf:Description>
  <rdf:Description rdf:about="http://carsten.io/hxl/ns-2012-01-23#Male">
    <owl:disjointWith rdf:resource="http://carsten.io/hxl/ns-2012-01-23#Female"/>
  </rdf:Description>
  <rdf:Description rdf:about="http://carsten.io/hxl/ns-2012-01-23#Gender">
    <rdf:type rdf:resource="http://www.w3.org/2000/01/rdf-schema#Class"/>
  </rdf:Description>
  <rdf:Description rdf:about="http://carsten.io/hxl/ns-2012-01-23#Gender">
    <skos:prefLabel xml:lang="en">Gender</skos:prefLabel>
  </rdf:Description>
  <rdf:Description rdf:about="http://carsten.io/hxl/ns-2012-01-23#Gender">
    <rdfs:comment>Class to describe gender-specific issues, either at individual or group level.&lt;br /&gt;&lt;small&gt;Term origin: MIRA, CCDI&lt;/small&gt;</rdfs:comment>
  </rdf:Description>
  <rdf:Description rdf:about="http://carsten.io/hxl/ns-2012-01-23#Need">
    <rdf:type rdf:resource="http://www.w3.org/2000/01/rdf-schema#Class"/>
  </rdf:Description>
  <rdf:Description rdf:about="http://carsten.io/hxl/ns-2012-01-23#Need">
    <skos:prefLabel xml:lang="en">Need</skos:prefLabel>
  </rdf:Description>
  <rdf:Description rdf:about="http://carsten.io/hxl/ns-2012-01-23#Need">
    <skos:altLabel xml:lang="en">Gap</skos:altLabel>
  </rdf:Description>
  <rdf:Description rdf:about="http://carsten.io/hxl/ns-2012-01-23#Need">
    <skos:altLabel xml:lang="en">Lack</skos:altLabel>
  </rdf:Description>
  <rdf:Description rdf:about="http://carsten.io/hxl/ns-2012-01-23#Need">
    <rdfs:comment>A concrete need, lack, or gap, e.g. a shortage of food. Can be based on the application of relevant norms (usually a minimum requirement or a pre-existing ‘normal’ situation); and an assessment of how  the reality differs.	Identifying and measuring deficits, either actual or predicted.&lt;br /&gt;&lt;small&gt;Term origin: CAP OPS, ACAPS DSS (also: &lt;em&gt;Humanitarian Need&lt;/em&gt;), CCDI (&lt;em&gt;Humanitarian Need&lt;/em&gt;), CCDI Shelter Cluster (&lt;em&gt;Gap&lt;/em&gt;), HPM Ethiopia (&lt;em&gt;Gap&lt;/em&gt;).&lt;/small&gt;</rdfs:comment>
  </rdf:Description>
  <rdf:Description rdf:about="http://carsten.io/hxl/ns-2012-01-23#NeedTarget">
    <rdf:type rdf:resource="http://www.w3.org/2000/01/rdf-schema#Class"/>
  </rdf:Description>
  <rdf:Description rdf:about="http://carsten.io/hxl/ns-2012-01-23#NeedTarget">
    <skos:prefLabel xml:lang="en">Need target</skos:prefLabel>
  </rdf:Description>
  <rdf:Description rdf:about="http://carsten.io/hxl/ns-2012-01-23#NeedTarget">
    <rdfs:subClassOf rdf:resource="http://carsten.io/hxl/ns-2012-01-23#Objective"/>
  </rdf:Description>
  <rdf:Description rdf:about="http://carsten.io/hxl/ns-2012-01-23#NeedTarget">
    <rdfs:comment>An objective towards a specific need.</rdfs:comment>
  </rdf:Description>
  <rdf:Description rdf:about="http://carsten.io/hxl/ns-2012-01-23#NeedAchieved">
    <rdf:type rdf:resource="http://www.w3.org/2000/01/rdf-schema#Class"/>
  </rdf:Description>
  <rdf:Description rdf:about="http://carsten.io/hxl/ns-2012-01-23#NeedAchieved">
    <skos:prefLabel xml:lang="en">Need achieved</skos:prefLabel>
  </rdf:Description>
  <rdf:Description rdf:about="http://carsten.io/hxl/ns-2012-01-23#NeedAchieved">
    <rdfs:comment xml:lang="en">The part of a need target that has already been achieved.</rdfs:comment>
  </rdf:Description>
  <rdf:Description rdf:about="http://carsten.io/hxl/ns-2012-01-23#Intervention">
    <rdf:type rdf:resource="http://www.w3.org/2000/01/rdf-schema#Class"/>
  </rdf:Description>
  <rdf:Description rdf:about="http://carsten.io/hxl/ns-2012-01-23#Intervention">
    <skos:prefLabel xml:lang="en">Intervention</skos:prefLabel>
  </rdf:Description>
  <rdf:Description rdf:about="http://carsten.io/hxl/ns-2012-01-23#Intervention">
    <rdfs:subClassOf rdf:resource="http://carsten.io/hxl/ns-2012-01-23#Activity"/>
  </rdf:Description>
  <rdf:Description rdf:about="http://carsten.io/hxl/ns-2012-01-23#Intervention">
    <rdfs:comment>Relief assistance, remedial action, or some other humanitarian intervention; (such  as immunisation, food distribution, etc.).&lt;br /&gt;&lt;small&gt;Term origin: ACAPS.&lt;/small&gt;</rdfs:comment>
  </rdf:Description>
  <rdf:Description rdf:about="http://carsten.io/hxl/ns-2012-01-23#NeedsAssessment">
    <rdf:type rdf:resource="http://www.w3.org/2000/01/rdf-schema#Class"/>
  </rdf:Description>
  <rdf:Description rdf:about="http://carsten.io/hxl/ns-2012-01-23#NeedsAssessment">
    <skos:prefLabel xml:lang="en">Needs Assessment</skos:prefLabel>
  </rdf:Description>
  <rdf:Description rdf:about="http://carsten.io/hxl/ns-2012-01-23#NeedsAssessment">
    <rdfs:subClassOf rdf:resource="http://carsten.io/hxl/ns-2012-01-23#Report"/>
  </rdf:Description>
  <rdf:Description rdf:about="http://carsten.io/hxl/ns-2012-01-23#NeedsAssessment">
    <rdfs:comment>The process of obtaining and analyzing information to determine the current status and service needs of a defined  population and/or geographic area (NOAA definition);.&lt;br /&gt;&lt;small&gt;Term origin: ACAPS.&lt;/small&gt;</rdfs:comment>
  </rdf:Description>
  <rdf:Description rdf:about="http://carsten.io/hxl/ns-2012-01-23#Response">
    <rdf:type rdf:resource="http://www.w3.org/2000/01/rdf-schema#Class"/>
  </rdf:Description>
  <rdf:Description rdf:about="http://carsten.io/hxl/ns-2012-01-23#Response">
    <skos:prefLabel xml:lang="en">Response</skos:prefLabel>
  </rdf:Description>
  <rdf:Description rdf:about="http://carsten.io/hxl/ns-2012-01-23#Response">
    <rdfs:comment>Generic term for the collection of all activities that address the needs araising from an emergency.&lt;br /&gt;&lt;small&gt;Term origin: ACAPS DSS, ACAPS DSS, MIRA, EDXL, CCDI (&lt;em&gt;Humanitarian Response&lt;/em&gt;), CERF (&lt;em&gt;Humanitarian Response&lt;/em&gt;)&lt;/small&gt;</rdfs:comment>
  </rdf:Description>
  <rdf:Description rdf:about="http://carsten.io/hxl/ns-2012-01-23#IDP">
    <rdf:type rdf:resource="http://www.w3.org/2000/01/rdf-schema#Class"/>
  </rdf:Description>
  <rdf:Description rdf:about="http://carsten.io/hxl/ns-2012-01-23#IDP">
    <rdfs:subClassOf rdf:resource="http://carsten.io/hxl/ns-2012-01-23#Displaced"/>
  </rdf:Description>
  <rdf:Description rdf:about="http://carsten.io/hxl/ns-2012-01-23#IDP">
    <skos:prefLabel xml:lang="en">Internally Displaced Person</skos:prefLabel>
  </rdf:Description>
  <rdf:Description rdf:about="http://carsten.io/hxl/ns-2012-01-23#IDP">
    <skos:altLabel xml:lang="en">IDP</skos:altLabel>
  </rdf:Description>
  <rdf:Description rdf:about="http://carsten.io/hxl/ns-2012-01-23#IDP">
    <rdfs:comment>A group of internally displaced persons (IDPs).&lt;br /&gt;&lt;small&gt;Term origin: Humanitarian Profile, CERF, HPM Ethiopia&lt;/small&gt;</rdfs:comment>
  </rdf:Description>
  <rdf:Description rdf:about="http://carsten.io/hxl/ns-2012-01-23#Refugee">
    <rdf:type rdf:resource="http://www.w3.org/2000/01/rdf-schema#Class"/>
  </rdf:Description>
  <rdf:Description rdf:about="http://carsten.io/hxl/ns-2012-01-23#Refugee">
    <rdfs:subClassOf rdf:resource="http://carsten.io/hxl/ns-2012-01-23#Displaced"/>
  </rdf:Description>
  <rdf:Description rdf:about="http://carsten.io/hxl/ns-2012-01-23#Refugee">
    <skos:prefLabel xml:lang="en">Refugee</skos:prefLabel>
  </rdf:Description>
  <rdf:Description rdf:about="http://carsten.io/hxl/ns-2012-01-23#Refugee">
    <rdfs:comment>A group of refugees.&lt;br /&gt;&lt;small&gt;Term origin: Humanitarian Profile&lt;/small&gt;</rdfs:comment>
  </rdf:Description>
  <rdf:Description rdf:about="http://carsten.io/hxl/ns-2012-01-23#AsylumSeeker">
    <rdf:type rdf:resource="http://www.w3.org/2000/01/rdf-schema#Class"/>
  </rdf:Description>
  <rdf:Description rdf:about="http://carsten.io/hxl/ns-2012-01-23#AsylumSeeker">
    <rdfs:subClassOf rdf:resource="http://carsten.io/hxl/ns-2012-01-23#Displaced"/>
  </rdf:Description>
  <rdf:Description rdf:about="http://carsten.io/hxl/ns-2012-01-23#AsylumSeeker">
    <skos:prefLabel xml:lang="en">Asylum Seeker</skos:prefLabel>
  </rdf:Description>
  <rdf:Description rdf:about="http://carsten.io/hxl/ns-2012-01-23#AsylumSeeker">
    <rdfs:comment>A group of asylum seekers.&lt;br /&gt;&lt;small&gt;Term origin: Humanitarian Profile&lt;/small&gt;</rdfs:comment>
  </rdf:Description>
  <rdf:Description rdf:about="http://carsten.io/hxl/ns-2012-01-23#Incident">
    <rdf:type rdf:resource="http://www.w3.org/2000/01/rdf-schema#Class"/>
  </rdf:Description>
  <rdf:Description rdf:about="http://carsten.io/hxl/ns-2012-01-23#Incident">
    <skos:prefLabel xml:lang="en">Incident</skos:prefLabel>
  </rdf:Description>
  <rdf:Description rdf:about="http://carsten.io/hxl/ns-2012-01-23#Incident">
    <rdfs:comment>An individual incident in the context of a crisis, such as a recruitment of children.&lt;br /&gt;&lt;small&gt;Term origin: MRM/MARA, EDXL&lt;/small&gt;</rdfs:comment>
  </rdf:Description>
  <rdf:Description rdf:about="http://carsten.io/hxl/ns-2012-01-23#Indicator">
    <rdf:type rdf:resource="http://www.w3.org/2000/01/rdf-schema#Class"/>
  </rdf:Description>
  <rdf:Description rdf:about="http://carsten.io/hxl/ns-2012-01-23#Indicator">
    <skos:prefLabel xml:lang="en">Indicator</skos:prefLabel>
  </rdf:Description>
  <rdf:Description rdf:about="http://carsten.io/hxl/ns-2012-01-23#Indicator">
    <rdfs:comment>Concrete measurable reference for a concrete need; e.g., &lt;em&gt;5 litres of clean water per person and day&lt;/em&gt;.&lt;br /&gt;&lt;small&gt;Term origin: Pakistan SRF, ACAPS DSS, CCDI, CERF, HPM Ethiopia, Sigmah DB&lt;/small&gt;</rdfs:comment>
  </rdf:Description>
  <rdf:Description rdf:about="http://carsten.io/hxl/ns-2012-01-23#Injured">
    <rdf:type rdf:resource="http://www.w3.org/2000/01/rdf-schema#Class"/>
  </rdf:Description>
  <rdf:Description rdf:about="http://carsten.io/hxl/ns-2012-01-23#Injured">
    <rdfs:subClassOf rdf:resource="http://carsten.io/hxl/ns-2012-01-23#Casualty"/>
  </rdf:Description>
  <rdf:Description rdf:about="http://carsten.io/hxl/ns-2012-01-23#Injured">
    <skos:prefLabel xml:lang="en">Injured</skos:prefLabel>
  </rdf:Description>
  <rdf:Description rdf:about="http://carsten.io/hxl/ns-2012-01-23#Injured">
    <owl:disjointWith rdf:resource="http://carsten.io/hxl/ns-2012-01-23#Death"/>
  </rdf:Description>
  <rdf:Description rdf:about="http://carsten.io/hxl/ns-2012-01-23#Injured">
    <rdfs:comment>Injured part of the population.&lt;br /&gt;&lt;small&gt;Term origin: ACAPS DSS, Humanitarian Profile, Shelter Cluster, HERAMS Checklist (&lt;em&gt;Injury&lt;/em&gt;)&lt;/small&gt;</rdfs:comment>
  </rdf:Description>
  <rdf:Description rdf:about="http://carsten.io/hxl/ns-2012-01-23#Intervention">
    <rdf:type rdf:resource="http://www.w3.org/2000/01/rdf-schema#Class"/>
  </rdf:Description>
  <rdf:Description rdf:about="http://carsten.io/hxl/ns-2012-01-23#Intervention">
    <rdfs:subClassOf rdf:resource="http://carsten.io/hxl/ns-2012-01-23#Activity"/>
  </rdf:Description>
  <rdf:Description rdf:about="http://carsten.io/hxl/ns-2012-01-23#Intervention">
    <skos:prefLabel xml:lang="en">Intervention</skos:prefLabel>
  </rdf:Description>
  <rdf:Description rdf:about="http://carsten.io/hxl/ns-2012-01-23#Intervention">
    <rdfs:comment>&lt;em&gt;Needs further specification; is there any difference between an intervention and an activity?&lt;/em&gt;.&lt;br /&gt;&lt;small&gt;Term origin: MIRA, CCDI, HPM Ethiopia.&lt;/small&gt;</rdfs:comment>
  </rdf:Description>
  <rdf:Description rdf:about="http://carsten.io/hxl/ns-2012-01-23#Killing">
    <rdf:type rdf:resource="http://www.w3.org/2000/01/rdf-schema#Class"/>
  </rdf:Description>
  <rdf:Description rdf:about="http://carsten.io/hxl/ns-2012-01-23#Killing">
    <skos:prefLabel xml:lang="en">Killing</skos:prefLabel>
  </rdf:Description>
  <rdf:Description rdf:about="http://carsten.io/hxl/ns-2012-01-23#Killing">
    <rdfs:subClassOf rdf:resource="http://carsten.io/hxl/ns-2012-01-23#Incident"/>
  </rdf:Description>
  <rdf:Description rdf:about="http://carsten.io/hxl/ns-2012-01-23#Killing">
    <rdfs:comment>A (reported) killing.&lt;br /&gt;&lt;small&gt;Term origin: MRM/MARA, EIMS Report&lt;/small&gt;</rdfs:comment>
  </rdf:Description>
  <rdf:Description rdf:about="http://carsten.io/hxl/ns-2012-01-23#Location">
    <rdf:type rdf:resource="http://www.w3.org/2000/01/rdf-schema#Class"/>
  </rdf:Description>
  <rdf:Description rdf:about="http://carsten.io/hxl/ns-2012-01-23#Location">
    <skos:prefLabel xml:lang="en">Location</skos:prefLabel>
  </rdf:Description>
  <rdf:Description rdf:about="http://carsten.io/hxl/ns-2012-01-23#Location">
    <rdfs:comment>Geolocation - &lt;em&gt;will be further specficied using admin levels and p-codes in the next iteration&lt;/em&gt;.&lt;br /&gt;&lt;small&gt;Term origin: Pakistan SRF, CCDI, EDXL, Shelter Cluster, Sigmah DB&lt;/small&gt;</rdfs:comment>
  </rdf:Description>
  <rdf:Description rdf:about="http://carsten.io/hxl/ns-2012-01-23#Maiming">
    <rdf:type rdf:resource="http://www.w3.org/2000/01/rdf-schema#Class"/>
  </rdf:Description>
  <rdf:Description rdf:about="http://carsten.io/hxl/ns-2012-01-23#Maiming">
    <skos:prefLabel xml:lang="en">Maiming</skos:prefLabel>
  </rdf:Description>
  <rdf:Description rdf:about="http://carsten.io/hxl/ns-2012-01-23#Maiming">
    <rdfs:subClassOf rdf:resource="http://carsten.io/hxl/ns-2012-01-23#Incident"/>
  </rdf:Description>
  <rdf:Description rdf:about="http://carsten.io/hxl/ns-2012-01-23#Maiming">
    <rdfs:comment>A (reported) maiming;.&lt;br /&gt;&lt;small&gt;Term origin: MRM/MARA, EIMS Report&lt;/small&gt;</rdfs:comment>
  </rdf:Description>
  <rdf:Description rdf:about="http://carsten.io/hxl/ns-2012-01-23#Missing">
    <rdf:type rdf:resource="http://www.w3.org/2000/01/rdf-schema#Class"/>
  </rdf:Description>
  <rdf:Description rdf:about="http://carsten.io/hxl/ns-2012-01-23#Missing">
    <skos:prefLabel xml:lang="en">Missing</skos:prefLabel>
  </rdf:Description>
  <rdf:Description rdf:about="http://carsten.io/hxl/ns-2012-01-23#Missing">
    <rdfs:subClassOf rdf:resource="http://carsten.io/hxl/ns-2012-01-23#Casualty"/>
  </rdf:Description>
  <rdf:Description rdf:about="http://carsten.io/hxl/ns-2012-01-23#Missing">
    <owl:disjointWith rdf:resource="http://carsten.io/hxl/ns-2012-01-23#Death"/>
  </rdf:Description>
  <rdf:Description rdf:about="http://carsten.io/hxl/ns-2012-01-23#Missing">
    <rdfs:comment>Missing population.&lt;br /&gt;&lt;small&gt;Term origin: Humanitarian Profile.&lt;/small&gt;</rdfs:comment>
  </rdf:Description>
  <rdf:Description rdf:about="http://carsten.io/hxl/ns-2012-01-23#Objective">
    <rdf:type rdf:resource="http://www.w3.org/2000/01/rdf-schema#Class"/>
  </rdf:Description>
  <rdf:Description rdf:about="http://carsten.io/hxl/ns-2012-01-23#Objective">
    <skos:prefLabel xml:lang="en">Objective</skos:prefLabel>
  </rdf:Description>
  <rdf:Description rdf:about="http://carsten.io/hxl/ns-2012-01-23#Objective">
    <rdfs:comment>And objective is a goal for an activity, measureable in terms of an indicator.&lt;br /&gt;&lt;small&gt;Term origin: Sahana Project, CERF&lt;/small&gt;</rdfs:comment>
  </rdf:Description>
  <rdf:Description rdf:about="http://carsten.io/hxl/ns-2012-01-23#Organization">
    <rdf:type rdf:resource="http://www.w3.org/2000/01/rdf-schema#Class"/>
  </rdf:Description>
  <rdf:Description rdf:about="http://carsten.io/hxl/ns-2012-01-23#Organization">
    <rdfs:subClassOf rdf:resource="http://xmlns.com/foaf/0.1/Organization"/>
  </rdf:Description>
  <rdf:Description rdf:about="http://carsten.io/hxl/ns-2012-01-23#Organization">
    <skos:prefLabel xml:lang="en">Organization</skos:prefLabel>
  </rdf:Description>
  <rdf:Description rdf:about="http://carsten.io/hxl/ns-2012-01-23#Organization">
    <rdfs:comment>A humanitarian organization.&lt;br /&gt;&lt;small&gt;Term origin: IATI, CAP OPS, Pakistan SRF, EIMS Report,	Shelter Cluster, Sigmah DB.&lt;/small&gt;</rdfs:comment>
  </rdf:Description>
  <rdf:Description rdf:about="http://carsten.io/hxl/ns-2012-01-23#Output">
    <rdf:type rdf:resource="http://www.w3.org/2000/01/rdf-schema#Class"/>
  </rdf:Description>
  <rdf:Description rdf:about="http://carsten.io/hxl/ns-2012-01-23#Output">
    <skos:prefLabel xml:lang="en">Output</skos:prefLabel>
  </rdf:Description>
  <rdf:Description rdf:about="http://carsten.io/hxl/ns-2012-01-23#Output">
    <rdfs:comment>&lt;em&gt;Merge with &lt;strong&gt;objective&lt;/strong&gt;?&lt;/em&gt;.&lt;br /&gt;&lt;small&gt;Term origin: CAP OPS, Sahana Project&lt;/small&gt;</rdfs:comment>
  </rdf:Description>
  <rdf:Description rdf:about="http://carsten.io/hxl/ns-2012-01-23#Priority">
    <rdf:type rdf:resource="http://www.w3.org/2000/01/rdf-schema#Class"/>
  </rdf:Description>
  <rdf:Description rdf:about="http://carsten.io/hxl/ns-2012-01-23#Priority">
    <skos:prefLabel xml:lang="en">Priority</skos:prefLabel>
  </rdf:Description>
  <rdf:Description rdf:about="http://carsten.io/hxl/ns-2012-01-23#Priority">
    <rdfs:comment>The priority for a project or activity. Individuals of this class should be created whenever a fixed scale for priorities is in use.&lt;br /&gt;&lt;small&gt;Term origin: CAP OPS, UNHCR Camp DB, Sahana Project, MIRA, HPM Ethiopia.&lt;/small&gt;</rdfs:comment>
  </rdf:Description>
  <rdf:Description rdf:about="http://carsten.io/hxl/ns-2012-01-23#Project">
    <rdf:type rdf:resource="http://www.w3.org/2000/01/rdf-schema#Class"/>
  </rdf:Description>
  <rdf:Description rdf:about="http://carsten.io/hxl/ns-2012-01-23#Project">
    <rdfs:subClassOf rdf:resource="http://carsten.io/hxl/ns-2012-01-23#Activity"/>
  </rdf:Description>
  <rdf:Description rdf:about="http://carsten.io/hxl/ns-2012-01-23#Project">
    <skos:prefLabel xml:lang="en">Project</skos:prefLabel>
  </rdf:Description>
  <rdf:Description rdf:about="http://carsten.io/hxl/ns-2012-01-23#Project">
    <rdfs:comment>A project is a specific activity or intervention (or collection of these)	that have been grouped for management purposes.&lt;br /&gt;&lt;small&gt;Term origin: CAP OPS, Pakistan SRF, Sahana Project, Sigmah DB. &lt;/small&gt;</rdfs:comment>
  </rdf:Description>
  <rdf:Description rdf:about="http://carsten.io/hxl/ns-2012-01-23#Region">
    <rdf:type rdf:resource="http://www.w3.org/2000/01/rdf-schema#Class"/>
  </rdf:Description>
  <rdf:Description rdf:about="http://carsten.io/hxl/ns-2012-01-23#Region">
    <skos:prefLabel xml:lang="en">Region</skos:prefLabel>
  </rdf:Description>
  <rdf:Description rdf:about="http://carsten.io/hxl/ns-2012-01-23#Region">
    <rdfs:subClassOf rdf:resource="http://carsten.io/hxl/ns-2012-01-23#Location"/>
  </rdf:Description>
  <rdf:Description rdf:about="http://carsten.io/hxl/ns-2012-01-23#Region">
    <rdfs:comment>Geolocation admin level 1.&lt;br /&gt;&lt;small&gt;Term origin: ACAPS DSS,	CCDI, CERF, HPM Ethiopia.&lt;/small&gt;</rdfs:comment>
  </rdf:Description>
  <rdf:Description rdf:about="http://carsten.io/hxl/ns-2012-01-23#Report">
    <rdf:type rdf:resource="http://www.w3.org/2000/01/rdf-schema#Class"/>
  </rdf:Description>
  <rdf:Description rdf:about="http://carsten.io/hxl/ns-2012-01-23#Report">
    <skos:prefLabel xml:lang="en">Report</skos:prefLabel>
  </rdf:Description>
  <rdf:Description rdf:about="http://carsten.io/hxl/ns-2012-01-23#Report">
    <rdfs:subClassOf rdf:resource="http://xmlns.com/foaf/0.1/Document"/>
  </rdf:Description>
  <rdf:Description rdf:about="http://carsten.io/hxl/ns-2012-01-23#Report">
    <rdfs:comment>Generic class for any kind of report (such as a needs assessment or project report).</rdfs:comment>
  </rdf:Description>
  <rdf:Description rdf:about="http://carsten.io/hxl/ns-2012-01-23#ReportingPeriod">
    <rdf:type rdf:resource="http://www.w3.org/2000/01/rdf-schema#Class"/>
  </rdf:Description>
  <rdf:Description rdf:about="http://carsten.io/hxl/ns-2012-01-23#ReportingPeriod">
    <skos:prefLabel xml:lang="en">Reporting Period</skos:prefLabel>
  </rdf:Description>
  <rdf:Description rdf:about="http://carsten.io/hxl/ns-2012-01-23#ReportingPeriod">
    <rdfs:comment>The time frame that a report covers.&lt;br /&gt;&lt;small&gt;Term origin: Sigmah DB.&lt;/small&gt;</rdfs:comment>
  </rdf:Description>
  <rdf:Description rdf:about="http://carsten.io/hxl/ns-2012-01-23#RuralPopulation">
    <rdf:type rdf:resource="http://www.w3.org/2000/01/rdf-schema#Class"/>
  </rdf:Description>
  <rdf:Description rdf:about="http://carsten.io/hxl/ns-2012-01-23#RuralPopulation">
    <skos:prefLabel xml:lang="en">Rural Population</skos:prefLabel>
  </rdf:Description>
  <rdf:Description rdf:about="http://carsten.io/hxl/ns-2012-01-23#RuralPopulation">
    <rdfs:subClassOf rdf:resource="http://carsten.io/hxl/ns-2012-01-23#Population"/>
  </rdf:Description>
  <rdf:Description rdf:about="http://carsten.io/hxl/ns-2012-01-23#RuralPopulation">
    <rdfs:comment>Population living in the countryside.&lt;br /&gt;&lt;small&gt;Term origin: HPM Ethiopia, Shelter Cluster.&lt;/small&gt;</rdfs:comment>
  </rdf:Description>
  <rdf:Description rdf:about="http://carsten.io/hxl/ns-2012-01-23#RuralPopulation">
    <owl:disjointWith rdf:resource="http://carsten.io/hxl/ns-2012-01-23#UrbanPopulation"/>
  </rdf:Description>
  <rdf:Description rdf:about="http://carsten.io/hxl/ns-2012-01-23#UrbanPopulation">
    <rdf:type rdf:resource="http://www.w3.org/2000/01/rdf-schema#Class"/>
  </rdf:Description>
  <rdf:Description rdf:about="http://carsten.io/hxl/ns-2012-01-23#UrbanPopulation">
    <skos:prefLabel xml:lang="en">Urban Population</skos:prefLabel>
  </rdf:Description>
  <rdf:Description rdf:about="http://carsten.io/hxl/ns-2012-01-23#UrbanPopulation">
    <rdfs:subClassOf rdf:resource="http://carsten.io/hxl/ns-2012-01-23#Population"/>
  </rdf:Description>
  <rdf:Description rdf:about="http://carsten.io/hxl/ns-2012-01-23#UrbanPopulation">
    <rdfs:comment>Population living in cities.&lt;br /&gt;&lt;small&gt;Term origin: Shelter Cluster.&lt;/small&gt;</rdfs:comment>
  </rdf:Description>
  <rdf:Description rdf:about="http://carsten.io/hxl/ns-2012-01-23#UrbanPopulation">
    <owl:disjointWith rdf:resource="http://carsten.io/hxl/ns-2012-01-23#RuralPopulation"/>
  </rdf:Description>
  <rdf:Description rdf:about="http://carsten.io/hxl/ns-2012-01-23#Sector">
    <rdf:type rdf:resource="http://www.w3.org/2000/01/rdf-schema#Class"/>
  </rdf:Description>
  <rdf:Description rdf:about="http://carsten.io/hxl/ns-2012-01-23#Sector">
    <skos:prefLabel xml:lang="en">Sector</skos:prefLabel>
  </rdf:Description>
  <rdf:Description rdf:about="http://carsten.io/hxl/ns-2012-01-23#Sector">
    <rdfs:comment xml:lang="en">A sector adresses a specific thematic area in an Emergency, e.g. Health or Logistics.&lt;br /&gt;&lt;small&gt;Term origin: IATI, CAP OPS, UNHCR Camp DB, Pakistan SRF, ACAPS DSS, MIRA, CERF, HPM Ethiopia&lt;/small&gt;.</rdfs:comment>
  </rdf:Description>
  <rdf:Description rdf:about="http://carsten.io/hxl/ns-2012-01-23#Site">
    <rdf:type rdf:resource="http://www.w3.org/2000/01/rdf-schema#Class"/>
  </rdf:Description>
  <rdf:Description rdf:about="http://carsten.io/hxl/ns-2012-01-23#Site">
    <skos:prefLabel xml:lang="en">Site</skos:prefLabel>
  </rdf:Description>
  <rdf:Description rdf:about="http://carsten.io/hxl/ns-2012-01-23#Site">
    <rdfs:comment xml:lang="en">&lt;em&gt;What sites other than camps do we have?&lt;/em&gt;&lt;br /&gt;&lt;small&gt;Term origin: EIMS Report	Sigmah DB.&lt;/small&gt;</rdfs:comment>
  </rdf:Description>
  <rdf:Description rdf:about="http://carsten.io/hxl/ns-2012-01-23#Shelter">
    <rdf:type rdf:resource="http://www.w3.org/2000/01/rdf-schema#Class"/>
  </rdf:Description>
  <rdf:Description rdf:about="http://carsten.io/hxl/ns-2012-01-23#Shelter">
    <skos:prefLabel xml:lang="en">Shelter</skos:prefLabel>
  </rdf:Description>
  <rdf:Description rdf:about="http://carsten.io/hxl/ns-2012-01-23#Shelter">
    <rdfs:comment>A structure that provides privacy and protection from danger (WordNet).&lt;br /&gt;&lt;small&gt;Term origin: UNHCR Camp DB, ACAPS DSS.&lt;/small&gt;</rdfs:comment>
  </rdf:Description>
  <rdf:Description rdf:about="http://carsten.io/hxl/ns-2012-01-23#SubRegion">
    <rdf:type rdf:resource="http://www.w3.org/2000/01/rdf-schema#Class"/>
  </rdf:Description>
  <rdf:Description rdf:about="http://carsten.io/hxl/ns-2012-01-23#SubRegion">
    <skos:prefLabel xml:lang="en">Sub Region</skos:prefLabel>
  </rdf:Description>
  <rdf:Description rdf:about="http://carsten.io/hxl/ns-2012-01-23#SubRegion">
    <rdfs:subClassOf rdf:resource="http://carsten.io/hxl/ns-2012-01-23#Location"/>
  </rdf:Description>
  <rdf:Description rdf:about="http://carsten.io/hxl/ns-2012-01-23#SubRegion">
    <rdfs:comment>Geolocation admin level 2.&lt;br /&gt;&lt;small&gt;Term origin: CCDI, CERF.&lt;/small&gt;</rdfs:comment>
  </rdf:Description>
  <rdf:Description rdf:about="http://carsten.io/hxl/ns-2012-01-23#TotalPopulation">
    <rdf:type rdf:resource="http://www.w3.org/2000/01/rdf-schema#Class"/>
  </rdf:Description>
  <rdf:Description rdf:about="http://carsten.io/hxl/ns-2012-01-23#TotalPopulation">
    <rdfs:subClassOf rdf:resource="http://carsten.io/hxl/ns-2012-01-23#Population"/>
  </rdf:Description>
  <rdf:Description rdf:about="http://carsten.io/hxl/ns-2012-01-23#TotalPopulation">
    <skos:prefLabel xml:lang="en">Total Population</skos:prefLabel>
  </rdf:Description>
  <rdf:Description rdf:about="http://carsten.io/hxl/ns-2012-01-23#TotalPopulation">
    <rdfs:comment>The total population for an administrative unit (e.g. a region).&lt;br /&gt;&lt;small&gt;Term origin: Shelter Cluster.&lt;/small&gt;</rdfs:comment>
  </rdf:Description>
  <rdf:Description rdf:about="http://carsten.io/hxl/ns-2012-01-23#affectedBy">
    <rdf:type rdf:resource="http://www.w3.org/1999/02/22-rdf-syntax-ns#Property"/>
  </rdf:Description>
  <rdf:Description rdf:about="http://carsten.io/hxl/ns-2012-01-23#affectedBy">
    <rdf:type rdf:resource="http://www.w3.org/2002/07/owl#ObjectProperty"/>
  </rdf:Description>
  <rdf:Description rdf:about="http://carsten.io/hxl/ns-2012-01-23#affectedBy">
    <skos:prefLabel xml:lang="en">affected by</skos:prefLabel>
  </rdf:Description>
  <rdf:Description rdf:about="http://carsten.io/hxl/ns-2012-01-23#affectedBy">
    <rdfs:comment xml:lang="en">States that a Population is affacted by an Emergency.</rdfs:comment>
  </rdf:Description>
  <rdf:Description rdf:about="http://carsten.io/hxl/ns-2012-01-23#affectedBy">
    <rdfs:domain rdf:resource="http://carsten.io/hxl/ns-2012-01-23#AffectedPopulation"/>
  </rdf:Description>
  <rdf:Description rdf:about="http://carsten.io/hxl/ns-2012-01-23#affectedBy">
    <rdfs:range rdf:resource="http://carsten.io/hxl/ns-2012-01-23#Emergency"/>
  </rdf:Description>
  <rdf:Description rdf:about="http://carsten.io/hxl/ns-2012-01-23#addresses">
    <rdf:type rdf:resource="http://www.w3.org/1999/02/22-rdf-syntax-ns#Property"/>
  </rdf:Description>
  <rdf:Description rdf:about="http://carsten.io/hxl/ns-2012-01-23#addresses">
    <rdf:type rdf:resource="http://www.w3.org/2002/07/owl#ObjectProperty"/>
  </rdf:Description>
  <rdf:Description rdf:about="http://carsten.io/hxl/ns-2012-01-23#addresses">
    <skos:prefLabel xml:lang="en">addresses</skos:prefLabel>
  </rdf:Description>
  <rdf:Description rdf:about="http://carsten.io/hxl/ns-2012-01-23#addresses">
    <rdfs:comment xml:lang="en">States that a certain activity addresses a situation description.</rdfs:comment>
  </rdf:Description>
  <rdf:Description rdf:about="http://carsten.io/hxl/ns-2012-01-23#addresses">
    <rdfs:domain rdf:resource="http://carsten.io/hxl/ns-2012-01-23#Response"/>
  </rdf:Description>
  <rdf:Description rdf:about="http://carsten.io/hxl/ns-2012-01-23#addresses">
    <rdfs:domain rdf:resource="http://carsten.io/hxl/ns-2012-01-23#Activity"/>
  </rdf:Description>
  <rdf:Description rdf:about="http://carsten.io/hxl/ns-2012-01-23#addresses">
    <rdfs:range rdf:resource="http://carsten.io/hxl/ns-2012-01-23#Emergency"/>
  </rdf:Description>
  <rdf:Description rdf:about="http://carsten.io/hxl/ns-2012-01-23#addresses">
    <rdfs:range rdf:resource="http://carsten.io/hxl/ns-2012-01-23#Need"/>
  </rdf:Description>
  <rdf:Description rdf:about="http://carsten.io/hxl/ns-2012-01-23#contributesTo">
    <rdf:type rdf:resource="http://www.w3.org/1999/02/22-rdf-syntax-ns#Property"/>
  </rdf:Description>
  <rdf:Description rdf:about="http://carsten.io/hxl/ns-2012-01-23#contributesTo">
    <rdf:type rdf:resource="http://www.w3.org/2002/07/owl#ObjectProperty"/>
  </rdf:Description>
  <rdf:Description rdf:about="http://carsten.io/hxl/ns-2012-01-23#contributesTo">
    <skos:prefLabel xml:lang="en">contributes to</skos:prefLabel>
  </rdf:Description>
  <rdf:Description rdf:about="http://carsten.io/hxl/ns-2012-01-23#contributesTo">
    <rdfs:comment xml:lang="en">Specifiies the relationship between a donor and the project or activity budget he contributes money to.</rdfs:comment>
  </rdf:Description>
  <rdf:Description rdf:about="http://carsten.io/hxl/ns-2012-01-23#contributesTo">
    <rdfs:domain rdf:resource="http://carsten.io/hxl/ns-2012-01-23#Donor"/>
  </rdf:Description>
  <rdf:Description rdf:about="http://carsten.io/hxl/ns-2012-01-23#contributesTo">
    <rdfs:range rdf:resource="http://carsten.io/hxl/ns-2012-01-23#Budget"/>
  </rdf:Description>
  <rdf:Description rdf:about="http://carsten.io/hxl/ns-2012-01-23#leadBy">
    <rdf:type rdf:resource="http://www.w3.org/1999/02/22-rdf-syntax-ns#Property"/>
  </rdf:Description>
  <rdf:Description rdf:about="http://carsten.io/hxl/ns-2012-01-23#leadBy">
    <rdf:type rdf:resource="http://www.w3.org/2002/07/owl#ObjectProperty"/>
  </rdf:Description>
  <rdf:Description rdf:about="http://carsten.io/hxl/ns-2012-01-23#leadBy">
    <skos:prefLabel xml:lang="en">lead By</skos:prefLabel>
  </rdf:Description>
  <rdf:Description rdf:about="http://carsten.io/hxl/ns-2012-01-23#leadBy">
    <rdfs:comment xml:lang="en">Relates a cluster to its leading Agency.</rdfs:comment>
  </rdf:Description>
  <rdf:Description rdf:about="http://carsten.io/hxl/ns-2012-01-23#leadBy">
    <rdfs:domain rdf:resource="http://carsten.io/hxl/ns-2012-01-23#Cluster"/>
  </rdf:Description>
  <rdf:Description rdf:about="http://carsten.io/hxl/ns-2012-01-23#leadBy">
    <rdfs:range rdf:resource="http://carsten.io/hxl/ns-2012-01-23#Agency"/>
  </rdf:Description>
  <rdf:Description rdf:about="http://carsten.io/hxl/ns-2012-01-23#fromAge">
    <rdf:type rdf:resource="http://www.w3.org/1999/02/22-rdf-syntax-ns#Property"/>
  </rdf:Description>
  <rdf:Description rdf:about="http://carsten.io/hxl/ns-2012-01-23#fromAge">
    <rdf:type rdf:resource="http://www.w3.org/2002/07/owl#DataProperty"/>
  </rdf:Description>
  <rdf:Description rdf:about="http://carsten.io/hxl/ns-2012-01-23#fromAge">
    <skos:prefLabel xml:lang="en">from age</skos:prefLabel>
  </rdf:Description>
  <rdf:Description rdf:about="http://carsten.io/hxl/ns-2012-01-23#fromAge">
    <rdfs:comment>Specifies the bottom of an age range for an AgeGroup (in years).</rdfs:comment>
  </rdf:Description>
  <rdf:Description rdf:about="http://carsten.io/hxl/ns-2012-01-23#fromAge">
    <rdfs:domain rdf:resource="http://carsten.io/hxl/ns-2012-01-23#AgeGroup"/>
  </rdf:Description>
  <rdf:Description rdf:about="http://carsten.io/hxl/ns-2012-01-23#fromAge">
    <rdfs:range rdf:resource="http://www.w3.org/2001/XMLSchema#int"/>
  </rdf:Description>
  <rdf:Description rdf:about="http://carsten.io/hxl/ns-2012-01-23#toAge">
    <rdf:type rdf:resource="http://www.w3.org/1999/02/22-rdf-syntax-ns#Property"/>
  </rdf:Description>
  <rdf:Description rdf:about="http://carsten.io/hxl/ns-2012-01-23#toAge">
    <rdf:type rdf:resource="http://www.w3.org/2002/07/owl#DataProperty"/>
  </rdf:Description>
  <rdf:Description rdf:about="http://carsten.io/hxl/ns-2012-01-23#toAge">
    <skos:prefLabel xml:lang="en">to age</skos:prefLabel>
  </rdf:Description>
  <rdf:Description rdf:about="http://carsten.io/hxl/ns-2012-01-23#toAge">
    <rdfs:comment>Specifies the top of an age range for an AgeGroup (in years).</rdfs:comment>
  </rdf:Description>
  <rdf:Description rdf:about="http://carsten.io/hxl/ns-2012-01-23#toAge">
    <rdfs:domain rdf:resource="http://carsten.io/hxl/ns-2012-01-23#AgeGroup"/>
  </rdf:Description>
  <rdf:Description rdf:about="http://carsten.io/hxl/ns-2012-01-23#toAge">
    <rdfs:range rdf:resource="http://www.w3.org/2001/XMLSchema#int"/>
  </rdf:Description>
  <rdf:Description rdf:about="http://carsten.io/hxl/ns-2012-01-23#start">
    <rdf:type rdf:resource="http://www.w3.org/1999/02/22-rdf-syntax-ns#Property"/>
  </rdf:Description>
  <rdf:Description rdf:about="http://carsten.io/hxl/ns-2012-01-23#start">
    <rdf:type rdf:resource="http://www.w3.org/2002/07/owl#DataProperty"/>
  </rdf:Description>
  <rdf:Description rdf:about="http://carsten.io/hxl/ns-2012-01-23#start">
    <skos:prefLabel xml:lang="en">start</skos:prefLabel>
  </rdf:Description>
  <rdf:Description rdf:about="http://carsten.io/hxl/ns-2012-01-23#start">
    <rdfs:comment>Specifies the start of activities, projects, etc.</rdfs:comment>
  </rdf:Description>
  <rdf:Description rdf:about="http://carsten.io/hxl/ns-2012-01-23#start">
    <rdfs:domain rdf:resource="http://carsten.io/hxl/ns-2012-01-23#Activity"/>
  </rdf:Description>
  <rdf:Description rdf:about="http://carsten.io/hxl/ns-2012-01-23#start">
    <rdfs:domain rdf:resource="http://carsten.io/hxl/ns-2012-01-23#Emergency"/>
  </rdf:Description>
  <rdf:Description rdf:about="http://carsten.io/hxl/ns-2012-01-23#start">
    <rdfs:domain rdf:resource="http://carsten.io/hxl/ns-2012-01-23#ReportingPeriod"/>
  </rdf:Description>
  <rdf:Description rdf:about="http://carsten.io/hxl/ns-2012-01-23#start">
    <rdfs:range rdf:resource="http://www.w3.org/2001/XMLSchema#date"/>
  </rdf:Description>
  <rdf:Description rdf:about="http://carsten.io/hxl/ns-2012-01-23#end">
    <rdf:type rdf:resource="http://www.w3.org/1999/02/22-rdf-syntax-ns#Property"/>
  </rdf:Description>
  <rdf:Description rdf:about="http://carsten.io/hxl/ns-2012-01-23#end">
    <rdf:type rdf:resource="http://www.w3.org/2002/07/owl#DataProperty"/>
  </rdf:Description>
  <rdf:Description rdf:about="http://carsten.io/hxl/ns-2012-01-23#end">
    <skos:prefLabel xml:lang="en">end</skos:prefLabel>
  </rdf:Description>
  <rdf:Description rdf:about="http://carsten.io/hxl/ns-2012-01-23#end">
    <rdfs:comment>Specifies the end of activities, projects, etc.</rdfs:comment>
  </rdf:Description>
  <rdf:Description rdf:about="http://carsten.io/hxl/ns-2012-01-23#end">
    <rdfs:domain rdf:resource="http://carsten.io/hxl/ns-2012-01-23#Activity"/>
  </rdf:Description>
  <rdf:Description rdf:about="http://carsten.io/hxl/ns-2012-01-23#end">
    <rdfs:domain rdf:resource="http://carsten.io/hxl/ns-2012-01-23#Emergency"/>
  </rdf:Description>
  <rdf:Description rdf:about="http://carsten.io/hxl/ns-2012-01-23#end">
    <rdfs:domain rdf:resource="http://carsten.io/hxl/ns-2012-01-23#ReportingPeriod"/>
  </rdf:Description>
  <rdf:Description rdf:about="http://carsten.io/hxl/ns-2012-01-23#end">
    <rdfs:range rdf:resource="http://www.w3.org/2001/XMLSchema#date"/>
  </rdf:Description>
  <rdf:Description rdf:about="http://carsten.io/hxl/ns-2012-01-23#partOf">
    <rdf:type rdf:resource="http://www.w3.org/1999/02/22-rdf-syntax-ns#Property"/>
  </rdf:Description>
  <rdf:Description rdf:about="http://carsten.io/hxl/ns-2012-01-23#partOf">
    <skos:prefLabel xml:lang="en">part of</skos:prefLabel>
  </rdf:Description>
  <rdf:Description rdf:about="http://carsten.io/hxl/ns-2012-01-23#partOf">
    <rdfs:subPropertyOf rdf:resource="http://purl.org/dc/terms/partOf"/>
  </rdf:Description>
  <rdf:Description rdf:about="http://carsten.io/hxl/ns-2012-01-23#partOf">
    <rdfs:comment xml:lang="en">Specifies part-whole relationships; e.g., a specific Project can be partOf the Response to a certain Emergency.</rdfs:comment>
  </rdf:Description>
  <rdf:Description rdf:about="http://carsten.io/hxl/ns-2012-01-23#partOf">
    <rdfs:domain rdf:resource="http://carsten.io/hxl/ns-2012-01-23#Activity"/>
  </rdf:Description>
  <rdf:Description rdf:about="http://carsten.io/hxl/ns-2012-01-23#partOf">
    <rdfs:range rdf:resource="http://carsten.io/hxl/ns-2012-01-23#Response"/>
  </rdf:Description>
  <rdf:Description rdf:about="http://carsten.io/hxl/ns-2012-01-23#partOf">
    <rdfs:range rdf:resource="http://carsten.io/hxl/ns-2012-01-23#Activity"/>
  </rdf:Description>
  <rdf:Description rdf:about="http://carsten.io/hxl/ns-2012-01-23#hasBudget">
    <rdf:type rdf:resource="http://www.w3.org/1999/02/22-rdf-syntax-ns#Property"/>
  </rdf:Description>
  <rdf:Description rdf:about="http://carsten.io/hxl/ns-2012-01-23#hasBudget">
    <rdf:type rdf:resource="http://www.w3.org/2002/07/owl#ObjectProperty"/>
  </rdf:Description>
  <rdf:Description rdf:about="http://carsten.io/hxl/ns-2012-01-23#hasBudget">
    <skos:prefLabel xml:lang="en">has budget</skos:prefLabel>
  </rdf:Description>
  <rdf:Description rdf:about="http://carsten.io/hxl/ns-2012-01-23#hasBudget">
    <rdfs:comment xml:lang="en">Links a specific budget to a Project or Activity.</rdfs:comment>
  </rdf:Description>
  <rdf:Description rdf:about="http://carsten.io/hxl/ns-2012-01-23#hasBudget">
    <rdfs:domain rdf:resource="http://carsten.io/hxl/ns-2012-01-23#Activity"/>
  </rdf:Description>
  <rdf:Description rdf:about="http://carsten.io/hxl/ns-2012-01-23#hasBudget">
    <rdfs:range rdf:resource="http://carsten.io/hxl/ns-2012-01-23#Budget"/>
  </rdf:Description>
  <rdf:Description rdf:about="http://carsten.io/hxl/ns-2012-01-23#raisedBy">
    <rdf:type rdf:resource="http://www.w3.org/1999/02/22-rdf-syntax-ns#Property"/>
  </rdf:Description>
  <rdf:Description rdf:about="http://carsten.io/hxl/ns-2012-01-23#raisedBy">
    <rdf:type rdf:resource="http://www.w3.org/2002/07/owl#ObjectProperty"/>
  </rdf:Description>
  <rdf:Description rdf:about="http://carsten.io/hxl/ns-2012-01-23#raisedBy">
    <skos:prefLabel xml:lang="en">raises</skos:prefLabel>
  </rdf:Description>
  <rdf:Description rdf:about="http://carsten.io/hxl/ns-2012-01-23#raisedBy">
    <rdfs:comment xml:lang="en">Provenance record for a specific budget that links it back to the appeal it was raised through.</rdfs:comment>
  </rdf:Description>
  <rdf:Description rdf:about="http://carsten.io/hxl/ns-2012-01-23#raisedBy">
    <rdfs:domain rdf:resource="http://carsten.io/hxl/ns-2012-01-23#Budget"/>
  </rdf:Description>
  <rdf:Description rdf:about="http://carsten.io/hxl/ns-2012-01-23#raisedBy">
    <rdfs:range rdf:resource="http://carsten.io/hxl/ns-2012-01-23#Appeal"/>
  </rdf:Description>
  <rdf:Description rdf:about="http://carsten.io/hxl/ns-2012-01-23#subBudgetOf">
    <rdf:type rdf:resource="http://www.w3.org/1999/02/22-rdf-syntax-ns#Property"/>
  </rdf:Description>
  <rdf:Description rdf:about="http://carsten.io/hxl/ns-2012-01-23#subBudgetOf">
    <rdf:type rdf:resource="http://www.w3.org/2002/07/owl#ObjectProperty"/>
  </rdf:Description>
  <rdf:Description rdf:about="http://carsten.io/hxl/ns-2012-01-23#subBudgetOf">
    <skos:prefLabel xml:lang="en">sub-budget of</skos:prefLabel>
  </rdf:Description>
  <rdf:Description rdf:about="http://carsten.io/hxl/ns-2012-01-23#subBudgetOf">
    <rdfs:comment xml:lang="en">Supports adding up budgets for different activities to the budget of a project.</rdfs:comment>
  </rdf:Description>
  <rdf:Description rdf:about="http://carsten.io/hxl/ns-2012-01-23#subBudgetOf">
    <rdfs:domain rdf:resource="http://carsten.io/hxl/ns-2012-01-23#Budget"/>
  </rdf:Description>
  <rdf:Description rdf:about="http://carsten.io/hxl/ns-2012-01-23#subBudgetOf">
    <rdfs:range rdf:resource="http://carsten.io/hxl/ns-2012-01-23#Budget"/>
  </rdf:Description>
  <rdf:Description rdf:about="http://carsten.io/hxl/ns-2012-01-23#identifies">
    <rdf:type rdf:resource="http://www.w3.org/1999/02/22-rdf-syntax-ns#Property"/>
  </rdf:Description>
  <rdf:Description rdf:about="http://carsten.io/hxl/ns-2012-01-23#identifies">
    <rdf:type rdf:resource="http://www.w3.org/2002/07/owl#ObjectProperty"/>
  </rdf:Description>
  <rdf:Description rdf:about="http://carsten.io/hxl/ns-2012-01-23#identifies">
    <skos:prefLabel xml:lang="en">identifies</skos:prefLabel>
  </rdf:Description>
  <rdf:Description rdf:about="http://carsten.io/hxl/ns-2012-01-23#identifies">
    <rdfs:comment xml:lang="en">Links a NeedsAssessment to the different Needs it identifies.</rdfs:comment>
  </rdf:Description>
  <rdf:Description rdf:about="http://carsten.io/hxl/ns-2012-01-23#identifies">
    <rdfs:domain rdf:resource="http://carsten.io/hxl/ns-2012-01-23#NeedsAssessment"/>
  </rdf:Description>
  <rdf:Description rdf:about="http://carsten.io/hxl/ns-2012-01-23#identifies">
    <rdfs:range rdf:resource="http://carsten.io/hxl/ns-2012-01-23#Need"/>
  </rdf:Description>
  <rdf:Description rdf:about="http://carsten.io/hxl/ns-2012-01-23#analyzes">
    <rdf:type rdf:resource="http://www.w3.org/1999/02/22-rdf-syntax-ns#Property"/>
  </rdf:Description>
  <rdf:Description rdf:about="http://carsten.io/hxl/ns-2012-01-23#analyzes">
    <rdf:type rdf:resource="http://www.w3.org/2002/07/owl#ObjectProperty"/>
  </rdf:Description>
  <rdf:Description rdf:about="http://carsten.io/hxl/ns-2012-01-23#analyzes">
    <skos:prefLabel xml:lang="en">analyzes</skos:prefLabel>
  </rdf:Description>
  <rdf:Description rdf:about="http://carsten.io/hxl/ns-2012-01-23#analyzes">
    <rdfs:comment xml:lang="en">Links a NeedsAssessment to the Situation it analyzes.</rdfs:comment>
  </rdf:Description>
  <rdf:Description rdf:about="http://carsten.io/hxl/ns-2012-01-23#analyzes">
    <rdfs:domain rdf:resource="http://carsten.io/hxl/ns-2012-01-23#NeedsAssessment"/>
  </rdf:Description>
  <rdf:Description rdf:about="http://carsten.io/hxl/ns-2012-01-23#analyzes">
    <rdfs:range rdf:resource="http://carsten.io/hxl/ns-2012-01-23#Situation"/>
  </rdf:Description>
  <rdf:Description rdf:about="http://carsten.io/hxl/ns-2012-01-23#convers">
    <rdf:type rdf:resource="http://www.w3.org/1999/02/22-rdf-syntax-ns#Property"/>
  </rdf:Description>
  <rdf:Description rdf:about="http://carsten.io/hxl/ns-2012-01-23#convers">
    <rdf:type rdf:resource="http://www.w3.org/2002/07/owl#ObjectProperty"/>
  </rdf:Description>
  <rdf:Description rdf:about="http://carsten.io/hxl/ns-2012-01-23#convers">
    <skos:prefLabel xml:lang="en">covers</skos:prefLabel>
  </rdf:Description>
  <rdf:Description rdf:about="http://carsten.io/hxl/ns-2012-01-23#convers">
    <rdfs:comment xml:lang="en">Used to define the sectors that are covered by a cluster; can be used to re-define clusters by Emergency.</rdfs:comment>
  </rdf:Description>
  <rdf:Description rdf:about="http://carsten.io/hxl/ns-2012-01-23#convers">
    <rdfs:domain rdf:resource="http://carsten.io/hxl/ns-2012-01-23#Cluster"/>
  </rdf:Description>
  <rdf:Description rdf:about="http://carsten.io/hxl/ns-2012-01-23#convers">
    <rdfs:range rdf:resource="http://carsten.io/hxl/ns-2012-01-23#Sector"/>
  </rdf:Description>
  <rdf:Description rdf:about="http://carsten.io/hxl/ns-2012-01-23#hasObjective">
    <rdf:type rdf:resource="http://www.w3.org/1999/02/22-rdf-syntax-ns#Property"/>
  </rdf:Description>
  <rdf:Description rdf:about="http://carsten.io/hxl/ns-2012-01-23#hasObjective">
    <rdf:type rdf:resource="http://www.w3.org/2002/07/owl#ObjectProperty"/>
  </rdf:Description>
  <rdf:Description rdf:about="http://carsten.io/hxl/ns-2012-01-23#hasObjective">
    <skos:prefLabel xml:lang="en">has objective</skos:prefLabel>
  </rdf:Description>
  <rdf:Description rdf:about="http://carsten.io/hxl/ns-2012-01-23#hasObjective">
    <rdfs:comment xml:lang="en">Defines the objectives for an activity or project.</rdfs:comment>
  </rdf:Description>
  <rdf:Description rdf:about="http://carsten.io/hxl/ns-2012-01-23#hasObjective">
    <rdfs:domain rdf:resource="http://carsten.io/hxl/ns-2012-01-23#Activity"/>
  </rdf:Description>
  <rdf:Description rdf:about="http://carsten.io/hxl/ns-2012-01-23#hasObjective">
    <rdfs:range rdf:resource="http://carsten.io/hxl/ns-2012-01-23#Objective"/>
  </rdf:Description>
  <rdf:Description rdf:about="http://carsten.io/hxl/ns-2012-01-23#hasOutput">
    <rdf:type rdf:resource="http://www.w3.org/1999/02/22-rdf-syntax-ns#Property"/>
  </rdf:Description>
  <rdf:Description rdf:about="http://carsten.io/hxl/ns-2012-01-23#hasOutput">
    <rdf:type rdf:resource="http://www.w3.org/2002/07/owl#ObjectProperty"/>
  </rdf:Description>
  <rdf:Description rdf:about="http://carsten.io/hxl/ns-2012-01-23#hasOutput">
    <skos:prefLabel xml:lang="en">has output</skos:prefLabel>
  </rdf:Description>
  <rdf:Description rdf:about="http://carsten.io/hxl/ns-2012-01-23#hasOutput">
    <rdfs:comment xml:lang="en">Defines the output for an activity or project.</rdfs:comment>
  </rdf:Description>
  <rdf:Description rdf:about="http://carsten.io/hxl/ns-2012-01-23#hasOutput">
    <rdfs:domain rdf:resource="http://carsten.io/hxl/ns-2012-01-23#Activity"/>
  </rdf:Description>
  <rdf:Description rdf:about="http://carsten.io/hxl/ns-2012-01-23#hasOutput">
    <rdfs:range rdf:resource="http://carsten.io/hxl/ns-2012-01-23#Output"/>
  </rdf:Description>
  <rdf:Description rdf:about="http://carsten.io/hxl/ns-2012-01-23#hasPriority">
    <rdf:type rdf:resource="http://www.w3.org/1999/02/22-rdf-syntax-ns#Property"/>
  </rdf:Description>
  <rdf:Description rdf:about="http://carsten.io/hxl/ns-2012-01-23#hasPriority">
    <rdf:type rdf:resource="http://www.w3.org/2002/07/owl#ObjectProperty"/>
  </rdf:Description>
  <rdf:Description rdf:about="http://carsten.io/hxl/ns-2012-01-23#hasPriority">
    <skos:prefLabel xml:lang="en">has priority</skos:prefLabel>
  </rdf:Description>
  <rdf:Description rdf:about="http://carsten.io/hxl/ns-2012-01-23#hasPriority">
    <rdfs:comment xml:lang="en">Defines the priority for an activity or project.</rdfs:comment>
  </rdf:Description>
  <rdf:Description rdf:about="http://carsten.io/hxl/ns-2012-01-23#hasPriority">
    <rdfs:domain rdf:resource="http://carsten.io/hxl/ns-2012-01-23#Activity"/>
  </rdf:Description>
  <rdf:Description rdf:about="http://carsten.io/hxl/ns-2012-01-23#hasPriority">
    <rdfs:range rdf:resource="http://carsten.io/hxl/ns-2012-01-23#Priority"/>
  </rdf:Description>
  <rdf:Description rdf:about="http://carsten.io/hxl/ns-2012-01-23#period">
    <rdf:type rdf:resource="http://www.w3.org/1999/02/22-rdf-syntax-ns#Property"/>
  </rdf:Description>
  <rdf:Description rdf:about="http://carsten.io/hxl/ns-2012-01-23#period">
    <rdf:type rdf:resource="http://www.w3.org/2002/07/owl#ObjectProperty"/>
  </rdf:Description>
  <rdf:Description rdf:about="http://carsten.io/hxl/ns-2012-01-23#period">
    <skos:prefLabel xml:lang="en">period</skos:prefLabel>
  </rdf:Description>
  <rdf:Description rdf:about="http://carsten.io/hxl/ns-2012-01-23#period">
    <rdfs:comment xml:lang="en">Defines the reporting period for a report.</rdfs:comment>
  </rdf:Description>
  <rdf:Description rdf:about="http://carsten.io/hxl/ns-2012-01-23#period">
    <rdfs:domain rdf:resource="http://carsten.io/hxl/ns-2012-01-23#Report"/>
  </rdf:Description>
  <rdf:Description rdf:about="http://carsten.io/hxl/ns-2012-01-23#period">
    <rdfs:range rdf:resource="http://carsten.io/hxl/ns-2012-01-23#ReportingPeriod"/>
  </rdf:Description>
  <rdf:Description rdf:about="http://carsten.io/hxl/ns-2012-01-23#inputTo">
    <rdf:type rdf:resource="http://www.w3.org/1999/02/22-rdf-syntax-ns#Property"/>
  </rdf:Description>
  <rdf:Description rdf:about="http://carsten.io/hxl/ns-2012-01-23#inputTo">
    <rdf:type rdf:resource="http://www.w3.org/2002/07/owl#ObjectProperty"/>
  </rdf:Description>
  <rdf:Description rdf:about="http://carsten.io/hxl/ns-2012-01-23#inputTo">
    <skos:prefLabel xml:lang="en">input to</skos:prefLabel>
  </rdf:Description>
  <rdf:Description rdf:about="http://carsten.io/hxl/ns-2012-01-23#inputTo">
    <rdfs:comment xml:lang="en">Specififes that data collection is input to a report.</rdfs:comment>
  </rdf:Description>
  <rdf:Description rdf:about="http://carsten.io/hxl/ns-2012-01-23#inputTo">
    <rdfs:domain rdf:resource="http://carsten.io/hxl/ns-2012-01-23#DataCollection"/>
  </rdf:Description>
  <rdf:Description rdf:about="http://carsten.io/hxl/ns-2012-01-23#inputTo">
    <rdfs:range rdf:resource="http://carsten.io/hxl/ns-2012-01-23#Report"/>
  </rdf:Description>
  <rdf:Description rdf:about="http://carsten.io/hxl/ns-2012-01-23#subject">
    <rdf:type rdf:resource="http://www.w3.org/1999/02/22-rdf-syntax-ns#Property"/>
  </rdf:Description>
  <rdf:Description rdf:about="http://carsten.io/hxl/ns-2012-01-23#subject">
    <rdf:type rdf:resource="http://www.w3.org/2002/07/owl#ObjectProperty"/>
  </rdf:Description>
  <rdf:Description rdf:about="http://carsten.io/hxl/ns-2012-01-23#subject">
    <skos:prefLabel xml:lang="en">subject</skos:prefLabel>
  </rdf:Description>
  <rdf:Description rdf:about="http://carsten.io/hxl/ns-2012-01-23#subject">
    <rdfs:subPropertyOf rdf:resource="http://purl.org/dc/terms/subject"/>
  </rdf:Description>
  <rdf:Description rdf:about="http://carsten.io/hxl/ns-2012-01-23#subject">
    <rdfs:comment xml:lang="en">Specififes the subjects of a report.</rdfs:comment>
  </rdf:Description>
  <rdf:Description rdf:about="http://carsten.io/hxl/ns-2012-01-23#subject">
    <rdfs:domain rdf:resource="http://carsten.io/hxl/ns-2012-01-23#Report"/>
  </rdf:Description>
  <rdf:Description rdf:about="http://carsten.io/hxl/ns-2012-01-23#subject">
    <rdfs:range rdf:resource="http://carsten.io/hxl/ns-2012-01-23#Incident"/>
  </rdf:Description>
  <rdf:Description rdf:about="http://carsten.io/hxl/ns-2012-01-23#subject">
    <rdfs:range rdf:resource="http://carsten.io/hxl/ns-2012-01-23#Damage"/>
  </rdf:Description>
  <rdf:Description rdf:about="http://carsten.io/hxl/ns-2012-01-23#subject">
    <rdfs:range rdf:resource="http://carsten.io/hxl/ns-2012-01-23#Indicator"/>
  </rdf:Description>
  <rdf:Description rdf:about="http://carsten.io/hxl/ns-2012-01-23#subject">
    <rdfs:range rdf:resource="http://carsten.io/hxl/ns-2012-01-23#Budget"/>
  </rdf:Description>
  <rdf:Description rdf:about="http://carsten.io/hxl/ns-2012-01-23#subject">
    <rdfs:range rdf:resource="http://carsten.io/hxl/ns-2012-01-23#Need"/>
  </rdf:Description>
  <rdf:Description rdf:about="http://carsten.io/hxl/ns-2012-01-23#measures">
    <rdf:type rdf:resource="http://www.w3.org/1999/02/22-rdf-syntax-ns#Property"/>
  </rdf:Description>
  <rdf:Description rdf:about="http://carsten.io/hxl/ns-2012-01-23#measures">
    <rdf:type rdf:resource="http://www.w3.org/2002/07/owl#ObjectProperty"/>
  </rdf:Description>
  <rdf:Description rdf:about="http://carsten.io/hxl/ns-2012-01-23#measures">
    <skos:prefLabel xml:lang="en">measures</skos:prefLabel>
  </rdf:Description>
  <rdf:Description rdf:about="http://carsten.io/hxl/ns-2012-01-23#measures">
    <rdfs:subPropertyOf rdf:resource="http://purl.org/dc/terms/subject"/>
  </rdf:Description>
  <rdf:Description rdf:about="http://carsten.io/hxl/ns-2012-01-23#measures">
    <rdfs:comment xml:lang="en">Specififes the need or objective that a certain indicator addresses or measures. &lt;em&gt;Eventually create second property for objectives?&lt;/em&gt;</rdfs:comment>
  </rdf:Description>
  <rdf:Description rdf:about="http://carsten.io/hxl/ns-2012-01-23#measures">
    <rdfs:domain rdf:resource="http://carsten.io/hxl/ns-2012-01-23#Indicator"/>
  </rdf:Description>
  <rdf:Description rdf:about="http://carsten.io/hxl/ns-2012-01-23#measures">
    <rdfs:range rdf:resource="http://carsten.io/hxl/ns-2012-01-23#Objective"/>
  </rdf:Description>
  <rdf:Description rdf:about="http://carsten.io/hxl/ns-2012-01-23#basedOn">
    <rdf:type rdf:resource="http://www.w3.org/1999/02/22-rdf-syntax-ns#Property"/>
  </rdf:Description>
  <rdf:Description rdf:about="http://carsten.io/hxl/ns-2012-01-23#basedOn">
    <rdf:type rdf:resource="http://www.w3.org/2002/07/owl#ObjectProperty"/>
  </rdf:Description>
  <rdf:Description rdf:about="http://carsten.io/hxl/ns-2012-01-23#basedOn">
    <skos:prefLabel xml:lang="en">based on</skos:prefLabel>
  </rdf:Description>
  <rdf:Description rdf:about="http://carsten.io/hxl/ns-2012-01-23#basedOn">
    <rdfs:subPropertyOf rdf:resource="http://purl.org/dc/terms/subject"/>
  </rdf:Description>
  <rdf:Description rdf:about="http://carsten.io/hxl/ns-2012-01-23#basedOn">
    <rdfs:comment xml:lang="en">Specififes that a gap for a certain need has been identified based on a specific indicator.</rdfs:comment>
  </rdf:Description>
  <rdf:Description rdf:about="http://carsten.io/hxl/ns-2012-01-23#basedOn">
    <rdfs:domain rdf:resource="http://carsten.io/hxl/ns-2012-01-23#Need"/>
  </rdf:Description>
  <rdf:Description rdf:about="http://carsten.io/hxl/ns-2012-01-23#basedOn">
    <rdfs:range rdf:resource="http://carsten.io/hxl/ns-2012-01-23#Indicator"/>
  </rdf:Description>
  <rdf:Description rdf:about="http://carsten.io/hxl/ns-2012-01-23#location">
    <rdf:type rdf:resource="http://www.w3.org/1999/02/22-rdf-syntax-ns#Property"/>
  </rdf:Description>
  <rdf:Description rdf:about="http://carsten.io/hxl/ns-2012-01-23#location">
    <rdf:type rdf:resource="http://www.w3.org/2002/07/owl#ObjectProperty"/>
  </rdf:Description>
  <rdf:Description rdf:about="http://carsten.io/hxl/ns-2012-01-23#location">
    <skos:prefLabel xml:lang="en">location</skos:prefLabel>
  </rdf:Description>
  <rdf:Description rdf:about="http://carsten.io/hxl/ns-2012-01-23#location">
    <rdfs:subPropertyOf rdf:resource="http://purl.org/dc/terms/spatial"/>
  </rdf:Description>
  <rdf:Description rdf:about="http://carsten.io/hxl/ns-2012-01-23#location">
    <rdfs:comment xml:lang="en">Specififes the location for things like emergencies, projects, or camps.</rdfs:comment>
  </rdf:Description>
  <rdf:Description rdf:about="http://carsten.io/hxl/ns-2012-01-23#location">
    <rdfs:domain rdf:resource="http://carsten.io/hxl/ns-2012-01-23#Emergency"/>
  </rdf:Description>
  <rdf:Description rdf:about="http://carsten.io/hxl/ns-2012-01-23#location">
    <rdfs:domain rdf:resource="http://carsten.io/hxl/ns-2012-01-23#Site"/>
  </rdf:Description>
  <rdf:Description rdf:about="http://carsten.io/hxl/ns-2012-01-23#location">
    <rdfs:domain rdf:resource="http://carsten.io/hxl/ns-2012-01-23#Incident"/>
  </rdf:Description>
  <rdf:Description rdf:about="http://carsten.io/hxl/ns-2012-01-23#location">
    <rdfs:domain rdf:resource="http://carsten.io/hxl/ns-2012-01-23#Situation"/>
  </rdf:Description>
  <rdf:Description rdf:about="http://carsten.io/hxl/ns-2012-01-23#location">
    <rdfs:range rdf:resource="http://carsten.io/hxl/ns-2012-01-23#Location"/>
  </rdf:Description>
  <rdf:Description rdf:about="http://carsten.io/hxl/ns-2012-01-23#achievedOf">
    <rdf:type rdf:resource="http://www.w3.org/1999/02/22-rdf-syntax-ns#Property"/>
  </rdf:Description>
  <rdf:Description rdf:about="http://carsten.io/hxl/ns-2012-01-23#achievedOf">
    <rdf:type rdf:resource="http://www.w3.org/2002/07/owl#ObjectProperty"/>
  </rdf:Description>
  <rdf:Description rdf:about="http://carsten.io/hxl/ns-2012-01-23#achievedOf">
    <skos:prefLabel xml:lang="en">achieved of</skos:prefLabel>
  </rdf:Description>
  <rdf:Description rdf:about="http://carsten.io/hxl/ns-2012-01-23#achievedOf">
    <rdfs:subPropertyOf rdf:resource="http://carsten.io/hxl/ns-2012-01-23#measures"/>
  </rdf:Description>
  <rdf:Description rdf:about="http://carsten.io/hxl/ns-2012-01-23#achievedOf">
    <rdfs:comment>Relates the need achieved to the need target.</rdfs:comment>
  </rdf:Description>
  <rdf:Description rdf:about="http://carsten.io/hxl/ns-2012-01-23#achievedOf">
    <rdfs:domain rdf:resource="http://carsten.io/hxl/ns-2012-01-23#NeedAchieved"/>
  </rdf:Description>
  <rdf:Description rdf:about="http://carsten.io/hxl/ns-2012-01-23#achievedOf">
    <rdfs:range rdf:resource="http://carsten.io/hxl/ns-2012-01-23#NeedTarget"/>
  </rdf:Description>
  <rdf:Description rdf:about="http://xmlns.com/foaf/0.1/Organization">
    <rdf:type rdf:resource="http://www.w3.org/2000/01/rdf-schema#Class"/>
  </rdf:Description>
  <rdf:Description rdf:about="http://xmlns.com/foaf/0.1/Organization">
    <rdf:type rdf:resource="http://www.w3.org/2002/07/owl#Class"/>
  </rdf:Description>
  <rdf:Description rdf:about="http://xmlns.com/foaf/0.1/Organization">
    <skos:prefLabel>foaf:Organization</skos:prefLabel>
  </rdf:Description>
  <rdf:Description rdf:about="http://xmlns.com/foaf/0.1/Organization">
    <rdfs:subClassOf rdf:resource="http://xmlns.com/foaf/0.1/Agent"/>
  </rdf:Description>
  <rdf:Description rdf:about="http://xmlns.com/foaf/0.1/Group">
    <rdf:type rdf:resource="http://www.w3.org/2000/01/rdf-schema#Class"/>
  </rdf:Description>
  <rdf:Description rdf:about="http://xmlns.com/foaf/0.1/Group">
    <rdf:type rdf:resource="http://www.w3.org/2002/07/owl#Class"/>
  </rdf:Description>
  <rdf:Description rdf:about="http://xmlns.com/foaf/0.1/Group">
    <skos:prefLabel>foaf:Group</skos:prefLabel>
  </rdf:Description>
  <rdf:Description rdf:about="http://xmlns.com/foaf/0.1/Group">
    <rdfs:subClassOf rdf:resource="http://xmlns.com/foaf/0.1/Agent"/>
  </rdf:Description>
</rdf:RDF>
