<?xml version="1.0" encoding="utf-8"?>
<rdf:RDF xmlns:dc="http://purl.org/dc/terms/" xmlns:foaf="http://xmlns.com/foaf/0.1/" xmlns:geo="http://www.opengis.net/geosparql#" xmlns:hxl="http://hxl.humanitarianresponse.info/ns/#" xmlns:label="http://www.wasab.dk/morten/2004/03/label#" xmlns:owl="http://www.w3.org/2002/07/owl#" xmlns:rdf="http://www.w3.org/1999/02/22-rdf-syntax-ns#" xmlns:rdfs="http://www.w3.org/2000/01/rdf-schema#" xmlns:skos="http://www.w3.org/2004/02/skos/core#" xmlns:xsd="http://www.w3.org/2001/XMLSchema#">
  <rdf:Description rdf:about="http://hxl.humanitarianresponse.info/ns/">
    <rdf:type rdf:resource="http://www.w3.org/2002/07/owl#Ontology"/>
  </rdf:Description>
  <rdf:Description rdf:about="http://hxl.humanitarianresponse.info/ns/">
    <dc:date rdf:datatype="http://www.w3.org/2001/XMLSchema#date">2012-11-06</dc:date>
  </rdf:Description>
  <rdf:Description rdf:about="http://hxl.humanitarianresponse.info/ns/">
    <dc:creator rdf:resource="http://hxl.humanitarianresponse.info/data/persons/unocha/carsten_kessler"/>
  </rdf:Description>
  <rdf:Description rdf:about="http://hxl.humanitarianresponse.info/ns/">
    <dc:creator rdf:resource="http://hxl.humanitarianresponse.info/data/persons/unocha/cj_hendrix"/>
  </rdf:Description>
  <rdf:Description rdf:about="http://hxl.humanitarianresponse.info/ns/">
    <dc:creator rdf:resource="http://hxl.humanitarianresponse.info/data/persons/unocha/minu_limbu"/>
  </rdf:Description>
  <rdf:Description rdf:about="http://hxl.humanitarianresponse.info/ns/">
    <dc:title xml:lang="en">Humanitarian eXchange Language (HXL) Situation and Response Standard</dc:title>
  </rdf:Description>
  <rdf:Description rdf:about="http://hxl.humanitarianresponse.info/ns/">
    <dc:abstract xml:lang="en">&lt;p&gt;Draft specification of the Humanitarian eXchange Language (HXL) standard. &lt;span style='color: red'&gt;This vocabulary specification is currently &lt;b&gt;under development&lt;/b&gt; and may change at any time without notice.&lt;/span&gt;&lt;/p&gt; &lt;p&gt;The porpuse of HXL is to facilitate data exchange within the humanitarian domain. It provides a core domain model that has been created bottom-up by inspecting a broad range of systems in use with different humanitarian organisations. As needs vary widely across organisations in this domain, this vocabulary does &lt;em&gt;not&lt;/em&gt; intend to be complete; in fact, it is the smallest common denominator. Any organisations that wish to publish &lt;em&gt;full&lt;/em&gt; exports of their data can do so by extending this domain model with application- or organisation-specific models that reflect their internal data models (which may already be formalised in an XML schema or database schema).&lt;/p&gt;</dc:abstract>
  </rdf:Description>
  <rdf:Description rdf:about="http://hxl.humanitarianresponse.info/ns/">
    <dc:license xml:lang="en">&lt;a href='http://creativecommons.org/licenses/by/3.0/'&gt;&lt;img src='cc.png' align='right' /&gt;&lt;/a&gt;The HXL vocabulary is published under a Creative Commons Attribution license (&lt;a href='http://creativecommons.org/licenses/by/3.0/'&gt;CC BY 3.0&lt;/a&gt;).</dc:license>
  </rdf:Description>
  <rdf:Description rdf:about="http://hxl.humanitarianresponse.info/ns/">
    <rdfs:seeAlso xml:lang="en">For further information about the HXL project, see &lt;a href='https://sites.google.com/site/hxlproject/'&gt;https://sites.google.com/site/hxlproject/&lt;/a&gt;.</rdfs:seeAlso>
  </rdf:Description>
  <rdf:Description rdf:about="http://hxl.humanitarianresponse.info/ns/">
    <dc:replaces rdf:resource="http://hxl.humanitarianresponse.info/ns-2012-10-29/"/>
  </rdf:Description>
  <rdf:Description rdf:about="http://hxl.humanitarianresponse.info/ns/">
    <skos:changeNote>&lt;b&gt;Changes on November 6, 2012:&lt;/b&gt;&lt;ol&gt;&lt;li&gt;&lt;a href='#atLocation'&gt;hxl:atLocation&lt;/a&gt; is a transitive property now to make queries along the administrative unit hierarchy easier.&lt;/li&gt;&lt;/ol&gt;&lt;b&gt;Changes on October 29, 2012:&lt;/b&gt;&lt;ol&gt;&lt;li&gt;Class &lt;a href='#Source'&gt;hxl:Source&lt;/a&gt; added as a superclass for all things that can be sources of information (people, organisations, systems, etc.).&lt;/li&gt;&lt;li&gt;Class &lt;a href='#System'&gt;hxl:System&lt;/a&gt; added as a new subclass hxl:Source. hxl:HXLer and hxl:Organisation are now also subclasses of hxl:Source.&lt;/li&gt;&lt;/ol&gt;&lt;b&gt;Changes on October 9, 2012:&lt;/b&gt;&lt;ol&gt;&lt;li&gt;Class hxl:ReportingPeriod and its hxl:start and hxl:end properties have been removed; use &lt;a href='#validOn'&gt;hxl:validOn&lt;/a&gt; in the future.&lt;/li&gt;&lt;/ol&gt;&lt;b&gt;Changes on September 28, 2012:&lt;/b&gt;&lt;ol&gt;&lt;li&gt;The set of top level concepts has been adjusted for our upcoming demo.&lt;/li&gt;&lt;li&gt;Preferred labels for populations changed to the plural variants.&lt;/li&gt;&lt;li&gt;The different validity properties have been replaced by &lt;a href='#validOn'&gt;hxl:validOn&lt;/a&gt;. This ensures a proper distinction between actual data and their metadata, which have to be attached to the enclosing data container.&lt;/li&gt;&lt;li&gt;The preferred label of &lt;a href='#Population'&gt;hxl:Population&lt;/a&gt; has been changed to Population Group.&lt;/li&gt;&lt;li&gt;Property &lt;a href='#ftsId'&gt;hxl:ftsId&lt;/a&gt; has been added.&lt;/li&gt;&lt;/ol&gt;&lt;b&gt;Changes on September 11, 2012:&lt;/b&gt;&lt;ol&gt;&lt;li&gt;The properties &lt;i&gt;validityStart&lt;/i&gt; and &lt;i&gt;validityEnd&lt;/i&gt; were changed to &lt;a href='http://hxl.humanitarianresponse.info/ns#validFrom'&gt;validFrom&lt;/a&gt; and &lt;a href='http://hxl.humanitarianresponse.info/ns#validUntil'&gt;validUntil&lt;/a&gt;. These formerly had &lt;a href 'http://hxl.humanitarianresponse.info/ns#Baseclass&gt;Baseclass&lt;/a&gt; as their domain, but these have been changed so that they only apply to those classes which need validity dates.&lt;/li&gt;&lt;li&gt;The properties &lt;a href='http://hxl.humanitarianresponse.info/ns#start'&gt;start&lt;/a&gt; and &lt;a href='http://hxl.humanitarianresponse.info/ns#end'&gt;end&lt;/a&gt; have also had their domains changed from &lt;a href 'http://hxl.humanitarianresponse.info/ns#Baseclass'&gt;Baseclass&lt;/a&gt; to those classes which need start and end dates.&lt;/li&gt;&lt;/ol&gt;&lt;b&gt;Changes on September 3, 2012:&lt;/b&gt;&lt;ol&gt;&lt;li&gt;The property &lt;i&gt;currentLocation&lt;/i&gt; has been removed.  Use &lt;a href='#atLocation'&gt;atLocation&lt;/a&gt; instead.&lt;/li&gt;&lt;li&gt;The properties &lt;a href='#featureName'&gt;featureName&lt;/a&gt;, &lt;a href='#featureAltName'&gt;featureAltName&lt;/a&gt;, and &lt;a href='#featureRefName'&gt;featureRefName&lt;/a&gt; have been made subproperties of &lt;a href='#title'&gt;title&lt;/a&gt;.&lt;/li&gt;&lt;li&gt;The property &lt;i&gt;inDisplacedLocationType&lt;/i&gt; has been replaced with &lt;a href='#displacedLocationType'&gt;displacedLocationType&lt;/a&gt; which now is in the domain of &lt;a href='#APL'&gt;Affected Population Location&lt;/a&gt;&lt;/li&gt;&lt;/ol&gt;&lt;b&gt;Changes on August 29, 2012:&lt;/b&gt;&lt;ol&gt;&lt;li&gt;Typo fixed: hxl:AFL replaced by hxl:APL.&lt;/li&gt;&lt;/ol&gt;&lt;b&gt;Changes on August 22, 2012:&lt;/b&gt;&lt;ol&gt;&lt;li&gt;The class &lt;i&gt;Camp&lt;/i&gt; has been renamed to &lt;a href='#APL'&gt;Affected Population Location&lt;/a&gt; to comply with official terminology.&lt;/li&gt;&lt;li&gt;The class &lt;a href='#Country'&gt;Country&lt;/a&gt; is not a subclass of &lt;a href='http://purl.org/ontology/places#Country'&gt;http://purl.org/ontology/places#Country&lt;/a&gt; any more, as the HXL definition of a country is different.&lt;/li&gt;&lt;li&gt;The class GlideNumber has been removed. The property &lt;a href='#hasGLIDEnumber'&gt;hasGLIDEnumber&lt;/a&gt; now links an &lt;a href='#Emergency'&gt;Emergency&lt;/a&gt; directly to the corresponding GLIDE number, represented as a String.&lt;/li&gt;&lt;li&gt;Plural for all classes added.&lt;/li&gt;&lt;/ol&gt;&lt;b&gt;Changes on August 21, 2012:&lt;/b&gt;&lt;ol&gt;&lt;li&gt;&lt;a href='#currentLocation'&gt;currentLocation&lt;/a&gt; is now a subproperty of &lt;a href='#atLocation'&gt;atLocation&lt;/a&gt;.&lt;/li&gt;&lt;li&gt;The subclasses of &lt;a href='#SexCategory'&gt;SexCategory&lt;/a&gt; (male, female, etc.) have been removed. They will be moved to a reference list on the triple store as instances of SexCategory.&lt;/li&gt;&lt;/ol&gt;&lt;b&gt;Changes on August 6, 2012:&lt;/b&gt;&lt;ol&gt;&lt;li&gt;Removed property hxl:inAdminUnit, which was formerly used to make the link between a &lt;a href='#AdminUnit'&gt;hxl:AdminUnit&lt;/a&gt; and its parent in the hierarchy of administrative units.  We now use the more generic &lt;a href='#atLocation'&gt;hxl:atLocation&lt;/a&gt; property (inherited from the HXLBaseClass) for this.&lt;/li&gt;&lt;li&gt;Modified defintion of &lt;a href='#Country'&gt;hxl:Country&lt;/a&gt;.&lt;/li&gt;&lt;li&gt;Modified definitions of &lt;a href='#AgeGroup'&gt;hxl:AgeGroup&lt;/a&gt; and &lt;a href='#DisplacedLocationType'&gt;hxl:DisplacedLocationType&lt;/a&gt; to reflect the requirement that specific instances must have names that do not start with numbers.&lt;/li&gt;&lt;/ol&gt;&lt;b&gt;Changes on August 2, 2012:&lt;/b&gt;&lt;ol&gt;&lt;li&gt;Link to date/time standard document added to &lt;a href='#metadataSection'&gt;Metadata Section&lt;/a&gt;.&lt;/li&gt;&lt;/ol&gt;&lt;b&gt;Changes on July 13, 2012:&lt;/b&gt;&lt;ol&gt;&lt;li&gt;Added more stricht datatypes for all properties that point to numbers (xsd:int) or dates (xsd:date).&lt;/li&gt;&lt;/ol&gt;&lt;b&gt;Changes on July 12, 2012:&lt;/b&gt;&lt;ol&gt;&lt;li&gt;&lt;a href='#atLocation'&gt;atLocation&lt;/a&gt; has been turned into a generic property.&lt;/li&gt;&lt;li&gt;All classes and properties related to admin dataset versions have been deleted. Versioning and validity dates should be handled through data container metadata.&lt;/li&gt;&lt;/ol&gt;&lt;b&gt;Changes on July 11, 2012:&lt;/b&gt;&lt;ol&gt;&lt;li&gt;Plurals added for HXL classes, using the &lt;a href='http://www.wasab.dk/morten/2004/03/label'&gt;label vocabulary&lt;/a&gt;.&lt;/li&gt;&lt;li&gt;&lt;a href='#reportCategory'&gt;reportCategory&lt;/a&gt; has been moved to the metadata section.&lt;/li&gt;&lt;li&gt;For consistency, &lt;em&gt;Sex&lt;/em&gt; has been renamed &lt;a href='#SexCategory'&gt;Sex Category&lt;/a&gt;&lt;/li&gt;&lt;li&gt;Property &lt;a href='#relatedInfo'&gt;relatedInfo&lt;/a&gt; added.&lt;/li&gt;&lt;li&gt;The date and time properties have been moved into the &lt;a href='#metadataSection'&gt;metadata section&lt;/a&gt;&lt;/li&gt;&lt;/ol&gt;&lt;b&gt;Changes on July 5, 2012:&lt;/b&gt;&lt;ol&gt;&lt;li&gt;ReportCategory and ReportCategorySet have been moved to the &lt;a href='#metadataSection'&gt;metadata section&lt;/li&gt;.&lt;/li&gt;&lt;li&gt;Use of RDF containers is now properly documented for all subclasses of rdf:Bag.&lt;/li&gt;&lt;li&gt;Class &lt;a href='#HXLer'&gt;HXLer&lt;/a&gt; has been introduced.&lt;/li&gt;&lt;li&gt;Property &lt;em&gt;yperiod of validity&lt;/em&gt; has been replaced by &lt;a href='#validityStart'&gt;validityStart&lt;/a&gt; and &lt;a href='#validityEnd'&gt;validityEnd&lt;/a&gt;. &lt;/li&gt;&lt;/ol&gt;&lt;b&gt;Changes on July 4, 2012:&lt;/b&gt;&lt;ol&gt;&lt;li&gt;The gelolocation section now contains only those classes and properties that are specific to HXL. They extend the classes and properties (esp. topological relations) introduced by &lt;a href='http://www.opengeospatial.org/standards/geosparql'&gt;OGC's GeoSPARQL standard&lt;/a&gt;.&lt;/li&gt;&lt;li&gt;The documentation now contains all domains and ranges inherited from super-/subclasses for each class.&lt;/li&gt;&lt;li&gt;&lt;a href='#validityDate'&gt;hxl:validityDate&lt;/a&gt; introduced.&lt;/li&gt;&lt;li&gt;Property &lt;a href='#aboutEmergency'&gt;aboutEmergency&lt;/a&gt; introduced to link a DataContainer to the Emergency it contains data about.&lt;/li&gt;&lt;li&gt;All sets in HXL are now subclasses of rdf:Bag, so that we can get rid of our membership functions.&lt;/li&gt;&lt;li&gt;Introduced &lt;a href='#ReportCategory'&gt;ReportCategory&lt;/a&gt;, &lt;a href='#reportCategory'&gt;reportCategory&lt;/a&gt;, and &lt;a href='#ReportCategorySet'&gt;ReportCategorySet&lt;/a&gt; to define the report category for a specific DataContainer and collect the possible ReportCategories for a specific Emergency in a set.&lt;/li&gt;&lt;li&gt;Generic properties &lt;a href='#comment'&gt;comment&lt;/a&gt;, &lt;a href='#title'&gt;title&lt;/a&gt; and &lt;a hre='#description'&gt;description&lt;/a&gt; introduced.&lt;/li&gt;&lt;/ol&gt;&lt;/b&gt;&lt;b&gt;Changes on July 3, 2012:&lt;/b&gt;&lt;ol&gt;&lt;li&gt;Versioning: We will use the URI &lt;a href='http://hxl.humanitarianresponse.info/ns'&gt;http://hxl.humanitarianresponse.info/ns&lt;/a&gt; for all future versions of this vocabulary from now on. Previous versions can be found &lt;a href='http://hxl.humanitarianresponse.info/ns-2012-06-14/'&gt;here&lt;/a&gt;.&lt;/li&gt;&lt;li&gt;&lt;a href='#Country'&gt;hxl:Country&lt;/a&gt; is now a subclass of &lt;a href='http://purl.org/ontology/places#Country'&gt;http://purl.org/ontology/places#Country&lt;/a&gt;&lt;/li&gt;&lt;li&gt;&lt;a href='#Thing'&gt;hxl:BaseClass&lt;/a&gt; has been introduced as an abstract base class. Every other class in HXL is a subclass of hxl:BaseClass. This allows us to define generic properties for all classes in HXL.&lt;/li&gt;&lt;li&gt;Class &lt;em&gt;Activity&lt;/em&gt; has been removed.&lt;/li&gt;&lt;li&gt;Properties &lt;em&gt;containsPrimaryData&lt;/em&gt; and &lt;em&gt;containsSecondaryData&lt;/em&gt; have been removed.&lt;li&gt;Properties &lt;em&gt;displacedLocationSetTitle&lt;/em&gt;, &lt;em&gt;displacedLocationTypeSetDescription&lt;/em&gt;, &lt;em&gt;ageGroupSetDescription&lt;/em&gt;, &lt;em&gt;ageGroupSetTitle&lt;/em&gt;, and &lt;em&gt;populationDescription&lt;/em&gt; have been removed. Use the generic title / description properties instead.&lt;/li&gt;&lt;/ol&gt;</skos:changeNote>
  </rdf:Description>
  <rdf:Description rdf:about="http://hxl.humanitarianresponse.info/ns/#humanitarianProfileSection">
    <rdf:type rdf:resource="http://hxl.humanitarianresponse.info/ns/#vocabularySection"/>
  </rdf:Description>
  <rdf:Description rdf:about="http://hxl.humanitarianresponse.info/ns/#humanitarianProfileSection">
    <rdfs:comment xml:lang="en">This section of the vocabulary defines the humanitarian profile standard which includes classes for describing populations affected by an emergency.</rdfs:comment>
  </rdf:Description>
  <rdf:Description rdf:about="http://hxl.humanitarianresponse.info/ns/#humanitarianProfileSection">
    <dc:title xml:lang="en">Humanitarian Profile Section</dc:title>
  </rdf:Description>
  <rdf:Description rdf:about="http://hxl.humanitarianresponse.info/ns/#geolocationSection">
    <rdf:type rdf:resource="http://hxl.humanitarianresponse.info/ns/#vocabularySection"/>
  </rdf:Description>
  <rdf:Description rdf:about="http://hxl.humanitarianresponse.info/ns/#geolocationSection">
    <rdfs:comment xml:lang="en">This section of the vocabulary defines the geolocation standard. The &lt;a href='hxl-geolocation-standard-draft.pdf'&gt;draft HXL geolocation standard&lt;/a&gt; contains a detailed description of how to use the classes and properties.</rdfs:comment>
  </rdf:Description>
  <rdf:Description rdf:about="http://hxl.humanitarianresponse.info/ns/#geolocationSection">
    <dc:title>Geolocation Section</dc:title>
  </rdf:Description>
  <rdf:Description rdf:about="http://hxl.humanitarianresponse.info/ns/#situationSection">
    <rdf:type rdf:resource="http://hxl.humanitarianresponse.info/ns/#vocabularySection"/>
  </rdf:Description>
  <rdf:Description rdf:about="http://hxl.humanitarianresponse.info/ns/#situationSection">
    <rdfs:comment xml:lang="en">This section of the vocabulary defines the standards for situations and emergencies.</rdfs:comment>
  </rdf:Description>
  <rdf:Description rdf:about="http://hxl.humanitarianresponse.info/ns/#situationSection">
    <dc:title>Situation Section</dc:title>
  </rdf:Description>
  <rdf:Description rdf:about="http://hxl.humanitarianresponse.info/ns/#responseSection">
    <rdf:type rdf:resource="http://hxl.humanitarianresponse.info/ns/#vocabularySection"/>
  </rdf:Description>
  <rdf:Description rdf:about="http://hxl.humanitarianresponse.info/ns/#responseSection">
    <rdfs:comment xml:lang="en">This section of the vocabulary defines the standards for response activities.</rdfs:comment>
  </rdf:Description>
  <rdf:Description rdf:about="http://hxl.humanitarianresponse.info/ns/#responseSection">
    <dc:title>Response Section</dc:title>
  </rdf:Description>
  <rdf:Description rdf:about="http://hxl.humanitarianresponse.info/ns/#metadataSection">
    <rdf:type rdf:resource="http://hxl.humanitarianresponse.info/ns/#vocabularySection"/>
  </rdf:Description>
  <rdf:Description rdf:about="http://hxl.humanitarianresponse.info/ns/#metadataSection">
    <rdfs:comment xml:lang="en">This section of the vocabulary defines the standards for metadata about a set of HXL data that is being exchanged. The &lt;a href='hxl-datetime-standard-draft.pdf'&gt;draft HXL date/time standard&lt;/a&gt; contains a detailed description of how to use the classes and properties related to dates and timestamps.</rdfs:comment>
  </rdf:Description>
  <rdf:Description rdf:about="http://hxl.humanitarianresponse.info/ns/#metadataSection">
    <dc:title>Metadata Section</dc:title>
  </rdf:Description>
  <rdf:Description rdf:about="http://hxl.humanitarianresponse.info/data/persons/unocha/carsten_kessler">
    <rdf:type rdf:resource="http://xmlns.com/foaf/0.1/Person"/>
  </rdf:Description>
  <rdf:Description rdf:about="http://hxl.humanitarianresponse.info/data/persons/unocha/carsten_kessler">
    <foaf:name>Carsten Keßler</foaf:name>
  </rdf:Description>
  <rdf:Description rdf:about="http://hxl.humanitarianresponse.info/data/persons/unocha/carsten_kessler">
    <foaf:mbox>me@carsten.io</foaf:mbox>
  </rdf:Description>
  <rdf:Description rdf:about="http://hxl.humanitarianresponse.info/data/persons/unocha/carsten_kessler">
    <foaf:homepage rdf:resource="http://carsten.io"/>
  </rdf:Description>
  <rdf:Description rdf:about="http://hxl.humanitarianresponse.info/data/persons/unocha/cj_hendrix">
    <rdf:type rdf:resource="http://xmlns.com/foaf/0.1/Person"/>
  </rdf:Description>
  <rdf:Description rdf:about="http://hxl.humanitarianresponse.info/data/persons/unocha/cj_hendrix">
    <foaf:name>CJ Hendrix</foaf:name>
  </rdf:Description>
  <rdf:Description rdf:about="http://hxl.humanitarianresponse.info/data/persons/unocha/cj_hendrix">
    <foaf:mbox>hendrix.cj@gmail.com</foaf:mbox>
  </rdf:Description>
  <rdf:Description rdf:about="http://hxl.humanitarianresponse.info/data/persons/unocha/minu_limbu">
    <rdf:type rdf:resource="http://xmlns.com/foaf/0.1/Person"/>
  </rdf:Description>
  <rdf:Description rdf:about="http://hxl.humanitarianresponse.info/data/persons/unocha/minu_limbu">
    <foaf:name>Minu Limbu</foaf:name>
  </rdf:Description>
  <rdf:Description rdf:about="http://hxl.humanitarianresponse.info/data/persons/unocha/minu_limbu">
    <foaf:mbox>minulimbu@gmail.com</foaf:mbox>
  </rdf:Description>
  <rdf:Description rdf:about="http://hxl.humanitarianresponse.info/ns/#BaseClass">
    <rdf:type rdf:resource="http://www.w3.org/2000/01/rdf-schema#Class"/>
  </rdf:Description>
  <rdf:Description rdf:about="http://hxl.humanitarianresponse.info/ns/#BaseClass">
    <rdfs:comment xml:lang="en">Abstract base class. Any other class in HXL is a subclass of hxl:BaseClass.</rdfs:comment>
  </rdf:Description>
  <rdf:Description rdf:about="http://hxl.humanitarianresponse.info/ns/#Source">
    <rdf:type rdf:resource="http://www.w3.org/2000/01/rdf-schema#Class"/>
  </rdf:Description>
  <rdf:Description rdf:about="http://hxl.humanitarianresponse.info/ns/#Source">
    <rdfs:isDefinedBy rdf:resource="http://hxl.humanitarianresponse.info/ns/#metadataSection"/>
  </rdf:Description>
  <rdf:Description rdf:about="http://hxl.humanitarianresponse.info/ns/#Source">
    <rdfs:subClassOf rdf:resource="http://xmlns.com/foaf/0.1/Agent"/>
  </rdf:Description>
  <rdf:Description rdf:about="http://hxl.humanitarianresponse.info/ns/#Source">
    <rdfs:subClassOf rdf:resource="http://hxl.humanitarianresponse.info/ns/#BaseClass"/>
  </rdf:Description>
  <rdf:Description rdf:about="http://hxl.humanitarianresponse.info/ns/#Source">
    <skos:prefLabel xml:lang="en">Source</skos:prefLabel>
  </rdf:Description>
  <rdf:Description rdf:about="http://hxl.humanitarianresponse.info/ns/#Source">
    <label:plural xml:lang="en">Sources</label:plural>
  </rdf:Description>
  <rdf:Description rdf:about="http://hxl.humanitarianresponse.info/ns/#Source">
    <rdfs:comment xml:lang="en">Superclass for any source of information (HXLer, Organisation, etc.) provided by an HXL datacontainer.</rdfs:comment>
  </rdf:Description>
  <rdf:Description rdf:about="http://hxl.humanitarianresponse.info/ns/#System">
    <rdf:type rdf:resource="http://www.w3.org/2000/01/rdf-schema#Class"/>
  </rdf:Description>
  <rdf:Description rdf:about="http://hxl.humanitarianresponse.info/ns/#System">
    <rdfs:subClassOf rdf:resource="http://hxl.humanitarianresponse.info/ns/#Source"/>
  </rdf:Description>
  <rdf:Description rdf:about="http://hxl.humanitarianresponse.info/ns/#System">
    <rdfs:isDefinedBy rdf:resource="http://hxl.humanitarianresponse.info/ns/#metadataSection"/>
  </rdf:Description>
  <rdf:Description rdf:about="http://hxl.humanitarianresponse.info/ns/#System">
    <skos:prefLabel xml:lang="en">System</skos:prefLabel>
  </rdf:Description>
  <rdf:Description rdf:about="http://hxl.humanitarianresponse.info/ns/#System">
    <label:plural xml:lang="en">Systems</label:plural>
  </rdf:Description>
  <rdf:Description rdf:about="http://hxl.humanitarianresponse.info/ns/#System">
    <rdfs:comment xml:lang="en">A system (e.g. information system, database) providing HXL data.</rdfs:comment>
  </rdf:Description>
  <rdf:Description rdf:about="http://hxl.humanitarianresponse.info/ns/#HXLer">
    <rdf:type rdf:resource="http://www.w3.org/2000/01/rdf-schema#Class"/>
  </rdf:Description>
  <rdf:Description rdf:about="http://hxl.humanitarianresponse.info/ns/#HXLer">
    <rdfs:subClassOf rdf:resource="http://xmlns.com/foaf/0.1/Agent"/>
  </rdf:Description>
  <rdf:Description rdf:about="http://hxl.humanitarianresponse.info/ns/#HXLer">
    <rdfs:subClassOf rdf:resource="http://hxl.humanitarianresponse.info/ns/#BaseClass"/>
  </rdf:Description>
  <rdf:Description rdf:about="http://hxl.humanitarianresponse.info/ns/#HXLer">
    <rdfs:subClassOf rdf:resource="http://hxl.humanitarianresponse.info/ns/#Source"/>
  </rdf:Description>
  <rdf:Description rdf:about="http://hxl.humanitarianresponse.info/ns/#HXLer">
    <rdfs:isDefinedBy rdf:resource="http://hxl.humanitarianresponse.info/ns/#metadataSection"/>
  </rdf:Description>
  <rdf:Description rdf:about="http://hxl.humanitarianresponse.info/ns/#HXLer">
    <skos:prefLabel xml:lang="en">HXLer</skos:prefLabel>
  </rdf:Description>
  <rdf:Description rdf:about="http://hxl.humanitarianresponse.info/ns/#HXLer">
    <label:plural xml:lang="en">HXLers</label:plural>
  </rdf:Description>
  <rdf:Description rdf:about="http://hxl.humanitarianresponse.info/ns/#HXLer">
    <rdfs:comment xml:lang="en">Superclass for any individuals or organizations interacting with HXL.</rdfs:comment>
  </rdf:Description>
  <rdf:Description rdf:about="http://hxl.humanitarianresponse.info/ns/#comment">
    <rdf:type rdf:resource="http://www.w3.org/1999/02/22-rdf-syntax-ns#Property"/>
  </rdf:Description>
  <rdf:Description rdf:about="http://hxl.humanitarianresponse.info/ns/#comment">
    <rdf:type rdf:resource="http://www.w3.org/2002/07/owl#DataProperty"/>
  </rdf:Description>
  <rdf:Description rdf:about="http://hxl.humanitarianresponse.info/ns/#comment">
    <rdfs:subPropertyOf rdf:resource="http://www.w3.org/2000/01/rdf-schema#comment"/>
  </rdf:Description>
  <rdf:Description rdf:about="http://hxl.humanitarianresponse.info/ns/#comment">
    <skos:prefLabel xml:lang="en">comment</skos:prefLabel>
  </rdf:Description>
  <rdf:Description rdf:about="http://hxl.humanitarianresponse.info/ns/#comment">
    <rdfs:isDefinedBy rdf:resource="http://hxl.humanitarianresponse.info/ns/#metadataSection"/>
  </rdf:Description>
  <rdf:Description rdf:about="http://hxl.humanitarianresponse.info/ns/#comment">
    <rdfs:comment xml:lang="en">Generic property for comments.</rdfs:comment>
  </rdf:Description>
  <rdf:Description rdf:about="http://hxl.humanitarianresponse.info/ns/#comment">
    <rdfs:domain rdf:resource="http://hxl.humanitarianresponse.info/ns/#BaseClass"/>
  </rdf:Description>
  <rdf:Description rdf:about="http://hxl.humanitarianresponse.info/ns/#comment">
    <rdfs:range rdf:resource="http://www.w3.org/2000/01/rdf-schema#Literal"/>
  </rdf:Description>
  <rdf:Description rdf:about="http://hxl.humanitarianresponse.info/ns/#title">
    <rdf:type rdf:resource="http://www.w3.org/1999/02/22-rdf-syntax-ns#Property"/>
  </rdf:Description>
  <rdf:Description rdf:about="http://hxl.humanitarianresponse.info/ns/#title">
    <rdf:type rdf:resource="http://www.w3.org/2002/07/owl#DataProperty"/>
  </rdf:Description>
  <rdf:Description rdf:about="http://hxl.humanitarianresponse.info/ns/#title">
    <rdfs:subPropertyOf rdf:resource="http://purl.org/dc/terms/title"/>
  </rdf:Description>
  <rdf:Description rdf:about="http://hxl.humanitarianresponse.info/ns/#title">
    <skos:prefLabel>title</skos:prefLabel>
  </rdf:Description>
  <rdf:Description rdf:about="http://hxl.humanitarianresponse.info/ns/#title">
    <rdfs:isDefinedBy rdf:resource="http://hxl.humanitarianresponse.info/ns/#metadataSection"/>
  </rdf:Description>
  <rdf:Description rdf:about="http://hxl.humanitarianresponse.info/ns/#title">
    <rdfs:comment>Generic property for titles.</rdfs:comment>
  </rdf:Description>
  <rdf:Description rdf:about="http://hxl.humanitarianresponse.info/ns/#title">
    <rdfs:domain rdf:resource="http://hxl.humanitarianresponse.info/ns/#BaseClass"/>
  </rdf:Description>
  <rdf:Description rdf:about="http://hxl.humanitarianresponse.info/ns/#title">
    <rdfs:range rdf:resource="http://www.w3.org/2000/01/rdf-schema#Literal"/>
  </rdf:Description>
  <rdf:Description rdf:about="http://hxl.humanitarianresponse.info/ns/#description">
    <rdf:type rdf:resource="http://www.w3.org/1999/02/22-rdf-syntax-ns#Property"/>
  </rdf:Description>
  <rdf:Description rdf:about="http://hxl.humanitarianresponse.info/ns/#description">
    <rdf:type rdf:resource="http://www.w3.org/2002/07/owl#DataProperty"/>
  </rdf:Description>
  <rdf:Description rdf:about="http://hxl.humanitarianresponse.info/ns/#description">
    <rdfs:subPropertyOf rdf:resource="http://purl.org/dc/terms/description"/>
  </rdf:Description>
  <rdf:Description rdf:about="http://hxl.humanitarianresponse.info/ns/#description">
    <skos:prefLabel>description</skos:prefLabel>
  </rdf:Description>
  <rdf:Description rdf:about="http://hxl.humanitarianresponse.info/ns/#description">
    <rdfs:isDefinedBy rdf:resource="http://hxl.humanitarianresponse.info/ns/#metadataSection"/>
  </rdf:Description>
  <rdf:Description rdf:about="http://hxl.humanitarianresponse.info/ns/#description">
    <rdfs:comment>Generic property for descriptions.</rdfs:comment>
  </rdf:Description>
  <rdf:Description rdf:about="http://hxl.humanitarianresponse.info/ns/#description">
    <rdfs:domain rdf:resource="http://hxl.humanitarianresponse.info/ns/#BaseClass"/>
  </rdf:Description>
  <rdf:Description rdf:about="http://hxl.humanitarianresponse.info/ns/#description">
    <rdfs:range rdf:resource="http://www.w3.org/2000/01/rdf-schema#Literal"/>
  </rdf:Description>
  <rdf:Description rdf:about="http://hxl.humanitarianresponse.info/ns/#Situation">
    <rdf:type rdf:resource="http://www.w3.org/2000/01/rdf-schema#Class"/>
  </rdf:Description>
  <rdf:Description rdf:about="http://hxl.humanitarianresponse.info/ns/#Situation">
    <rdfs:subClassOf rdf:resource="http://hxl.humanitarianresponse.info/ns/#BaseClass"/>
  </rdf:Description>
  <rdf:Description rdf:about="http://hxl.humanitarianresponse.info/ns/#Situation">
    <rdfs:isDefinedBy rdf:resource="http://hxl.humanitarianresponse.info/ns/#situationSection"/>
  </rdf:Description>
  <rdf:Description rdf:about="http://hxl.humanitarianresponse.info/ns/#Situation">
    <skos:prefLabel xml:lang="en">Situation</skos:prefLabel>
  </rdf:Description>
  <rdf:Description rdf:about="http://hxl.humanitarianresponse.info/ns/#Situation">
    <label:plural xml:lang="en">Situations</label:plural>
  </rdf:Description>
  <rdf:Description rdf:about="http://hxl.humanitarianresponse.info/ns/#Situation">
    <rdfs:comment xml:lang="en">Generic situation.</rdfs:comment>
  </rdf:Description>
  <rdf:Description rdf:about="http://hxl.humanitarianresponse.info/ns/#AdminUnit">
    <rdf:type rdf:resource="http://www.w3.org/2000/01/rdf-schema#Class"/>
  </rdf:Description>
  <rdf:Description rdf:about="http://hxl.humanitarianresponse.info/ns/#AdminUnit">
    <rdfs:isDefinedBy rdf:resource="http://hxl.humanitarianresponse.info/ns/#geolocationSection"/>
  </rdf:Description>
  <rdf:Description rdf:about="http://hxl.humanitarianresponse.info/ns/#AdminUnit">
    <skos:prefLabel xml:lang="en">Administrative Unit</skos:prefLabel>
  </rdf:Description>
  <rdf:Description rdf:about="http://hxl.humanitarianresponse.info/ns/#AdminUnit">
    <label:plural xml:lang="en">Administrative Units</label:plural>
  </rdf:Description>
  <rdf:Description rdf:about="http://hxl.humanitarianresponse.info/ns/#AdminUnit">
    <rdfs:subClassOf rdf:resource="http://www.opengis.net/geosparql#Feature"/>
  </rdf:Description>
  <rdf:Description rdf:about="http://hxl.humanitarianresponse.info/ns/#AdminUnit">
    <rdfs:subClassOf rdf:resource="http://hxl.humanitarianresponse.info/ns/#BaseClass"/>
  </rdf:Description>
  <rdf:Description rdf:about="http://hxl.humanitarianresponse.info/ns/#AdminUnit">
    <rdfs:comment xml:lang="en">Administrative units can include coutries, regions, cities, etc. The hierarchy of administrative units can vary from country to country.</rdfs:comment>
  </rdf:Description>
  <rdf:Description rdf:about="http://hxl.humanitarianresponse.info/ns/#PopulatedPlace">
    <rdf:type rdf:resource="http://www.w3.org/2000/01/rdf-schema#Class"/>
  </rdf:Description>
  <rdf:Description rdf:about="http://hxl.humanitarianresponse.info/ns/#PopulatedPlace">
    <rdfs:isDefinedBy rdf:resource="http://hxl.humanitarianresponse.info/ns/#geolocationSection"/>
  </rdf:Description>
  <rdf:Description rdf:about="http://hxl.humanitarianresponse.info/ns/#PopulatedPlace">
    <skos:prefLabel xml:lang="en">Populated Place</skos:prefLabel>
  </rdf:Description>
  <rdf:Description rdf:about="http://hxl.humanitarianresponse.info/ns/#PopulatedPlace">
    <label:plural xml:lang="en">Populated Places</label:plural>
  </rdf:Description>
  <rdf:Description rdf:about="http://hxl.humanitarianresponse.info/ns/#PopulatedPlace">
    <rdfs:subClassOf rdf:resource="http://hxl.humanitarianresponse.info/ns/#AdminUnit"/>
  </rdf:Description>
  <rdf:Description rdf:about="http://hxl.humanitarianresponse.info/ns/#PopulatedPlace">
    <rdfs:comment xml:lang="en">Lowest-level administrative unit, such as a town or settlement.</rdfs:comment>
  </rdf:Description>
  <rdf:Description rdf:about="http://hxl.humanitarianresponse.info/ns/#Country">
    <rdf:type rdf:resource="http://www.w3.org/2000/01/rdf-schema#Class"/>
  </rdf:Description>
  <rdf:Description rdf:about="http://hxl.humanitarianresponse.info/ns/#Country">
    <rdfs:subClassOf rdf:resource="http://hxl.humanitarianresponse.info/ns/#AdminUnit"/>
  </rdf:Description>
  <rdf:Description rdf:about="http://hxl.humanitarianresponse.info/ns/#Country">
    <rdfs:isDefinedBy rdf:resource="http://hxl.humanitarianresponse.info/ns/#geolocationSection"/>
  </rdf:Description>
  <rdf:Description rdf:about="http://hxl.humanitarianresponse.info/ns/#Country">
    <skos:prefLabel xml:lang="en">Country</skos:prefLabel>
  </rdf:Description>
  <rdf:Description rdf:about="http://hxl.humanitarianresponse.info/ns/#Country">
    <label:plural xml:lang="en">Countries</label:plural>
  </rdf:Description>
  <rdf:Description rdf:about="http://hxl.humanitarianresponse.info/ns/#Country">
    <rdfs:comment xml:lang="en">Highest-level administrative unit (level 0). This includes but is not limited to the three-letter country codes defined by ISO 3166-1, which may represent nations, dependent territories, and special areas of geographical interest. Instantiation of a hxl:Country object is for the administrative purposes of the Humanitarian Exchange Language and does not imply endoresement or recognition of any type by anybody.</rdfs:comment>
  </rdf:Description>
  <rdf:Description rdf:about="http://hxl.humanitarianresponse.info/ns/#AdminUnitLevel">
    <rdf:type rdf:resource="http://www.w3.org/2000/01/rdf-schema#Class"/>
  </rdf:Description>
  <rdf:Description rdf:about="http://hxl.humanitarianresponse.info/ns/#AdminUnitLevel">
    <rdfs:subClassOf rdf:resource="http://hxl.humanitarianresponse.info/ns/#BaseClass"/>
  </rdf:Description>
  <rdf:Description rdf:about="http://hxl.humanitarianresponse.info/ns/#AdminUnitLevel">
    <rdfs:isDefinedBy rdf:resource="http://hxl.humanitarianresponse.info/ns/#geolocationSection"/>
  </rdf:Description>
  <rdf:Description rdf:about="http://hxl.humanitarianresponse.info/ns/#AdminUnitLevel">
    <skos:prefLabel xml:lang="en">Administrative Unit Level</skos:prefLabel>
  </rdf:Description>
  <rdf:Description rdf:about="http://hxl.humanitarianresponse.info/ns/#AdminUnitLevel">
    <label:plural xml:lang="en">Administrative Unit Levels</label:plural>
  </rdf:Description>
  <rdf:Description rdf:about="http://hxl.humanitarianresponse.info/ns/#AdminUnitLevel">
    <rdfs:comment xml:lang="en">The specific administrative unit levels can vary from country to country. Administrative Unit Level 0 is a country – in this case, hxl:Country should be used.</rdfs:comment>
  </rdf:Description>
  <rdf:Description rdf:about="http://hxl.humanitarianresponse.info/ns/#AffectedPopulation">
    <rdf:type rdf:resource="http://www.w3.org/2000/01/rdf-schema#Class"/>
  </rdf:Description>
  <rdf:Description rdf:about="http://hxl.humanitarianresponse.info/ns/#AffectedPopulation">
    <rdfs:isDefinedBy rdf:resource="http://hxl.humanitarianresponse.info/ns/#humanitarianProfileSection"/>
  </rdf:Description>
  <rdf:Description rdf:about="http://hxl.humanitarianresponse.info/ns/#AffectedPopulation">
    <skos:prefLabel xml:lang="en">Affected Population</skos:prefLabel>
  </rdf:Description>
  <rdf:Description rdf:about="http://hxl.humanitarianresponse.info/ns/#AffectedPopulation">
    <label:plural xml:lang="en">Affected Populations</label:plural>
  </rdf:Description>
  <rdf:Description rdf:about="http://hxl.humanitarianresponse.info/ns/#AffectedPopulation">
    <rdfs:subClassOf rdf:resource="http://hxl.humanitarianresponse.info/ns/#Population"/>
  </rdf:Description>
  <rdf:Description rdf:about="http://hxl.humanitarianresponse.info/ns/#AffectedPopulation">
    <rdfs:comment xml:lang="en">A population affected by an emergency. &lt;br /&gt;&lt;small&gt;Term origin: Humanitarian Profile (&lt;em&gt;Affected&lt;/em&gt;);&lt;/small&gt;</rdfs:comment>
  </rdf:Description>
  <rdf:Description rdf:about="http://hxl.humanitarianresponse.info/ns/#Population">
    <rdf:type rdf:resource="http://www.w3.org/2000/01/rdf-schema#Class"/>
  </rdf:Description>
  <rdf:Description rdf:about="http://hxl.humanitarianresponse.info/ns/#Population">
    <rdfs:subClassOf rdf:resource="http://hxl.humanitarianresponse.info/ns/#BaseClass"/>
  </rdf:Description>
  <rdf:Description rdf:about="http://hxl.humanitarianresponse.info/ns/#Population">
    <hxl:topLevelConcept rdf:datatype="http://www.w3.org/2001/XMLSchema#boolean">true</hxl:topLevelConcept>
  </rdf:Description>
  <rdf:Description rdf:about="http://hxl.humanitarianresponse.info/ns/#Population">
    <rdfs:isDefinedBy rdf:resource="http://hxl.humanitarianresponse.info/ns/#humanitarianProfileSection"/>
  </rdf:Description>
  <rdf:Description rdf:about="http://hxl.humanitarianresponse.info/ns/#Population">
    <skos:prefLabel xml:lang="en">Population Group</skos:prefLabel>
  </rdf:Description>
  <rdf:Description rdf:about="http://hxl.humanitarianresponse.info/ns/#Population">
    <label:plural xml:lang="en">Population Groups</label:plural>
  </rdf:Description>
  <rdf:Description rdf:about="http://hxl.humanitarianresponse.info/ns/#Population">
    <rdfs:subClassOf rdf:resource="http://xmlns.com/foaf/0.1/Group"/>
  </rdf:Description>
  <rdf:Description rdf:about="http://hxl.humanitarianresponse.info/ns/#Population">
    <rdfs:comment xml:lang="en">Generic class for any kind of population. Example: Total population, affected population, etc.; use the subclasses for the data annotation.</rdfs:comment>
  </rdf:Description>
  <rdf:Description rdf:about="http://hxl.humanitarianresponse.info/ns/#Casualty">
    <rdf:type rdf:resource="http://www.w3.org/2000/01/rdf-schema#Class"/>
  </rdf:Description>
  <rdf:Description rdf:about="http://hxl.humanitarianresponse.info/ns/#Casualty">
    <rdfs:isDefinedBy rdf:resource="http://hxl.humanitarianresponse.info/ns/#humanitarianProfileSection"/>
  </rdf:Description>
  <rdf:Description rdf:about="http://hxl.humanitarianresponse.info/ns/#Casualty">
    <rdfs:subClassOf rdf:resource="http://hxl.humanitarianresponse.info/ns/#AffectedPopulation"/>
  </rdf:Description>
  <rdf:Description rdf:about="http://hxl.humanitarianresponse.info/ns/#Casualty">
    <skos:prefLabel xml:lang="en">Casualties</skos:prefLabel>
  </rdf:Description>
  <rdf:Description rdf:about="http://hxl.humanitarianresponse.info/ns/#Casualty">
    <label:plural xml:lang="en">Casualties</label:plural>
  </rdf:Description>
  <rdf:Description rdf:about="http://hxl.humanitarianresponse.info/ns/#Casualty">
    <rdfs:comment>Examples: &lt;em&gt;Injured&lt;/em&gt; or &lt;em&gt;dead&lt;/em&gt;.&lt;br /&gt;&lt;small&gt;Term origin: ACAPS DSS, Humanitarian Profile.&lt;/small&gt;</rdfs:comment>
  </rdf:Description>
  <rdf:Description rdf:about="http://hxl.humanitarianresponse.info/ns/#Dead">
    <rdf:type rdf:resource="http://www.w3.org/2000/01/rdf-schema#Class"/>
  </rdf:Description>
  <rdf:Description rdf:about="http://hxl.humanitarianresponse.info/ns/#Dead">
    <rdfs:isDefinedBy rdf:resource="http://hxl.humanitarianresponse.info/ns/#humanitarianProfileSection"/>
  </rdf:Description>
  <rdf:Description rdf:about="http://hxl.humanitarianresponse.info/ns/#Dead">
    <skos:prefLabel xml:lang="en">Deaths</skos:prefLabel>
  </rdf:Description>
  <rdf:Description rdf:about="http://hxl.humanitarianresponse.info/ns/#Dead">
    <skos:altLabel xml:lang="en">Dead</skos:altLabel>
  </rdf:Description>
  <rdf:Description rdf:about="http://hxl.humanitarianresponse.info/ns/#Dead">
    <label:plural xml:lang="en">Deaths</label:plural>
  </rdf:Description>
  <rdf:Description rdf:about="http://hxl.humanitarianresponse.info/ns/#Dead">
    <rdfs:subClassOf rdf:resource="http://hxl.humanitarianresponse.info/ns/#Casualty"/>
  </rdf:Description>
  <rdf:Description rdf:about="http://hxl.humanitarianresponse.info/ns/#Dead">
    <owl:disjointWith rdf:resource="http://hxl.humanitarianresponse.info/ns/#Injured"/>
  </rdf:Description>
  <rdf:Description rdf:about="http://hxl.humanitarianresponse.info/ns/#Dead">
    <rdfs:comment>A (reported) death.&lt;br /&gt;&lt;small&gt;Term origin: ACAPS DSS, HPM Ethiopia, Shelter Cluster, Humanitarian Profile (&lt;em&gt;Dead&lt;/em&gt;).&lt;/small&gt;</rdfs:comment>
  </rdf:Description>
  <rdf:Description rdf:about="http://hxl.humanitarianresponse.info/ns/#Displaced">
    <rdf:type rdf:resource="http://www.w3.org/2000/01/rdf-schema#Class"/>
  </rdf:Description>
  <rdf:Description rdf:about="http://hxl.humanitarianresponse.info/ns/#Displaced">
    <rdfs:isDefinedBy rdf:resource="http://hxl.humanitarianresponse.info/ns/#humanitarianProfileSection"/>
  </rdf:Description>
  <rdf:Description rdf:about="http://hxl.humanitarianresponse.info/ns/#Displaced">
    <skos:prefLabel xml:lang="en">Displaced Population</skos:prefLabel>
  </rdf:Description>
  <rdf:Description rdf:about="http://hxl.humanitarianresponse.info/ns/#Displaced">
    <label:plural xml:lang="en">Displaced Populations</label:plural>
  </rdf:Description>
  <rdf:Description rdf:about="http://hxl.humanitarianresponse.info/ns/#Displaced">
    <rdfs:subClassOf rdf:resource="http://hxl.humanitarianresponse.info/ns/#AffectedPopulation"/>
  </rdf:Description>
  <rdf:Description rdf:about="http://hxl.humanitarianresponse.info/ns/#Displaced">
    <rdfs:comment>Refers to internally displaced persons, refugees, and others of concern.&lt;br /&gt;&lt;small&gt;Term origin: Humanitarian Profile, ACAPS DSS (&lt;em&gt;Displacement&lt;/em&gt;)&lt;/small&gt;</rdfs:comment>
  </rdf:Description>
  <rdf:Description rdf:about="http://hxl.humanitarianresponse.info/ns/#Displaced">
    <owl:disjointWith rdf:resource="http://hxl.humanitarianresponse.info/ns/#NonDisplaced"/>
  </rdf:Description>
  <rdf:Description rdf:about="http://hxl.humanitarianresponse.info/ns/#APL">
    <rdf:type rdf:resource="http://www.w3.org/2000/01/rdf-schema#Class"/>
  </rdf:Description>
  <rdf:Description rdf:about="http://hxl.humanitarianresponse.info/ns/#APL">
    <hxl:topLevelConcept rdf:datatype="http://www.w3.org/2001/XMLSchema#boolean">true</hxl:topLevelConcept>
  </rdf:Description>
  <rdf:Description rdf:about="http://hxl.humanitarianresponse.info/ns/#APL">
    <rdfs:subClassOf rdf:resource="http://www.opengis.net/geosparql#Feature"/>
  </rdf:Description>
  <rdf:Description rdf:about="http://hxl.humanitarianresponse.info/ns/#APL">
    <rdfs:subClassOf rdf:resource="http://hxl.humanitarianresponse.info/ns/#BaseClass"/>
  </rdf:Description>
  <rdf:Description rdf:about="http://hxl.humanitarianresponse.info/ns/#APL">
    <rdfs:isDefinedBy rdf:resource="http://hxl.humanitarianresponse.info/ns/#geolocationSection"/>
  </rdf:Description>
  <rdf:Description rdf:about="http://hxl.humanitarianresponse.info/ns/#APL">
    <skos:prefLabel xml:lang="en">Affected Population Location</skos:prefLabel>
  </rdf:Description>
  <rdf:Description rdf:about="http://hxl.humanitarianresponse.info/ns/#APL">
    <label:plural xml:lang="en">Affected Population Locations</label:plural>
  </rdf:Description>
  <rdf:Description rdf:about="http://hxl.humanitarianresponse.info/ns/#APL">
    <rdfs:comment xml:lang="en">A site providing shelter for an affected population, such as refugees.</rdfs:comment>
  </rdf:Description>
  <rdf:Description rdf:about="http://hxl.humanitarianresponse.info/ns/#Need">
    <rdf:type rdf:resource="http://www.w3.org/2000/01/rdf-schema#Class"/>
  </rdf:Description>
  <rdf:Description rdf:about="http://hxl.humanitarianresponse.info/ns/#Need">
    <hxl:topLevelConcept rdf:datatype="http://www.w3.org/2001/XMLSchema#boolean">true</hxl:topLevelConcept>
  </rdf:Description>
  <rdf:Description rdf:about="http://hxl.humanitarianresponse.info/ns/#Need">
    <rdfs:subClassOf rdf:resource="http://hxl.humanitarianresponse.info/ns/#BaseClass"/>
  </rdf:Description>
  <rdf:Description rdf:about="http://hxl.humanitarianresponse.info/ns/#Need">
    <skos:prefLabel xml:lang="en">Need</skos:prefLabel>
  </rdf:Description>
  <rdf:Description rdf:about="http://hxl.humanitarianresponse.info/ns/#Need">
    <label:plural xml:lang="en">Needs</label:plural>
  </rdf:Description>
  <rdf:Description rdf:about="http://hxl.humanitarianresponse.info/ns/#Need">
    <rdfs:comment xml:lang="en">Needs of an affected population.&lt;br /&gt;&lt;small&gt;For demo purposes only.&lt;/small&gt;</rdfs:comment>
  </rdf:Description>
  <rdf:Description rdf:about="http://hxl.humanitarianresponse.info/ns/#Distribution">
    <rdf:type rdf:resource="http://www.w3.org/2000/01/rdf-schema#Class"/>
  </rdf:Description>
  <rdf:Description rdf:about="http://hxl.humanitarianresponse.info/ns/#Distribution">
    <hxl:topLevelConcept rdf:datatype="http://www.w3.org/2001/XMLSchema#boolean">true</hxl:topLevelConcept>
  </rdf:Description>
  <rdf:Description rdf:about="http://hxl.humanitarianresponse.info/ns/#Distribution">
    <rdfs:subClassOf rdf:resource="http://hxl.humanitarianresponse.info/ns/#BaseClass"/>
  </rdf:Description>
  <rdf:Description rdf:about="http://hxl.humanitarianresponse.info/ns/#Distribution">
    <skos:prefLabel xml:lang="en">Distribution</skos:prefLabel>
  </rdf:Description>
  <rdf:Description rdf:about="http://hxl.humanitarianresponse.info/ns/#Distribution">
    <label:plural xml:lang="en">Distributions</label:plural>
  </rdf:Description>
  <rdf:Description rdf:about="http://hxl.humanitarianresponse.info/ns/#Distribution">
    <rdfs:comment xml:lang="en">A distribution as part of response activities.&lt;br /&gt;&lt;small&gt;For demo purposes only.&lt;/small&gt;</rdfs:comment>
  </rdf:Description>
  <rdf:Description rdf:about="http://hxl.humanitarianresponse.info/ns/#Incident">
    <rdf:type rdf:resource="http://www.w3.org/2000/01/rdf-schema#Class"/>
  </rdf:Description>
  <rdf:Description rdf:about="http://hxl.humanitarianresponse.info/ns/#Incident">
    <hxl:topLevelConcept rdf:datatype="http://www.w3.org/2001/XMLSchema#boolean">true</hxl:topLevelConcept>
  </rdf:Description>
  <rdf:Description rdf:about="http://hxl.humanitarianresponse.info/ns/#Incident">
    <rdfs:subClassOf rdf:resource="http://hxl.humanitarianresponse.info/ns/#BaseClass"/>
  </rdf:Description>
  <rdf:Description rdf:about="http://hxl.humanitarianresponse.info/ns/#Incident">
    <skos:prefLabel xml:lang="en">Incident</skos:prefLabel>
  </rdf:Description>
  <rdf:Description rdf:about="http://hxl.humanitarianresponse.info/ns/#Incident">
    <label:plural xml:lang="en">Incidents</label:plural>
  </rdf:Description>
  <rdf:Description rdf:about="http://hxl.humanitarianresponse.info/ns/#Incident">
    <rdfs:comment xml:lang="en">Examples: Natural disaster, outbreak of an armed conflict, outbreak of a disease in an APL, etc.&lt;br /&gt;&lt;small&gt;For demo purposes only.&lt;/small&gt;</rdfs:comment>
  </rdf:Description>
  <rdf:Description rdf:about="http://hxl.humanitarianresponse.info/ns/#placeOfOrigin">
    <rdf:type rdf:resource="http://www.w3.org/1999/02/22-rdf-syntax-ns#Property"/>
  </rdf:Description>
  <rdf:Description rdf:about="http://hxl.humanitarianresponse.info/ns/#placeOfOrigin">
    <rdf:type rdf:resource="http://www.w3.org/2002/07/owl#ObjectProperty"/>
  </rdf:Description>
  <rdf:Description rdf:about="http://hxl.humanitarianresponse.info/ns/#placeOfOrigin">
    <rdfs:isDefinedBy rdf:resource="http://hxl.humanitarianresponse.info/ns/#humanitarianProfileSection"/>
  </rdf:Description>
  <rdf:Description rdf:about="http://hxl.humanitarianresponse.info/ns/#placeOfOrigin">
    <skos:prefLabel xml:lang="en">place of origin</skos:prefLabel>
  </rdf:Description>
  <rdf:Description rdf:about="http://hxl.humanitarianresponse.info/ns/#placeOfOrigin">
    <rdfs:domain rdf:resource="http://hxl.humanitarianresponse.info/ns/#Displaced"/>
  </rdf:Description>
  <rdf:Description rdf:about="http://hxl.humanitarianresponse.info/ns/#placeOfOrigin">
    <rdfs:range rdf:resource="http://www.opengis.net/geosparql#Feature"/>
  </rdf:Description>
  <rdf:Description rdf:about="http://hxl.humanitarianresponse.info/ns/#placeOfOrigin">
    <rdfs:comment>This attribute only applies to Displaced and its subclasses. It should include p-coded location from which the population being reported moved as a result of the emergency.&lt;br /&gt;&lt;small&gt;Term origin: Humanitarian profile.&lt;/small&gt;</rdfs:comment>
  </rdf:Description>
  <rdf:Description rdf:about="http://hxl.humanitarianresponse.info/ns/#placeOfOriginOf">
    <owl:inverseOf rdf:resource="http://hxl.humanitarianresponse.info/ns/#placeOfOrigin"/>
  </rdf:Description>
  <rdf:Description rdf:about="http://hxl.humanitarianresponse.info/ns/#nationality">
    <rdf:type rdf:resource="http://www.w3.org/1999/02/22-rdf-syntax-ns#Property"/>
  </rdf:Description>
  <rdf:Description rdf:about="http://hxl.humanitarianresponse.info/ns/#nationality">
    <rdf:type rdf:resource="http://www.w3.org/2002/07/owl#ObjectProperty"/>
  </rdf:Description>
  <rdf:Description rdf:about="http://hxl.humanitarianresponse.info/ns/#nationality">
    <rdfs:isDefinedBy rdf:resource="http://hxl.humanitarianresponse.info/ns/#humanitarianProfileSection"/>
  </rdf:Description>
  <rdf:Description rdf:about="http://hxl.humanitarianresponse.info/ns/#nationality">
    <skos:prefLabel xml:lang="en">nationality</skos:prefLabel>
  </rdf:Description>
  <rdf:Description rdf:about="http://hxl.humanitarianresponse.info/ns/#nationality">
    <rdfs:domain rdf:resource="http://hxl.humanitarianresponse.info/ns/#Population"/>
  </rdf:Description>
  <rdf:Description rdf:about="http://hxl.humanitarianresponse.info/ns/#nationality">
    <rdfs:range rdf:resource="http://hxl.humanitarianresponse.info/ns/#Country"/>
  </rdf:Description>
  <rdf:Description rdf:about="http://hxl.humanitarianresponse.info/ns/#nationality">
    <rdfs:comment>This item generally only applies to populations displaced across international borders and contains the nationality of the population being reported.&lt;br /&gt;&lt;small&gt;Term origin: Humanitarian profile.&lt;/small&gt;</rdfs:comment>
  </rdf:Description>
  <rdf:Description rdf:about="http://hxl.humanitarianresponse.info/ns/#nationalityOf">
    <owl:inverseOf rdf:resource="http://hxl.humanitarianresponse.info/ns/#nationality"/>
  </rdf:Description>
  <rdf:Description rdf:about="http://hxl.humanitarianresponse.info/ns/#NonDisplaced">
    <rdf:type rdf:resource="http://www.w3.org/2000/01/rdf-schema#Class"/>
  </rdf:Description>
  <rdf:Description rdf:about="http://hxl.humanitarianresponse.info/ns/#NonDisplaced">
    <rdfs:isDefinedBy rdf:resource="http://hxl.humanitarianresponse.info/ns/#humanitarianProfileSection"/>
  </rdf:Description>
  <rdf:Description rdf:about="http://hxl.humanitarianresponse.info/ns/#NonDisplaced">
    <skos:prefLabel xml:lang="en">Non-Displaced Population</skos:prefLabel>
  </rdf:Description>
  <rdf:Description rdf:about="http://hxl.humanitarianresponse.info/ns/#NonDisplaced">
    <label:plural xml:lang="en">Non-Displaced Populations</label:plural>
  </rdf:Description>
  <rdf:Description rdf:about="http://hxl.humanitarianresponse.info/ns/#NonDisplaced">
    <rdfs:subClassOf rdf:resource="http://hxl.humanitarianresponse.info/ns/#AffectedPopulation"/>
  </rdf:Description>
  <rdf:Description rdf:about="http://hxl.humanitarianresponse.info/ns/#NonDisplaced">
    <rdfs:comment>Refers to the part of the affected population that is not displaced (i.e., host or non-host);.&lt;br /&gt;&lt;small&gt;Term origin: Humanitarian Profile.&lt;/small&gt;</rdfs:comment>
  </rdf:Description>
  <rdf:Description rdf:about="http://hxl.humanitarianresponse.info/ns/#NonDisplaced">
    <owl:disjointWith rdf:resource="http://hxl.humanitarianresponse.info/ns/#Displaced"/>
  </rdf:Description>
  <rdf:Description rdf:about="http://hxl.humanitarianresponse.info/ns/#HostPopulation">
    <rdf:type rdf:resource="http://www.w3.org/2000/01/rdf-schema#Class"/>
  </rdf:Description>
  <rdf:Description rdf:about="http://hxl.humanitarianresponse.info/ns/#HostPopulation">
    <rdfs:isDefinedBy rdf:resource="http://hxl.humanitarianresponse.info/ns/#humanitarianProfileSection"/>
  </rdf:Description>
  <rdf:Description rdf:about="http://hxl.humanitarianresponse.info/ns/#HostPopulation">
    <skos:prefLabel xml:lang="en">Host Population</skos:prefLabel>
  </rdf:Description>
  <rdf:Description rdf:about="http://hxl.humanitarianresponse.info/ns/#HostPopulation">
    <label:plural xml:lang="en">Host Populations</label:plural>
  </rdf:Description>
  <rdf:Description rdf:about="http://hxl.humanitarianresponse.info/ns/#HostPopulation">
    <rdfs:subClassOf rdf:resource="http://hxl.humanitarianresponse.info/ns/#NonDisplaced"/>
  </rdf:Description>
  <rdf:Description rdf:about="http://hxl.humanitarianresponse.info/ns/#HostPopulation">
    <rdfs:comment>Persons who are part of a host community or family receiving affected people. Due to the stress placed on the host families and communities, they are considered part of the humanitarian caseload.&lt;br /&gt;&lt;small&gt;Term origin: Humanitarian Profile.&lt;/small&gt;</rdfs:comment>
  </rdf:Description>
  <rdf:Description rdf:about="http://hxl.humanitarianresponse.info/ns/#HostPopulation">
    <owl:disjointWith rdf:resource="http://hxl.humanitarianresponse.info/ns/#NonHostPopulation"/>
  </rdf:Description>
  <rdf:Description rdf:about="http://hxl.humanitarianresponse.info/ns/#NonHostPopulation">
    <rdf:type rdf:resource="http://www.w3.org/2000/01/rdf-schema#Class"/>
  </rdf:Description>
  <rdf:Description rdf:about="http://hxl.humanitarianresponse.info/ns/#NonHostPopulation">
    <rdfs:isDefinedBy rdf:resource="http://hxl.humanitarianresponse.info/ns/#humanitarianProfileSection"/>
  </rdf:Description>
  <rdf:Description rdf:about="http://hxl.humanitarianresponse.info/ns/#NonHostPopulation">
    <skos:prefLabel xml:lang="en">Non-host Population</skos:prefLabel>
  </rdf:Description>
  <rdf:Description rdf:about="http://hxl.humanitarianresponse.info/ns/#NonHostPopulation">
    <label:plural xml:lang="en">Non-host Populations</label:plural>
  </rdf:Description>
  <rdf:Description rdf:about="http://hxl.humanitarianresponse.info/ns/#NonHostPopulation">
    <rdfs:subClassOf rdf:resource="http://hxl.humanitarianresponse.info/ns/#NonDisplaced"/>
  </rdf:Description>
  <rdf:Description rdf:about="http://hxl.humanitarianresponse.info/ns/#NonHostPopulation">
    <rdfs:comment>People requiring immediate assistance during a period of emergency who have not moved from their homes or places of habitual residence.&lt;br /&gt;&lt;small&gt;Term origin: Humanitarian Profile.&lt;/small&gt;</rdfs:comment>
  </rdf:Description>
  <rdf:Description rdf:about="http://hxl.humanitarianresponse.info/ns/#NonHostPopulation">
    <owl:disjointWith rdf:resource="http://hxl.humanitarianresponse.info/ns/#HostPopulation"/>
  </rdf:Description>
  <rdf:Description rdf:about="http://hxl.humanitarianresponse.info/ns/#Emergency">
    <rdf:type rdf:resource="http://www.w3.org/2000/01/rdf-schema#Class"/>
  </rdf:Description>
  <rdf:Description rdf:about="http://hxl.humanitarianresponse.info/ns/#Emergency">
    <rdfs:isDefinedBy rdf:resource="http://hxl.humanitarianresponse.info/ns/#situationSection"/>
  </rdf:Description>
  <rdf:Description rdf:about="http://hxl.humanitarianresponse.info/ns/#Emergency">
    <skos:prefLabel xml:lang="en">Emergency</skos:prefLabel>
  </rdf:Description>
  <rdf:Description rdf:about="http://hxl.humanitarianresponse.info/ns/#Emergency">
    <label:plural xml:lang="en">Emergencies</label:plural>
  </rdf:Description>
  <rdf:Description rdf:about="http://hxl.humanitarianresponse.info/ns/#Emergency">
    <rdfs:subClassOf rdf:resource="http://hxl.humanitarianresponse.info/ns/#Situation"/>
  </rdf:Description>
  <rdf:Description rdf:about="http://hxl.humanitarianresponse.info/ns/#Emergency">
    <rdfs:comment>&lt;p&gt;Any situation in which life or well-being will be threatened  unless immediate  and  appropriate   action  is  taken,  and  which demands   an   extraordinary   response   and   exceptional measures (from UNHCR Handbook for Emergencies).&lt;/p&gt;&lt;!-- &lt;p&gt;A sudden crisis situation or event requiring immediate action (WART) &lt;/p&gt;&lt;p&gt;Any situation in which there is an exceptional and widespread threat to life, health or basic  subsistence,  that  is  beyond  the  coping  capacity  of individuals and the community  (Oxfam GB Emergency Response Manual). &lt;/p&gt;&lt;p&gt;Where and when a disaster provokes an immediate, exceptional and widespread threat to life, health or basic subsistence, which overwhelms the coping capacity of individual and community, implying need of external assistance” (source: ACFIN Emergency module)&lt;/p&gt; --&gt;&lt;small&gt;Term origin: CAP OPS, Pakistan SRF, ACAPS DSS, CERF, MIRA.&lt;/small&gt;</rdfs:comment>
  </rdf:Description>
  <rdf:Description rdf:about="http://hxl.humanitarianresponse.info/ns/#SexCategory">
    <rdf:type rdf:resource="http://www.w3.org/2000/01/rdf-schema#Class"/>
  </rdf:Description>
  <rdf:Description rdf:about="http://hxl.humanitarianresponse.info/ns/#SexCategory">
    <rdfs:subClassOf rdf:resource="http://hxl.humanitarianresponse.info/ns/#BaseClass"/>
  </rdf:Description>
  <rdf:Description rdf:about="http://hxl.humanitarianresponse.info/ns/#SexCategory">
    <rdfs:isDefinedBy rdf:resource="http://hxl.humanitarianresponse.info/ns/#humanitarianProfileSection"/>
  </rdf:Description>
  <rdf:Description rdf:about="http://hxl.humanitarianresponse.info/ns/#SexCategory">
    <skos:prefLabel xml:lang="en">Sex Category</skos:prefLabel>
  </rdf:Description>
  <rdf:Description rdf:about="http://hxl.humanitarianresponse.info/ns/#SexCategory">
    <label:plural xml:lang="en">Sex Categories</label:plural>
  </rdf:Description>
  <rdf:Description rdf:about="http://hxl.humanitarianresponse.info/ns/#SexCategory">
    <rdfs:comment>Class to describe sex-specific issues, either at individual or group level.&lt;br /&gt;&lt;small&gt;Term origin: MIRA, CCDI&lt;/small&gt;</rdfs:comment>
  </rdf:Description>
  <rdf:Description rdf:about="http://hxl.humanitarianresponse.info/ns/#Response">
    <rdf:type rdf:resource="http://www.w3.org/2000/01/rdf-schema#Class"/>
  </rdf:Description>
  <rdf:Description rdf:about="http://hxl.humanitarianresponse.info/ns/#Response">
    <rdfs:subClassOf rdf:resource="http://hxl.humanitarianresponse.info/ns/#BaseClass"/>
  </rdf:Description>
  <rdf:Description rdf:about="http://hxl.humanitarianresponse.info/ns/#Response">
    <rdfs:isDefinedBy rdf:resource="http://hxl.humanitarianresponse.info/ns/#responseSection"/>
  </rdf:Description>
  <rdf:Description rdf:about="http://hxl.humanitarianresponse.info/ns/#Response">
    <skos:prefLabel xml:lang="en">Response</skos:prefLabel>
  </rdf:Description>
  <rdf:Description rdf:about="http://hxl.humanitarianresponse.info/ns/#Response">
    <skos:prefLabel xml:lang="en">Responses</skos:prefLabel>
  </rdf:Description>
  <rdf:Description rdf:about="http://hxl.humanitarianresponse.info/ns/#Response">
    <rdfs:comment>Generic term for the collection of all activities that address the needs arising from an emergency.&lt;br /&gt;&lt;small&gt;Term origin: ACAPS DSS, ACAPS DSS, MIRA, EDXL, CCDI (&lt;em&gt;Humanitarian Response&lt;/em&gt;), CERF (&lt;em&gt;Humanitarian Response&lt;/em&gt;)&lt;/small&gt;</rdfs:comment>
  </rdf:Description>
  <rdf:Description rdf:about="http://hxl.humanitarianresponse.info/ns/#IDP">
    <rdf:type rdf:resource="http://www.w3.org/2000/01/rdf-schema#Class"/>
  </rdf:Description>
  <rdf:Description rdf:about="http://hxl.humanitarianresponse.info/ns/#IDP">
    <rdfs:isDefinedBy rdf:resource="http://hxl.humanitarianresponse.info/ns/#humanitarianProfileSection"/>
  </rdf:Description>
  <rdf:Description rdf:about="http://hxl.humanitarianresponse.info/ns/#IDP">
    <rdfs:subClassOf rdf:resource="http://hxl.humanitarianresponse.info/ns/#Displaced"/>
  </rdf:Description>
  <rdf:Description rdf:about="http://hxl.humanitarianresponse.info/ns/#IDP">
    <skos:prefLabel xml:lang="en">Internally Displaced Population</skos:prefLabel>
  </rdf:Description>
  <rdf:Description rdf:about="http://hxl.humanitarianresponse.info/ns/#IDP">
    <label:plural xml:lang="en">Internally Displaced Populations</label:plural>
  </rdf:Description>
  <rdf:Description rdf:about="http://hxl.humanitarianresponse.info/ns/#IDP">
    <skos:altLabel xml:lang="en">IDP</skos:altLabel>
  </rdf:Description>
  <rdf:Description rdf:about="http://hxl.humanitarianresponse.info/ns/#IDP">
    <owl:disjointWith rdf:resource="http://hxl.humanitarianresponse.info/ns/#Others"/>
  </rdf:Description>
  <rdf:Description rdf:about="http://hxl.humanitarianresponse.info/ns/#IDP">
    <owl:disjointWith rdf:resource="http://hxl.humanitarianresponse.info/ns/#RefugeesAsylumSeekers"/>
  </rdf:Description>
  <rdf:Description rdf:about="http://hxl.humanitarianresponse.info/ns/#IDP">
    <rdfs:comment>A group of internally displaced persons (IDPs).&lt;br /&gt;&lt;small&gt;Term origin: Humanitarian Profile, CERF, HPM Ethiopia&lt;/small&gt;</rdfs:comment>
  </rdf:Description>
  <rdf:Description rdf:about="http://hxl.humanitarianresponse.info/ns/#Others">
    <rdf:type rdf:resource="http://www.w3.org/2000/01/rdf-schema#Class"/>
  </rdf:Description>
  <rdf:Description rdf:about="http://hxl.humanitarianresponse.info/ns/#Others">
    <rdfs:isDefinedBy rdf:resource="http://hxl.humanitarianresponse.info/ns/#humanitarianProfileSection"/>
  </rdf:Description>
  <rdf:Description rdf:about="http://hxl.humanitarianresponse.info/ns/#Others">
    <rdfs:subClassOf rdf:resource="http://hxl.humanitarianresponse.info/ns/#Displaced"/>
  </rdf:Description>
  <rdf:Description rdf:about="http://hxl.humanitarianresponse.info/ns/#Others">
    <skos:prefLabel xml:lang="en">Others of Concern</skos:prefLabel>
  </rdf:Description>
  <rdf:Description rdf:about="http://hxl.humanitarianresponse.info/ns/#Others">
    <label:plural xml:lang="en">Others of Concern</label:plural>
  </rdf:Description>
  <rdf:Description rdf:about="http://hxl.humanitarianresponse.info/ns/#Others">
    <owl:disjointWith rdf:resource="http://hxl.humanitarianresponse.info/ns/#IDP"/>
  </rdf:Description>
  <rdf:Description rdf:about="http://hxl.humanitarianresponse.info/ns/#Others">
    <owl:disjointWith rdf:resource="http://hxl.humanitarianresponse.info/ns/#RefugeesAsylumSeekers"/>
  </rdf:Description>
  <rdf:Description rdf:about="http://hxl.humanitarianresponse.info/ns/#Others">
    <rdfs:comment>Persons who have been displaced by the emergency and form part of the humanitarian caseload, but do not fall into the IDP or refugees/asylum seekers categories.&lt;br /&gt;&lt;small&gt;Term origin: Humanitarian Profile&lt;/small&gt;</rdfs:comment>
  </rdf:Description>
  <rdf:Description rdf:about="http://hxl.humanitarianresponse.info/ns/#RefugeesAsylumSeekers">
    <rdf:type rdf:resource="http://www.w3.org/2000/01/rdf-schema#Class"/>
  </rdf:Description>
  <rdf:Description rdf:about="http://hxl.humanitarianresponse.info/ns/#RefugeesAsylumSeekers">
    <rdfs:isDefinedBy rdf:resource="http://hxl.humanitarianresponse.info/ns/#humanitarianProfileSection"/>
  </rdf:Description>
  <rdf:Description rdf:about="http://hxl.humanitarianresponse.info/ns/#RefugeesAsylumSeekers">
    <rdfs:subClassOf rdf:resource="http://hxl.humanitarianresponse.info/ns/#Displaced"/>
  </rdf:Description>
  <rdf:Description rdf:about="http://hxl.humanitarianresponse.info/ns/#RefugeesAsylumSeekers">
    <skos:prefLabel xml:lang="en">Refugees and Asylum Seekers</skos:prefLabel>
  </rdf:Description>
  <rdf:Description rdf:about="http://hxl.humanitarianresponse.info/ns/#RefugeesAsylumSeekers">
    <label:plural xml:lang="en">Refugees and Asylum Seekers</label:plural>
  </rdf:Description>
  <rdf:Description rdf:about="http://hxl.humanitarianresponse.info/ns/#RefugeesAsylumSeekers">
    <owl:disjointWith rdf:resource="http://hxl.humanitarianresponse.info/ns/#IDP"/>
  </rdf:Description>
  <rdf:Description rdf:about="http://hxl.humanitarianresponse.info/ns/#RefugeesAsylumSeekers">
    <owl:disjointWith rdf:resource="http://hxl.humanitarianresponse.info/ns/#Others"/>
  </rdf:Description>
  <rdf:Description rdf:about="http://hxl.humanitarianresponse.info/ns/#RefugeesAsylumSeekers">
    <rdfs:comment>A group of refugees and asylum seekers.&lt;br /&gt;&lt;small&gt;Term origin: Humanitarian Profile&lt;/small&gt;</rdfs:comment>
  </rdf:Description>
  <rdf:Description rdf:about="http://hxl.humanitarianresponse.info/ns/#Injured">
    <rdf:type rdf:resource="http://www.w3.org/2000/01/rdf-schema#Class"/>
  </rdf:Description>
  <rdf:Description rdf:about="http://hxl.humanitarianresponse.info/ns/#Injured">
    <rdfs:isDefinedBy rdf:resource="http://hxl.humanitarianresponse.info/ns/#humanitarianProfileSection"/>
  </rdf:Description>
  <rdf:Description rdf:about="http://hxl.humanitarianresponse.info/ns/#Injured">
    <rdfs:subClassOf rdf:resource="http://hxl.humanitarianresponse.info/ns/#Casualty"/>
  </rdf:Description>
  <rdf:Description rdf:about="http://hxl.humanitarianresponse.info/ns/#Injured">
    <skos:prefLabel xml:lang="en">Injured</skos:prefLabel>
  </rdf:Description>
  <rdf:Description rdf:about="http://hxl.humanitarianresponse.info/ns/#Injured">
    <label:plural xml:lang="en">Injured</label:plural>
  </rdf:Description>
  <rdf:Description rdf:about="http://hxl.humanitarianresponse.info/ns/#Injured">
    <owl:disjointWith rdf:resource="http://hxl.humanitarianresponse.info/ns/#Dead"/>
  </rdf:Description>
  <rdf:Description rdf:about="http://hxl.humanitarianresponse.info/ns/#Injured">
    <rdfs:comment>Indicates the Injured population.&lt;br /&gt;&lt;small&gt;Term origin: ACAPS DSS, Humanitarian Profile, Shelter Cluster, HERAMS Checklist (&lt;em&gt;Injury&lt;/em&gt;)&lt;/small&gt;</rdfs:comment>
  </rdf:Description>
  <rdf:Description rdf:about="http://hxl.humanitarianresponse.info/ns/#Missing">
    <rdf:type rdf:resource="http://www.w3.org/2000/01/rdf-schema#Class"/>
  </rdf:Description>
  <rdf:Description rdf:about="http://hxl.humanitarianresponse.info/ns/#Missing">
    <rdfs:isDefinedBy rdf:resource="http://hxl.humanitarianresponse.info/ns/#humanitarianProfileSection"/>
  </rdf:Description>
  <rdf:Description rdf:about="http://hxl.humanitarianresponse.info/ns/#Missing">
    <skos:prefLabel xml:lang="en">Missing</skos:prefLabel>
  </rdf:Description>
  <rdf:Description rdf:about="http://hxl.humanitarianresponse.info/ns/#Missing">
    <label:plural xml:lang="en">Missing</label:plural>
  </rdf:Description>
  <rdf:Description rdf:about="http://hxl.humanitarianresponse.info/ns/#Missing">
    <rdfs:subClassOf rdf:resource="http://hxl.humanitarianresponse.info/ns/#Casualty"/>
  </rdf:Description>
  <rdf:Description rdf:about="http://hxl.humanitarianresponse.info/ns/#Missing">
    <owl:disjointWith rdf:resource="http://hxl.humanitarianresponse.info/ns/#Dead"/>
  </rdf:Description>
  <rdf:Description rdf:about="http://hxl.humanitarianresponse.info/ns/#Missing">
    <rdfs:comment>Associated with &lt;i&gt;Missing Persons&lt;/i&gt; as a major humanitarian concern in complex emergencies where many people go missing, causing anguish and uncertainty for their families and friends. See &lt;em&gt; ICRC &lt;/em&gt;. &lt;br /&gt;&lt;small&gt;Term origin: Humanitarian Profile.&lt;/small&gt;</rdfs:comment>
  </rdf:Description>
  <rdf:Description rdf:about="http://hxl.humanitarianresponse.info/ns/#Organisation">
    <rdf:type rdf:resource="http://www.w3.org/2000/01/rdf-schema#Class"/>
  </rdf:Description>
  <rdf:Description rdf:about="http://hxl.humanitarianresponse.info/ns/#Organisation">
    <rdfs:isDefinedBy rdf:resource="http://hxl.humanitarianresponse.info/ns/#responseSection"/>
  </rdf:Description>
  <rdf:Description rdf:about="http://hxl.humanitarianresponse.info/ns/#Organisation">
    <rdfs:subClassOf rdf:resource="http://xmlns.com/foaf/0.1/Organisation"/>
  </rdf:Description>
  <rdf:Description rdf:about="http://hxl.humanitarianresponse.info/ns/#Organisation">
    <rdfs:subClassOf rdf:resource="http://hxl.humanitarianresponse.info/ns/#BaseClass"/>
  </rdf:Description>
  <rdf:Description rdf:about="http://hxl.humanitarianresponse.info/ns/#Organisation">
    <rdfs:subClassOf rdf:resource="http://hxl.humanitarianresponse.info/ns/#Source"/>
  </rdf:Description>
  <rdf:Description rdf:about="http://hxl.humanitarianresponse.info/ns/#Organisation">
    <skos:prefLabel xml:lang="en">Organisation</skos:prefLabel>
  </rdf:Description>
  <rdf:Description rdf:about="http://hxl.humanitarianresponse.info/ns/#Organisation">
    <label:plural xml:lang="en">Organisations</label:plural>
  </rdf:Description>
  <rdf:Description rdf:about="http://hxl.humanitarianresponse.info/ns/#Organisation">
    <rdfs:comment>A humanitarian organisation.&lt;br /&gt;&lt;small&gt;Term origin: IATI, CAP OPS, Pakistan SRF, EIMS Report, Shelter Cluster, Sigmah DB.&lt;/small&gt;</rdfs:comment>
  </rdf:Description>
  <rdf:Description rdf:about="http://hxl.humanitarianresponse.info/ns/#TotalPopulation">
    <rdf:type rdf:resource="http://www.w3.org/2000/01/rdf-schema#Class"/>
  </rdf:Description>
  <rdf:Description rdf:about="http://hxl.humanitarianresponse.info/ns/#TotalPopulation">
    <rdfs:isDefinedBy rdf:resource="http://hxl.humanitarianresponse.info/ns/#humanitarianProfileSection"/>
  </rdf:Description>
  <rdf:Description rdf:about="http://hxl.humanitarianresponse.info/ns/#TotalPopulation">
    <rdfs:subClassOf rdf:resource="http://hxl.humanitarianresponse.info/ns/#Population"/>
  </rdf:Description>
  <rdf:Description rdf:about="http://hxl.humanitarianresponse.info/ns/#TotalPopulation">
    <skos:prefLabel xml:lang="en">Total Population</skos:prefLabel>
  </rdf:Description>
  <rdf:Description rdf:about="http://hxl.humanitarianresponse.info/ns/#TotalPopulation">
    <label:plural xml:lang="en">Total Populations</label:plural>
  </rdf:Description>
  <rdf:Description rdf:about="http://hxl.humanitarianresponse.info/ns/#TotalPopulation">
    <rdfs:comment>The total population for an administrative unit. Example: A region.&lt;br /&gt;&lt;small&gt;Term origin: Shelter Cluster.&lt;/small&gt;</rdfs:comment>
  </rdf:Description>
  <rdf:Description rdf:about="http://hxl.humanitarianresponse.info/ns/#DataContainer">
    <rdf:type rdf:resource="http://www.w3.org/2000/01/rdf-schema#Class"/>
  </rdf:Description>
  <rdf:Description rdf:about="http://hxl.humanitarianresponse.info/ns/#DataContainer">
    <rdfs:subClassOf rdf:resource="http://hxl.humanitarianresponse.info/ns/#BaseClass"/>
  </rdf:Description>
  <rdf:Description rdf:about="http://hxl.humanitarianresponse.info/ns/#DataContainer">
    <rdfs:isDefinedBy rdf:resource="http://hxl.humanitarianresponse.info/ns/#metadataSection"/>
  </rdf:Description>
  <rdf:Description rdf:about="http://hxl.humanitarianresponse.info/ns/#DataContainer">
    <skos:prefLabel xml:lang="en">Data Container</skos:prefLabel>
  </rdf:Description>
  <rdf:Description rdf:about="http://hxl.humanitarianresponse.info/ns/#DataContainer">
    <label:plural xml:lang="en">Data Containers</label:plural>
  </rdf:Description>
  <rdf:Description rdf:about="http://hxl.humanitarianresponse.info/ns/#DataContainer">
    <rdfs:comment>This is the &lt;em&gt;container&lt;/em&gt; element to attach any metadata to. Any HXL file has to include exactly one data container element and make all metadata statements about this container. When loading the file into the triple store, a new named graph will be created that inherits the metadata from this container.</rdfs:comment>
  </rdf:Description>
  <rdf:Description rdf:about="http://hxl.humanitarianresponse.info/ns/#relatedInfo">
    <rdf:type rdf:resource="http://www.w3.org/1999/02/22-rdf-syntax-ns#Property"/>
  </rdf:Description>
  <rdf:Description rdf:about="http://hxl.humanitarianresponse.info/ns/#relatedInfo">
    <rdf:type rdf:resource="http://www.w3.org/2002/07/owl#ObjectProperty"/>
  </rdf:Description>
  <rdf:Description rdf:about="http://hxl.humanitarianresponse.info/ns/#relatedInfo">
    <rdfs:isDefinedBy rdf:resource="http://hxl.humanitarianresponse.info/ns/#metadataSection"/>
  </rdf:Description>
  <rdf:Description rdf:about="http://hxl.humanitarianresponse.info/ns/#relatedInfo">
    <skos:prefLabel>related information</skos:prefLabel>
  </rdf:Description>
  <rdf:Description rdf:about="http://hxl.humanitarianresponse.info/ns/#relatedInfo">
    <rdfs:comment>Provides a link to a website with further information related to the data in the data container.</rdfs:comment>
  </rdf:Description>
  <rdf:Description rdf:about="http://hxl.humanitarianresponse.info/ns/#relatedInfo">
    <rdfs:domain rdf:resource="http://hxl.humanitarianresponse.info/ns/#DataContainer"/>
  </rdf:Description>
  <rdf:Description rdf:about="http://hxl.humanitarianresponse.info/ns/#relatedInfo">
    <rdfs:range rdf:resource="http://xmlns.com/foaf/0.1/Document"/>
  </rdf:Description>
  <rdf:Description rdf:about="http://hxl.humanitarianresponse.info/ns/#ApprovalLevel">
    <rdf:type rdf:resource="http://www.w3.org/2000/01/rdf-schema#Class"/>
  </rdf:Description>
  <rdf:Description rdf:about="http://hxl.humanitarianresponse.info/ns/#ApprovalLevel">
    <rdfs:subClassOf rdf:resource="http://hxl.humanitarianresponse.info/ns/#BaseClass"/>
  </rdf:Description>
  <rdf:Description rdf:about="http://hxl.humanitarianresponse.info/ns/#ApprovalLevel">
    <rdfs:isDefinedBy rdf:resource="http://hxl.humanitarianresponse.info/ns/#metadataSection"/>
  </rdf:Description>
  <rdf:Description rdf:about="http://hxl.humanitarianresponse.info/ns/#ApprovalLevel">
    <skos:prefLabel xml:lang="en">Approval Level</skos:prefLabel>
  </rdf:Description>
  <rdf:Description rdf:about="http://hxl.humanitarianresponse.info/ns/#ApprovalLevel">
    <label:plural xml:lang="en">Approval Levels</label:plural>
  </rdf:Description>
  <rdf:Description rdf:about="http://hxl.humanitarianresponse.info/ns/#ApprovalLevel">
    <rdfs:comment>Instances of this class define fixed levels of approval in the HXL data repository.</rdfs:comment>
  </rdf:Description>
  <rdf:Description rdf:about="http://hxl.humanitarianresponse.info/ns/#organisationHomepage">
    <rdf:type rdf:resource="http://www.w3.org/1999/02/22-rdf-syntax-ns#Property"/>
  </rdf:Description>
  <rdf:Description rdf:about="http://hxl.humanitarianresponse.info/ns/#organisationHomepage">
    <rdf:type rdf:resource="http://www.w3.org/2002/07/owl#ObjectProperty"/>
  </rdf:Description>
  <rdf:Description rdf:about="http://hxl.humanitarianresponse.info/ns/#organisationHomepage">
    <rdfs:isDefinedBy rdf:resource="http://hxl.humanitarianresponse.info/ns/#responseSection"/>
  </rdf:Description>
  <rdf:Description rdf:about="http://hxl.humanitarianresponse.info/ns/#organisationHomepage">
    <skos:prefLabel>organisation homepage</skos:prefLabel>
  </rdf:Description>
  <rdf:Description rdf:about="http://hxl.humanitarianresponse.info/ns/#organisationHomepage">
    <rdfs:subPropertyOf rdf:resource="http://xmlns.com/foaf/0.1/homepage"/>
  </rdf:Description>
  <rdf:Description rdf:about="http://hxl.humanitarianresponse.info/ns/#organisationHomepage">
    <rdfs:comment>States the website of a given organisation. &lt;small&gt;Term origin: FTS.&lt;/small&gt;</rdfs:comment>
  </rdf:Description>
  <rdf:Description rdf:about="http://hxl.humanitarianresponse.info/ns/#organisationHomepage">
    <rdfs:domain rdf:resource="http://hxl.humanitarianresponse.info/ns/#Organisation"/>
  </rdf:Description>
  <rdf:Description rdf:about="http://hxl.humanitarianresponse.info/ns/#organisationHomepage">
    <rdfs:range rdf:resource="http://xmlns.com/foaf/0.1/Document"/>
  </rdf:Description>
  <rdf:Description rdf:about="http://hxl.humanitarianresponse.info/ns/#organisationHomepageOf">
    <owl:inverseOf rdf:resource="http://hxl.humanitarianresponse.info/ns/#organisationHomepage"/>
  </rdf:Description>
  <rdf:Description rdf:about="http://hxl.humanitarianresponse.info/ns/#ftsId">
    <rdf:type rdf:resource="http://www.w3.org/1999/02/22-rdf-syntax-ns#Property"/>
  </rdf:Description>
  <rdf:Description rdf:about="http://hxl.humanitarianresponse.info/ns/#ftsId">
    <rdf:type rdf:resource="http://www.w3.org/2002/07/owl#DataProperty"/>
  </rdf:Description>
  <rdf:Description rdf:about="http://hxl.humanitarianresponse.info/ns/#ftsId">
    <rdfs:isDefinedBy rdf:resource="http://hxl.humanitarianresponse.info/ns/#responseSection"/>
  </rdf:Description>
  <rdf:Description rdf:about="http://hxl.humanitarianresponse.info/ns/#ftsId">
    <skos:prefLabel>FTS ID</skos:prefLabel>
  </rdf:Description>
  <rdf:Description rdf:about="http://hxl.humanitarianresponse.info/ns/#ftsId">
    <rdfs:comment>States the ID of the organisation in OCHA's Financial Tracking Service (FTS).</rdfs:comment>
  </rdf:Description>
  <rdf:Description rdf:about="http://hxl.humanitarianresponse.info/ns/#ftsId">
    <rdfs:domain rdf:resource="http://hxl.humanitarianresponse.info/ns/#Organisation"/>
  </rdf:Description>
  <rdf:Description rdf:about="http://hxl.humanitarianresponse.info/ns/#ftsId">
    <rdfs:range rdf:resource="http://www.w3.org/2000/01/rdf-schema#Literal"/>
  </rdf:Description>
  <rdf:Description rdf:about="http://hxl.humanitarianresponse.info/ns/#orgName">
    <rdf:type rdf:resource="http://www.w3.org/1999/02/22-rdf-syntax-ns#Property"/>
  </rdf:Description>
  <rdf:Description rdf:about="http://hxl.humanitarianresponse.info/ns/#orgName">
    <rdf:type rdf:resource="http://www.w3.org/2002/07/owl#DataProperty"/>
  </rdf:Description>
  <rdf:Description rdf:about="http://hxl.humanitarianresponse.info/ns/#orgName">
    <rdfs:isDefinedBy rdf:resource="http://hxl.humanitarianresponse.info/ns/#responseSection"/>
  </rdf:Description>
  <rdf:Description rdf:about="http://hxl.humanitarianresponse.info/ns/#orgName">
    <skos:prefLabel>organisation name</skos:prefLabel>
  </rdf:Description>
  <rdf:Description rdf:about="http://hxl.humanitarianresponse.info/ns/#orgName">
    <rdfs:comment>States the name of the organisation. &lt;small&gt;Term origin: FTS.&lt;/small&gt;</rdfs:comment>
  </rdf:Description>
  <rdf:Description rdf:about="http://hxl.humanitarianresponse.info/ns/#orgName">
    <rdfs:domain rdf:resource="http://hxl.humanitarianresponse.info/ns/#Organisation"/>
  </rdf:Description>
  <rdf:Description rdf:about="http://hxl.humanitarianresponse.info/ns/#orgName">
    <rdfs:range rdf:resource="http://www.w3.org/2000/01/rdf-schema#Literal"/>
  </rdf:Description>
  <rdf:Description rdf:about="http://hxl.humanitarianresponse.info/ns/#abbreviation">
    <rdf:type rdf:resource="http://www.w3.org/1999/02/22-rdf-syntax-ns#Property"/>
  </rdf:Description>
  <rdf:Description rdf:about="http://hxl.humanitarianresponse.info/ns/#abbreviation">
    <rdf:type rdf:resource="http://www.w3.org/2002/07/owl#DataProperty"/>
  </rdf:Description>
  <rdf:Description rdf:about="http://hxl.humanitarianresponse.info/ns/#abbreviation">
    <rdfs:isDefinedBy rdf:resource="http://hxl.humanitarianresponse.info/ns/#responseSection"/>
  </rdf:Description>
  <rdf:Description rdf:about="http://hxl.humanitarianresponse.info/ns/#abbreviation">
    <skos:prefLabel>organisation abbreviation</skos:prefLabel>
  </rdf:Description>
  <rdf:Description rdf:about="http://hxl.humanitarianresponse.info/ns/#abbreviation">
    <rdfs:comment>Indicates the abbreviation of the Organisation. &lt;small&gt;Term origin: FTS.&lt;/small&gt;</rdfs:comment>
  </rdf:Description>
  <rdf:Description rdf:about="http://hxl.humanitarianresponse.info/ns/#abbreviation">
    <rdfs:domain rdf:resource="http://hxl.humanitarianresponse.info/ns/#Organisation"/>
  </rdf:Description>
  <rdf:Description rdf:about="http://hxl.humanitarianresponse.info/ns/#abbreviation">
    <rdfs:range rdf:resource="http://www.w3.org/2000/01/rdf-schema#Literal"/>
  </rdf:Description>
  <rdf:Description rdf:about="http://hxl.humanitarianresponse.info/ns/#orgNativeName">
    <rdf:type rdf:resource="http://www.w3.org/1999/02/22-rdf-syntax-ns#Property"/>
  </rdf:Description>
  <rdf:Description rdf:about="http://hxl.humanitarianresponse.info/ns/#orgNativeName">
    <rdf:type rdf:resource="http://www.w3.org/2002/07/owl#DataProperty"/>
  </rdf:Description>
  <rdf:Description rdf:about="http://hxl.humanitarianresponse.info/ns/#orgNativeName">
    <rdfs:isDefinedBy rdf:resource="http://hxl.humanitarianresponse.info/ns/#responseSection"/>
  </rdf:Description>
  <rdf:Description rdf:about="http://hxl.humanitarianresponse.info/ns/#orgNativeName">
    <skos:prefLabel>native organisation name</skos:prefLabel>
  </rdf:Description>
  <rdf:Description rdf:about="http://hxl.humanitarianresponse.info/ns/#orgNativeName">
    <rdfs:comment>Specifies the native name of the organisation. &lt;small&gt;Term origin: FTS.&lt;/small&gt;</rdfs:comment>
  </rdf:Description>
  <rdf:Description rdf:about="http://hxl.humanitarianresponse.info/ns/#orgNativeName">
    <rdfs:domain rdf:resource="http://hxl.humanitarianresponse.info/ns/#Organisation"/>
  </rdf:Description>
  <rdf:Description rdf:about="http://hxl.humanitarianresponse.info/ns/#orgNativeName">
    <rdfs:range rdf:resource="http://www.w3.org/2000/01/rdf-schema#Literal"/>
  </rdf:Description>
  <rdf:Description rdf:about="http://hxl.humanitarianresponse.info/ns/#orgDisplayName">
    <rdf:type rdf:resource="http://www.w3.org/1999/02/22-rdf-syntax-ns#Property"/>
  </rdf:Description>
  <rdf:Description rdf:about="http://hxl.humanitarianresponse.info/ns/#orgDisplayName">
    <rdf:type rdf:resource="http://www.w3.org/2002/07/owl#DataProperty"/>
  </rdf:Description>
  <rdf:Description rdf:about="http://hxl.humanitarianresponse.info/ns/#orgDisplayName">
    <rdfs:isDefinedBy rdf:resource="http://hxl.humanitarianresponse.info/ns/#responseSection"/>
  </rdf:Description>
  <rdf:Description rdf:about="http://hxl.humanitarianresponse.info/ns/#orgDisplayName">
    <skos:prefLabel>organisation name for display</skos:prefLabel>
  </rdf:Description>
  <rdf:Description rdf:about="http://hxl.humanitarianresponse.info/ns/#orgDisplayName">
    <rdfs:comment>Indicates the organisation name that is most commonly used and displayed.  &lt;small&gt;Term origin: FTS.&lt;/small&gt;</rdfs:comment>
  </rdf:Description>
  <rdf:Description rdf:about="http://hxl.humanitarianresponse.info/ns/#orgDisplayName">
    <rdfs:domain rdf:resource="http://hxl.humanitarianresponse.info/ns/#Organisation"/>
  </rdf:Description>
  <rdf:Description rdf:about="http://hxl.humanitarianresponse.info/ns/#orgDisplayName">
    <rdfs:range rdf:resource="http://www.w3.org/2000/01/rdf-schema#Literal"/>
  </rdf:Description>
  <rdf:Description rdf:about="http://hxl.humanitarianresponse.info/ns/#reportedBy">
    <rdf:type rdf:resource="http://www.w3.org/1999/02/22-rdf-syntax-ns#Property"/>
  </rdf:Description>
  <rdf:Description rdf:about="http://hxl.humanitarianresponse.info/ns/#reportedBy">
    <rdf:type rdf:resource="http://www.w3.org/2002/07/owl#ObjectProperty"/>
  </rdf:Description>
  <rdf:Description rdf:about="http://hxl.humanitarianresponse.info/ns/#reportedBy">
    <rdfs:isDefinedBy rdf:resource="http://hxl.humanitarianresponse.info/ns/#metadataSection"/>
  </rdf:Description>
  <rdf:Description rdf:about="http://hxl.humanitarianresponse.info/ns/#reportedBy">
    <skos:prefLabel xml:lang="en">reported by</skos:prefLabel>
  </rdf:Description>
  <rdf:Description rdf:about="http://hxl.humanitarianresponse.info/ns/#reportedBy">
    <rdfs:comment xml:lang="en">The reporting person or organization - not necessarily involved in the aid activity itself, though in practice it often will be a donor or appealing agency.  &lt;br /&gt;&lt;small&gt;Term origin: IATI.&lt;/small&gt;</rdfs:comment>
  </rdf:Description>
  <rdf:Description rdf:about="http://hxl.humanitarianresponse.info/ns/#reportedBy">
    <rdfs:domain rdf:resource="http://hxl.humanitarianresponse.info/ns/#DataContainer"/>
  </rdf:Description>
  <rdf:Description rdf:about="http://hxl.humanitarianresponse.info/ns/#reportedBy">
    <rdfs:range rdf:resource="http://hxl.humanitarianresponse.info/ns/#HXLer"/>
  </rdf:Description>
  <rdf:Description rdf:about="http://hxl.humanitarianresponse.info/ns/#reporting">
    <owl:inverseOf rdf:resource="http://hxl.humanitarianresponse.info/ns/#reportedBy"/>
  </rdf:Description>
  <rdf:Description rdf:about="http://hxl.humanitarianresponse.info/ns/#aboutEmergency">
    <rdf:type rdf:resource="http://www.w3.org/1999/02/22-rdf-syntax-ns#Property"/>
  </rdf:Description>
  <rdf:Description rdf:about="http://hxl.humanitarianresponse.info/ns/#aboutEmergency">
    <rdf:type rdf:resource="http://www.w3.org/2002/07/owl#ObjectProperty"/>
  </rdf:Description>
  <rdf:Description rdf:about="http://hxl.humanitarianresponse.info/ns/#aboutEmergency">
    <rdfs:isDefinedBy rdf:resource="http://hxl.humanitarianresponse.info/ns/#metadataSection"/>
  </rdf:Description>
  <rdf:Description rdf:about="http://hxl.humanitarianresponse.info/ns/#aboutEmergency">
    <skos:prefLabel xml:lang="en">about emergency</skos:prefLabel>
  </rdf:Description>
  <rdf:Description rdf:about="http://hxl.humanitarianresponse.info/ns/#aboutEmergency">
    <rdfs:comment xml:lang="en">Links a DataContainer to the corresponding Emergency it contains data about.</rdfs:comment>
  </rdf:Description>
  <rdf:Description rdf:about="http://hxl.humanitarianresponse.info/ns/#aboutEmergency">
    <rdfs:domain rdf:resource="http://hxl.humanitarianresponse.info/ns/#DataContainer"/>
  </rdf:Description>
  <rdf:Description rdf:about="http://hxl.humanitarianresponse.info/ns/#aboutEmergency">
    <rdfs:range rdf:resource="http://hxl.humanitarianresponse.info/ns/#Emergency"/>
  </rdf:Description>
  <rdf:Description rdf:about="http://hxl.humanitarianresponse.info/ns/#hasDataContainer">
    <owl:inverseOf rdf:resource="http://hxl.humanitarianresponse.info/ns/#aboutEmergency"/>
  </rdf:Description>
  <rdf:Description rdf:about="http://hxl.humanitarianresponse.info/ns/#approvedBy">
    <rdf:type rdf:resource="http://www.w3.org/1999/02/22-rdf-syntax-ns#Property"/>
  </rdf:Description>
  <rdf:Description rdf:about="http://hxl.humanitarianresponse.info/ns/#approvedBy">
    <rdf:type rdf:resource="http://www.w3.org/2002/07/owl#ObjectProperty"/>
  </rdf:Description>
  <rdf:Description rdf:about="http://hxl.humanitarianresponse.info/ns/#approvedBy">
    <rdfs:isDefinedBy rdf:resource="http://hxl.humanitarianresponse.info/ns/#metadataSection"/>
  </rdf:Description>
  <rdf:Description rdf:about="http://hxl.humanitarianresponse.info/ns/#approvedBy">
    <skos:prefLabel xml:lang="en">approved by</skos:prefLabel>
  </rdf:Description>
  <rdf:Description rdf:about="http://hxl.humanitarianresponse.info/ns/#approvedBy">
    <rdfs:comment xml:lang="en">Link from a container to the person or organisation who has 'lifted' it to the current approvalLevel.</rdfs:comment>
  </rdf:Description>
  <rdf:Description rdf:about="http://hxl.humanitarianresponse.info/ns/#approvedBy">
    <rdfs:domain rdf:resource="http://hxl.humanitarianresponse.info/ns/#DataContainer"/>
  </rdf:Description>
  <rdf:Description rdf:about="http://hxl.humanitarianresponse.info/ns/#approvedBy">
    <rdfs:range rdf:resource="http://hxl.humanitarianresponse.info/ns/#HXLer"/>
  </rdf:Description>
  <rdf:Description rdf:about="http://hxl.humanitarianresponse.info/ns/#approves">
    <owl:inverseOf rdf:resource="http://hxl.humanitarianresponse.info/ns/#approvedBy"/>
  </rdf:Description>
  <rdf:Description rdf:about="http://hxl.humanitarianresponse.info/ns/#approvedAtLevel">
    <rdf:type rdf:resource="http://www.w3.org/1999/02/22-rdf-syntax-ns#Property"/>
  </rdf:Description>
  <rdf:Description rdf:about="http://hxl.humanitarianresponse.info/ns/#approvedAtLevel">
    <rdf:type rdf:resource="http://www.w3.org/2002/07/owl#ObjectProperty"/>
  </rdf:Description>
  <rdf:Description rdf:about="http://hxl.humanitarianresponse.info/ns/#approvedAtLevel">
    <rdfs:isDefinedBy rdf:resource="http://hxl.humanitarianresponse.info/ns/#metadataSection"/>
  </rdf:Description>
  <rdf:Description rdf:about="http://hxl.humanitarianresponse.info/ns/#approvedAtLevel">
    <skos:prefLabel xml:lang="en">approved at level</skos:prefLabel>
  </rdf:Description>
  <rdf:Description rdf:about="http://hxl.humanitarianresponse.info/ns/#approvedAtLevel">
    <rdfs:comment xml:lang="en">A container can have approval at different levels, which may in turn indicate for which kind of analyses the data in this container is fit.&lt;/em&gt;</rdfs:comment>
  </rdf:Description>
  <rdf:Description rdf:about="http://hxl.humanitarianresponse.info/ns/#approvedAtLevel">
    <rdfs:domain rdf:resource="http://hxl.humanitarianresponse.info/ns/#DataContainer"/>
  </rdf:Description>
  <rdf:Description rdf:about="http://hxl.humanitarianresponse.info/ns/#approvedAtLevel">
    <rdfs:range rdf:resource="http://hxl.humanitarianresponse.info/ns/#ApprovalLevel"/>
  </rdf:Description>
  <rdf:Description rdf:about="http://hxl.humanitarianresponse.info/ns/#approvalLevelOf">
    <owl:inverseOf rdf:resource="http://hxl.humanitarianresponse.info/ns/#approvedAtLevel"/>
  </rdf:Description>
  <rdf:Description rdf:about="http://hxl.humanitarianresponse.info/ns/#affectedBy">
    <rdf:type rdf:resource="http://www.w3.org/1999/02/22-rdf-syntax-ns#Property"/>
  </rdf:Description>
  <rdf:Description rdf:about="http://hxl.humanitarianresponse.info/ns/#affectedBy">
    <rdf:type rdf:resource="http://www.w3.org/2002/07/owl#ObjectProperty"/>
  </rdf:Description>
  <rdf:Description rdf:about="http://hxl.humanitarianresponse.info/ns/#affectedBy">
    <rdfs:isDefinedBy rdf:resource="http://hxl.humanitarianresponse.info/ns/#humanitarianProfileSection"/>
  </rdf:Description>
  <rdf:Description rdf:about="http://hxl.humanitarianresponse.info/ns/#affectedBy">
    <skos:prefLabel xml:lang="en">affected by</skos:prefLabel>
  </rdf:Description>
  <rdf:Description rdf:about="http://hxl.humanitarianresponse.info/ns/#affectedBy">
    <rdfs:comment xml:lang="en">States that a Population is affacted by an Emergency.</rdfs:comment>
  </rdf:Description>
  <rdf:Description rdf:about="http://hxl.humanitarianresponse.info/ns/#affectedBy">
    <rdfs:domain rdf:resource="http://hxl.humanitarianresponse.info/ns/#AffectedPopulation"/>
  </rdf:Description>
  <rdf:Description rdf:about="http://hxl.humanitarianresponse.info/ns/#affectedBy">
    <rdfs:range rdf:resource="http://hxl.humanitarianresponse.info/ns/#Emergency"/>
  </rdf:Description>
  <rdf:Description rdf:about="http://hxl.humanitarianresponse.info/ns/#affects">
    <owl:inverseOf rdf:resource="http://hxl.humanitarianresponse.info/ns/#affectedBy"/>
  </rdf:Description>
  <rdf:Description rdf:about="http://hxl.humanitarianresponse.info/ns/#fromAge">
    <rdf:type rdf:resource="http://www.w3.org/1999/02/22-rdf-syntax-ns#Property"/>
  </rdf:Description>
  <rdf:Description rdf:about="http://hxl.humanitarianresponse.info/ns/#fromAge">
    <rdf:type rdf:resource="http://www.w3.org/2002/07/owl#DataProperty"/>
  </rdf:Description>
  <rdf:Description rdf:about="http://hxl.humanitarianresponse.info/ns/#fromAge">
    <rdfs:isDefinedBy rdf:resource="http://hxl.humanitarianresponse.info/ns/#humanitarianProfileSection"/>
  </rdf:Description>
  <rdf:Description rdf:about="http://hxl.humanitarianresponse.info/ns/#fromAge">
    <skos:prefLabel xml:lang="en">from age</skos:prefLabel>
  </rdf:Description>
  <rdf:Description rdf:about="http://hxl.humanitarianresponse.info/ns/#fromAge">
    <rdfs:comment>Specifies the bottom of an age range for an AgeGroup (in years).</rdfs:comment>
  </rdf:Description>
  <rdf:Description rdf:about="http://hxl.humanitarianresponse.info/ns/#fromAge">
    <rdfs:domain rdf:resource="http://hxl.humanitarianresponse.info/ns/#AgeGroup"/>
  </rdf:Description>
  <rdf:Description rdf:about="http://hxl.humanitarianresponse.info/ns/#fromAge">
    <rdfs:range rdf:resource="http://www.w3.org/2001/XMLSchema#int"/>
  </rdf:Description>
  <rdf:Description rdf:about="http://hxl.humanitarianresponse.info/ns/#toAge">
    <rdf:type rdf:resource="http://www.w3.org/1999/02/22-rdf-syntax-ns#Property"/>
  </rdf:Description>
  <rdf:Description rdf:about="http://hxl.humanitarianresponse.info/ns/#toAge">
    <rdf:type rdf:resource="http://www.w3.org/2002/07/owl#DataProperty"/>
  </rdf:Description>
  <rdf:Description rdf:about="http://hxl.humanitarianresponse.info/ns/#toAge">
    <rdfs:isDefinedBy rdf:resource="http://hxl.humanitarianresponse.info/ns/#humanitarianProfileSection"/>
  </rdf:Description>
  <rdf:Description rdf:about="http://hxl.humanitarianresponse.info/ns/#toAge">
    <skos:prefLabel xml:lang="en">to age</skos:prefLabel>
  </rdf:Description>
  <rdf:Description rdf:about="http://hxl.humanitarianresponse.info/ns/#toAge">
    <rdfs:comment>Specifies the top of an age range for an AgeGroup (in years).</rdfs:comment>
  </rdf:Description>
  <rdf:Description rdf:about="http://hxl.humanitarianresponse.info/ns/#toAge">
    <rdfs:domain rdf:resource="http://hxl.humanitarianresponse.info/ns/#AgeGroup"/>
  </rdf:Description>
  <rdf:Description rdf:about="http://hxl.humanitarianresponse.info/ns/#toAge">
    <rdfs:range rdf:resource="http://www.w3.org/2001/XMLSchema#int"/>
  </rdf:Description>
  <rdf:Description rdf:about="http://hxl.humanitarianresponse.info/ns/#atLocation">
    <rdf:type rdf:resource="http://www.w3.org/1999/02/22-rdf-syntax-ns#Property"/>
  </rdf:Description>
  <rdf:Description rdf:about="http://hxl.humanitarianresponse.info/ns/#atLocation">
    <rdf:type rdf:resource="http://www.w3.org/2002/07/owl#TransitiveProperty"/>
  </rdf:Description>
  <rdf:Description rdf:about="http://hxl.humanitarianresponse.info/ns/#atLocation">
    <rdfs:isDefinedBy rdf:resource="http://hxl.humanitarianresponse.info/ns/#geolocationSection"/>
  </rdf:Description>
  <rdf:Description rdf:about="http://hxl.humanitarianresponse.info/ns/#atLocation">
    <skos:prefLabel xml:lang="en">at Location</skos:prefLabel>
  </rdf:Description>
  <rdf:Description rdf:about="http://hxl.humanitarianresponse.info/ns/#atLocation">
    <rdfs:comment xml:lang="en">Specififes the location for things like emergencies, projects, or affected population locations. This should be an administrative unit or other feature established in the HXL data repositiry (generally an Administrative Unit, Populated Place, or Affected Population Location agreed by the IM Working Group in a given emergency). It is also used to define the hierarchy of administrative units with each lower level admin unit requiring a hxl:atLocation property specifying the next higher level admin unit to which it belongs.</rdfs:comment>
  </rdf:Description>
  <rdf:Description rdf:about="http://hxl.humanitarianresponse.info/ns/#atLocation">
    <rdfs:domain rdf:resource="http://hxl.humanitarianresponse.info/ns/#BaseClass"/>
  </rdf:Description>
  <rdf:Description rdf:about="http://hxl.humanitarianresponse.info/ns/#atLocation">
    <rdfs:range rdf:resource="http://www.opengis.net/geosparql#Feature"/>
  </rdf:Description>
  <rdf:Description rdf:about="http://hxl.humanitarianresponse.info/ns/#locationOf">
    <owl:inverseOf rdf:resource="http://hxl.humanitarianresponse.info/ns/#atLocation"/>
  </rdf:Description>
  <rdf:Description rdf:about="http://hxl.humanitarianresponse.info/ns/#atLevel">
    <rdf:type rdf:resource="http://www.w3.org/1999/02/22-rdf-syntax-ns#Property"/>
  </rdf:Description>
  <rdf:Description rdf:about="http://hxl.humanitarianresponse.info/ns/#atLevel">
    <rdf:type rdf:resource="http://www.w3.org/2002/07/owl#ObjectProperty"/>
  </rdf:Description>
  <rdf:Description rdf:about="http://hxl.humanitarianresponse.info/ns/#atLevel">
    <rdfs:isDefinedBy rdf:resource="http://hxl.humanitarianresponse.info/ns/#geolocationSection"/>
  </rdf:Description>
  <rdf:Description rdf:about="http://hxl.humanitarianresponse.info/ns/#atLevel">
    <skos:prefLabel xml:lang="en">at level</skos:prefLabel>
  </rdf:Description>
  <rdf:Description rdf:about="http://hxl.humanitarianresponse.info/ns/#atLevel">
    <rdfs:comment>Specifies the level for an administrative unit.</rdfs:comment>
  </rdf:Description>
  <rdf:Description rdf:about="http://hxl.humanitarianresponse.info/ns/#atLevel">
    <rdfs:domain rdf:resource="http://hxl.humanitarianresponse.info/ns/#AdminUnit"/>
  </rdf:Description>
  <rdf:Description rdf:about="http://hxl.humanitarianresponse.info/ns/#atLevel">
    <rdfs:range rdf:resource="http://hxl.humanitarianresponse.info/ns/#AdminUnitLevel"/>
  </rdf:Description>
  <rdf:Description rdf:about="http://hxl.humanitarianresponse.info/ns/#levelOf">
    <owl:inverseOf rdf:resource="http://hxl.humanitarianresponse.info/ns/#atLevel"/>
  </rdf:Description>
  <rdf:Description rdf:about="http://hxl.humanitarianresponse.info/ns/#adminUnitLevelNumber">
    <rdf:type rdf:resource="http://www.w3.org/1999/02/22-rdf-syntax-ns#Property"/>
  </rdf:Description>
  <rdf:Description rdf:about="http://hxl.humanitarianresponse.info/ns/#adminUnitLevelNumber">
    <rdf:type rdf:resource="http://www.w3.org/2002/07/owl#DataProperty"/>
  </rdf:Description>
  <rdf:Description rdf:about="http://hxl.humanitarianresponse.info/ns/#adminUnitLevelNumber">
    <rdfs:isDefinedBy rdf:resource="http://hxl.humanitarianresponse.info/ns/#geolocationSection"/>
  </rdf:Description>
  <rdf:Description rdf:about="http://hxl.humanitarianresponse.info/ns/#adminUnitLevelNumber">
    <skos:prefLabel xml:lang="en">administrative unit level number</skos:prefLabel>
  </rdf:Description>
  <rdf:Description rdf:about="http://hxl.humanitarianresponse.info/ns/#adminUnitLevelNumber">
    <rdfs:comment xml:lang="en">The number for this administrative unit level; e.g. 0 for country, 1 for state, etc.</rdfs:comment>
  </rdf:Description>
  <rdf:Description rdf:about="http://hxl.humanitarianresponse.info/ns/#adminUnitLevelNumber">
    <rdfs:domain rdf:resource="http://hxl.humanitarianresponse.info/ns/#AdminUnitLevel"/>
  </rdf:Description>
  <rdf:Description rdf:about="http://hxl.humanitarianresponse.info/ns/#adminUnitLevelNumber">
    <rdfs:range rdf:resource="http://www.w3.org/2001/XMLSchema#int"/>
  </rdf:Description>
  <rdf:Description rdf:about="http://hxl.humanitarianresponse.info/ns/#adminUnitLevelTitle">
    <rdf:type rdf:resource="http://www.w3.org/1999/02/22-rdf-syntax-ns#Property"/>
  </rdf:Description>
  <rdf:Description rdf:about="http://hxl.humanitarianresponse.info/ns/#adminUnitLevelTitle">
    <rdf:type rdf:resource="http://www.w3.org/2002/07/owl#DataProperty"/>
  </rdf:Description>
  <rdf:Description rdf:about="http://hxl.humanitarianresponse.info/ns/#adminUnitLevelTitle">
    <rdfs:isDefinedBy rdf:resource="http://hxl.humanitarianresponse.info/ns/#geolocationSection"/>
  </rdf:Description>
  <rdf:Description rdf:about="http://hxl.humanitarianresponse.info/ns/#adminUnitLevelTitle">
    <skos:prefLabel xml:lang="en">administrative unit level title</skos:prefLabel>
  </rdf:Description>
  <rdf:Description rdf:about="http://hxl.humanitarianresponse.info/ns/#adminUnitLevelTitle">
    <rdfs:comment xml:lang="en">The title for this administrative unit level; e.g. &lt;em&gt;state&lt;/em&gt; or &lt;em&gt;city district&lt;/em&gt;.</rdfs:comment>
  </rdf:Description>
  <rdf:Description rdf:about="http://hxl.humanitarianresponse.info/ns/#adminUnitLevelTitle">
    <rdfs:domain rdf:resource="http://hxl.humanitarianresponse.info/ns/#AdminUnitLevel"/>
  </rdf:Description>
  <rdf:Description rdf:about="http://hxl.humanitarianresponse.info/ns/#adminUnitLevelTitle">
    <rdfs:range rdf:resource="http://www.w3.org/2000/01/rdf-schema#Literal"/>
  </rdf:Description>
  <rdf:Description rdf:about="http://hxl.humanitarianresponse.info/ns/#adminUnitLevelCountry">
    <rdf:type rdf:resource="http://www.w3.org/1999/02/22-rdf-syntax-ns#Property"/>
  </rdf:Description>
  <rdf:Description rdf:about="http://hxl.humanitarianresponse.info/ns/#adminUnitLevelCountry">
    <rdf:type rdf:resource="http://www.w3.org/2002/07/owl#ObjectProperty"/>
  </rdf:Description>
  <rdf:Description rdf:about="http://hxl.humanitarianresponse.info/ns/#adminUnitLevelCountry">
    <rdfs:isDefinedBy rdf:resource="http://hxl.humanitarianresponse.info/ns/#geolocationSection"/>
  </rdf:Description>
  <rdf:Description rdf:about="http://hxl.humanitarianresponse.info/ns/#adminUnitLevelCountry">
    <skos:prefLabel xml:lang="en">administrative unit level country</skos:prefLabel>
  </rdf:Description>
  <rdf:Description rdf:about="http://hxl.humanitarianresponse.info/ns/#adminUnitLevelCountry">
    <rdfs:comment xml:lang="en">Relates an administrative unit level to the country (or countries) that it can be used in.</rdfs:comment>
  </rdf:Description>
  <rdf:Description rdf:about="http://hxl.humanitarianresponse.info/ns/#adminUnitLevelCountry">
    <rdfs:domain rdf:resource="http://hxl.humanitarianresponse.info/ns/#AdminUnitLevel"/>
  </rdf:Description>
  <rdf:Description rdf:about="http://hxl.humanitarianresponse.info/ns/#adminUnitLevelCountry">
    <rdfs:range rdf:resource="http://www.w3.org/2001/XMLSchema#date"/>
  </rdf:Description>
  <rdf:Description rdf:about="http://hxl.humanitarianresponse.info/ns/#adminUnitLevelCountryOf">
    <owl:inverseOf rdf:resource="http://hxl.humanitarianresponse.info/ns/#adminUnitLevel"/>
  </rdf:Description>
  <rdf:Description rdf:about="http://hxl.humanitarianresponse.info/ns/#date">
    <rdf:type rdf:resource="http://www.w3.org/1999/02/22-rdf-syntax-ns#Property"/>
  </rdf:Description>
  <rdf:Description rdf:about="http://hxl.humanitarianresponse.info/ns/#date">
    <rdf:type rdf:resource="http://www.w3.org/2002/07/owl#DataProperty"/>
  </rdf:Description>
  <rdf:Description rdf:about="http://hxl.humanitarianresponse.info/ns/#date">
    <rdfs:isDefinedBy rdf:resource="http://hxl.humanitarianresponse.info/ns/#metadataSection"/>
  </rdf:Description>
  <rdf:Description rdf:about="http://hxl.humanitarianresponse.info/ns/#date">
    <skos:prefLabel xml:lang="en">date</skos:prefLabel>
  </rdf:Description>
  <rdf:Description rdf:about="http://hxl.humanitarianresponse.info/ns/#date">
    <rdfs:subPropertyOf rdf:resource="http://purl.org/dc/terms/date"/>
  </rdf:Description>
  <rdf:Description rdf:about="http://hxl.humanitarianresponse.info/ns/#date">
    <rdfs:comment>Generic property for date/time stamps (e.g., reporting time stamps for data containers) at arbitrary granularity.</rdfs:comment>
  </rdf:Description>
  <rdf:Description rdf:about="http://hxl.humanitarianresponse.info/ns/#date">
    <rdfs:domain rdf:resource="http://hxl.humanitarianresponse.info/ns/#BaseClass"/>
  </rdf:Description>
  <rdf:Description rdf:about="http://hxl.humanitarianresponse.info/ns/#date">
    <rdfs:range rdf:resource="http://www.w3.org/2001/XMLSchema#date"/>
  </rdf:Description>
  <rdf:Description rdf:about="http://hxl.humanitarianresponse.info/ns/#validOn">
    <rdf:type rdf:resource="http://www.w3.org/1999/02/22-rdf-syntax-ns#Property"/>
  </rdf:Description>
  <rdf:Description rdf:about="http://hxl.humanitarianresponse.info/ns/#validOn">
    <rdf:type rdf:resource="http://www.w3.org/2002/07/owl#DataProperty"/>
  </rdf:Description>
  <rdf:Description rdf:about="http://hxl.humanitarianresponse.info/ns/#validOn">
    <rdfs:isDefinedBy rdf:resource="http://hxl.humanitarianresponse.info/ns/#metadataSection"/>
  </rdf:Description>
  <rdf:Description rdf:about="http://hxl.humanitarianresponse.info/ns/#validOn">
    <skos:prefLabel xml:lang="en">valid on</skos:prefLabel>
  </rdf:Description>
  <rdf:Description rdf:about="http://hxl.humanitarianresponse.info/ns/#validOn">
    <rdfs:subPropertyOf rdf:resource="http://hxl.humanitarianresponse.info/ns/#date"/>
  </rdf:Description>
  <rdf:Description rdf:about="http://hxl.humanitarianresponse.info/ns/#validOn">
    <rdfs:comment>Property to express when a certain piece of data, such as a person count, was valid. Note that this may differ from the time when the data was &lt;em&gt;reported&lt;/em&gt;; use &lt;a href='#date'&gt;hxl:date&lt;/a&gt; for these.</rdfs:comment>
  </rdf:Description>
  <rdf:Description rdf:about="http://hxl.humanitarianresponse.info/ns/#validOn">
    <rdfs:domain rdf:resource="http://hxl.humanitarianresponse.info/ns/#DataContainer"/>
  </rdf:Description>
  <rdf:Description rdf:about="http://hxl.humanitarianresponse.info/ns/#validOn">
    <rdfs:range rdf:resource="http://www.w3.org/2001/XMLSchema#date"/>
  </rdf:Description>
  <rdf:Description rdf:about="http://hxl.humanitarianresponse.info/ns/#hasGLIDEnumber">
    <rdf:type rdf:resource="http://www.w3.org/1999/02/22-rdf-syntax-ns#Property"/>
  </rdf:Description>
  <rdf:Description rdf:about="http://hxl.humanitarianresponse.info/ns/#hasGLIDEnumber">
    <rdf:type rdf:resource="http://www.w3.org/2002/07/owl#DataProperty"/>
  </rdf:Description>
  <rdf:Description rdf:about="http://hxl.humanitarianresponse.info/ns/#hasGLIDEnumber">
    <rdfs:isDefinedBy rdf:resource="http://hxl.humanitarianresponse.info/ns/#situationSection"/>
  </rdf:Description>
  <rdf:Description rdf:about="http://hxl.humanitarianresponse.info/ns/#hasGLIDEnumber">
    <skos:prefLabel xml:lang="en">has GLIDE number</skos:prefLabel>
  </rdf:Description>
  <rdf:Description rdf:about="http://hxl.humanitarianresponse.info/ns/#hasGLIDEnumber">
    <rdfs:comment xml:lang="en">Assigns the GLIDE number to an Emergency, i.e. a common unique ID code for disasters. See &lt;a href='http://glidenumber.net/glide/public/about.jsp'&gt;about GLIDE&lt;/a&gt;.</rdfs:comment>
  </rdf:Description>
  <rdf:Description rdf:about="http://hxl.humanitarianresponse.info/ns/#hasGLIDEnumber">
    <rdfs:domain rdf:resource="http://hxl.humanitarianresponse.info/ns/#Emergency"/>
  </rdf:Description>
  <rdf:Description rdf:about="http://hxl.humanitarianresponse.info/ns/#hasGLIDEnumber">
    <rdfs:range rdf:resource="http://www.w3.org/2001/XMLSchema#string"/>
  </rdf:Description>
  <rdf:Description rdf:about="http://hxl.humanitarianresponse.info/ns/#isGLIDEnumberOf">
    <owl:inverseOf rdf:resource="http://hxl.humanitarianresponse.info/ns/#hasGLIDEnumber"/>
  </rdf:Description>
  <rdf:Description rdf:about="http://hxl.humanitarianresponse.info/ns/#count">
    <rdf:type rdf:resource="http://www.w3.org/1999/02/22-rdf-syntax-ns#Property"/>
  </rdf:Description>
  <rdf:Description rdf:about="http://hxl.humanitarianresponse.info/ns/#count">
    <rdf:type rdf:resource="http://www.w3.org/2002/07/owl#DataProperty"/>
  </rdf:Description>
  <rdf:Description rdf:about="http://hxl.humanitarianresponse.info/ns/#count">
    <rdfs:isDefinedBy rdf:resource="http://hxl.humanitarianresponse.info/ns/#situationSection"/>
  </rdf:Description>
  <rdf:Description rdf:about="http://hxl.humanitarianresponse.info/ns/#count">
    <skos:prefLabel xml:lang="en">count</skos:prefLabel>
  </rdf:Description>
  <rdf:Description rdf:about="http://hxl.humanitarianresponse.info/ns/#count">
    <rdfs:comment xml:lang="en">Property to count people, things, etc. Subproperties should be used if possible to clarify what has been counted.</rdfs:comment>
  </rdf:Description>
  <rdf:Description rdf:about="http://hxl.humanitarianresponse.info/ns/#count">
    <rdfs:domain rdf:resource="http://hxl.humanitarianresponse.info/ns/#BaseClass"/>
  </rdf:Description>
  <rdf:Description rdf:about="http://hxl.humanitarianresponse.info/ns/#count">
    <rdfs:range rdf:resource="http://www.w3.org/2001/XMLSchema#int"/>
  </rdf:Description>
  <rdf:Description rdf:about="http://hxl.humanitarianresponse.info/ns/#personCount">
    <rdf:type rdf:resource="http://www.w3.org/1999/02/22-rdf-syntax-ns#Property"/>
  </rdf:Description>
  <rdf:Description rdf:about="http://hxl.humanitarianresponse.info/ns/#personCount">
    <rdf:type rdf:resource="http://www.w3.org/2002/07/owl#DataProperty"/>
  </rdf:Description>
  <rdf:Description rdf:about="http://hxl.humanitarianresponse.info/ns/#personCount">
    <rdfs:isDefinedBy rdf:resource="http://hxl.humanitarianresponse.info/ns/#humanitarianProfileSection"/>
  </rdf:Description>
  <rdf:Description rdf:about="http://hxl.humanitarianresponse.info/ns/#personCount">
    <skos:prefLabel xml:lang="en">person count</skos:prefLabel>
  </rdf:Description>
  <rdf:Description rdf:about="http://hxl.humanitarianresponse.info/ns/#personCount">
    <rdfs:subPropertyOf rdf:resource="http://hxl.humanitarianresponse.info/ns/#count"/>
  </rdf:Description>
  <rdf:Description rdf:about="http://hxl.humanitarianresponse.info/ns/#personCount">
    <rdfs:comment xml:lang="en">An estimate or count of the number of persons in a population. The range is intentionally not restricted to numeric values, so that rough numbers or estimates are supported.</rdfs:comment>
  </rdf:Description>
  <rdf:Description rdf:about="http://hxl.humanitarianresponse.info/ns/#personCount">
    <rdfs:domain rdf:resource="http://hxl.humanitarianresponse.info/ns/#Population"/>
  </rdf:Description>
  <rdf:Description rdf:about="http://hxl.humanitarianresponse.info/ns/#personCount">
    <rdfs:range rdf:resource="http://www.w3.org/2001/XMLSchema#int"/>
  </rdf:Description>
  <rdf:Description rdf:about="http://hxl.humanitarianresponse.info/ns/#householdCount">
    <rdf:type rdf:resource="http://www.w3.org/1999/02/22-rdf-syntax-ns#Property"/>
  </rdf:Description>
  <rdf:Description rdf:about="http://hxl.humanitarianresponse.info/ns/#householdCount">
    <rdf:type rdf:resource="http://www.w3.org/2002/07/owl#DataProperty"/>
  </rdf:Description>
  <rdf:Description rdf:about="http://hxl.humanitarianresponse.info/ns/#householdCount">
    <rdfs:isDefinedBy rdf:resource="http://hxl.humanitarianresponse.info/ns/#humanitarianProfileSection"/>
  </rdf:Description>
  <rdf:Description rdf:about="http://hxl.humanitarianresponse.info/ns/#householdCount">
    <skos:prefLabel xml:lang="en">household count</skos:prefLabel>
  </rdf:Description>
  <rdf:Description rdf:about="http://hxl.humanitarianresponse.info/ns/#householdCount">
    <rdfs:subPropertyOf rdf:resource="http://hxl.humanitarianresponse.info/ns/#count"/>
  </rdf:Description>
  <rdf:Description rdf:about="http://hxl.humanitarianresponse.info/ns/#householdCount">
    <rdfs:comment xml:lang="en">An estimate or count of the number of households in a population. The method by which the number was determined or estimated should also be reported using the hxl:method property.</rdfs:comment>
  </rdf:Description>
  <rdf:Description rdf:about="http://hxl.humanitarianresponse.info/ns/#householdCount">
    <rdfs:domain rdf:resource="http://hxl.humanitarianresponse.info/ns/#Population"/>
  </rdf:Description>
  <rdf:Description rdf:about="http://hxl.humanitarianresponse.info/ns/#householdCount">
    <rdfs:range rdf:resource="http://www.w3.org/2001/XMLSchema#int"/>
  </rdf:Description>
  <rdf:Description rdf:about="http://hxl.humanitarianresponse.info/ns/#source">
    <rdf:type rdf:resource="http://www.w3.org/1999/02/22-rdf-syntax-ns#Property"/>
  </rdf:Description>
  <rdf:Description rdf:about="http://hxl.humanitarianresponse.info/ns/#source">
    <rdf:type rdf:resource="http://www.w3.org/2002/07/owl#ObjectProperty"/>
  </rdf:Description>
  <rdf:Description rdf:about="http://hxl.humanitarianresponse.info/ns/#source">
    <rdfs:isDefinedBy rdf:resource="http://hxl.humanitarianresponse.info/ns/#humanitarianProfileSection"/>
  </rdf:Description>
  <rdf:Description rdf:about="http://hxl.humanitarianresponse.info/ns/#source">
    <skos:prefLabel xml:lang="en">source</skos:prefLabel>
  </rdf:Description>
  <rdf:Description rdf:about="http://hxl.humanitarianresponse.info/ns/#source">
    <rdfs:comment xml:lang="en">The organisation(s) providing the information. Note that in some cases, if the source is the same for all records, this item could be reported as metadata for the dataset rather than for each record.&lt;br /&gt;&lt;small&gt;Source: Humanitarian profile.&lt;/small&gt;</rdfs:comment>
  </rdf:Description>
  <rdf:Description rdf:about="http://hxl.humanitarianresponse.info/ns/#source">
    <rdfs:domain rdf:resource="http://hxl.humanitarianresponse.info/ns/#Population"/>
  </rdf:Description>
  <rdf:Description rdf:about="http://hxl.humanitarianresponse.info/ns/#source">
    <rdfs:range rdf:resource="http://hxl.humanitarianresponse.info/ns/#Source"/>
  </rdf:Description>
  <rdf:Description rdf:about="http://hxl.humanitarianresponse.info/ns/#sourceOf">
    <owl:inverseOf rdf:resource="http://hxl.humanitarianresponse.info/ns/#source"/>
  </rdf:Description>
  <rdf:Description rdf:about="http://hxl.humanitarianresponse.info/ns/#method">
    <rdf:type rdf:resource="http://www.w3.org/1999/02/22-rdf-syntax-ns#Property"/>
  </rdf:Description>
  <rdf:Description rdf:about="http://hxl.humanitarianresponse.info/ns/#method">
    <rdf:type rdf:resource="http://www.w3.org/2002/07/owl#DataProperty"/>
  </rdf:Description>
  <rdf:Description rdf:about="http://hxl.humanitarianresponse.info/ns/#method">
    <rdfs:isDefinedBy rdf:resource="http://hxl.humanitarianresponse.info/ns/#humanitarianProfileSection"/>
  </rdf:Description>
  <rdf:Description rdf:about="http://hxl.humanitarianresponse.info/ns/#method">
    <skos:prefLabel xml:lang="en">method</skos:prefLabel>
  </rdf:Description>
  <rdf:Description rdf:about="http://hxl.humanitarianresponse.info/ns/#method">
    <rdfs:comment xml:lang="en">The method by which the person count or household count was derived.&lt;br /&gt;&lt;small&gt;Source: Humanitarian profile.&lt;/small&gt;</rdfs:comment>
  </rdf:Description>
  <rdf:Description rdf:about="http://hxl.humanitarianresponse.info/ns/#method">
    <rdfs:domain rdf:resource="http://hxl.humanitarianresponse.info/ns/#Population"/>
  </rdf:Description>
  <rdf:Description rdf:about="http://hxl.humanitarianresponse.info/ns/#method">
    <rdfs:range rdf:resource="http://www.w3.org/2000/01/rdf-schema#Literal"/>
  </rdf:Description>
  <rdf:Description rdf:about="http://hxl.humanitarianresponse.info/ns/#commonTitle">
    <rdf:type rdf:resource="http://www.w3.org/1999/02/22-rdf-syntax-ns#Property"/>
  </rdf:Description>
  <rdf:Description rdf:about="http://hxl.humanitarianresponse.info/ns/#commonTitle">
    <rdf:type rdf:resource="http://www.w3.org/2002/07/owl#DataProperty"/>
  </rdf:Description>
  <rdf:Description rdf:about="http://hxl.humanitarianresponse.info/ns/#commonTitle">
    <rdfs:isDefinedBy rdf:resource="http://hxl.humanitarianresponse.info/ns/#situationSection"/>
  </rdf:Description>
  <rdf:Description rdf:about="http://hxl.humanitarianresponse.info/ns/#commonTitle">
    <skos:prefLabel xml:lang="en">common title</skos:prefLabel>
  </rdf:Description>
  <rdf:Description rdf:about="http://hxl.humanitarianresponse.info/ns/#commonTitle">
    <rdfs:comment xml:lang="en">A commonly use title/name for an emergency.</rdfs:comment>
  </rdf:Description>
  <rdf:Description rdf:about="http://hxl.humanitarianresponse.info/ns/#commonTitle">
    <rdfs:domain rdf:resource="http://hxl.humanitarianresponse.info/ns/#Situation"/>
  </rdf:Description>
  <rdf:Description rdf:about="http://hxl.humanitarianresponse.info/ns/#commonTitle">
    <rdfs:range rdf:resource="http://www.w3.org/2000/01/rdf-schema#Literal"/>
  </rdf:Description>
  <rdf:Description rdf:about="http://purl.org/dc/terms/PeriodOfTime">
    <rdf:type rdf:resource="http://www.w3.org/2000/01/rdf-schema#Class"/>
  </rdf:Description>
  <rdf:Description rdf:about="http://purl.org/dc/terms/PeriodOfTime">
    <rdf:type rdf:resource="http://www.w3.org/2002/07/owl#Class"/>
  </rdf:Description>
  <rdf:Description rdf:about="http://purl.org/dc/terms/PeriodOfTime">
    <rdfs:isDefinedBy rdf:resource="http://hxl.humanitarianresponse.info/ns/#metadataSection"/>
  </rdf:Description>
  <rdf:Description rdf:about="http://purl.org/dc/terms/PeriodOfTime">
    <skos:prefLabel>dc:PeriodOfTime</skos:prefLabel>
  </rdf:Description>
  <rdf:Description rdf:about="http://xmlns.com/foaf/0.1/Agent">
    <rdf:type rdf:resource="http://www.w3.org/2000/01/rdf-schema#Class"/>
  </rdf:Description>
  <rdf:Description rdf:about="http://xmlns.com/foaf/0.1/Agent">
    <rdf:type rdf:resource="http://www.w3.org/2002/07/owl#Class"/>
  </rdf:Description>
  <rdf:Description rdf:about="http://xmlns.com/foaf/0.1/Agent">
    <rdfs:isDefinedBy rdf:resource="http://hxl.humanitarianresponse.info/ns/#situationSection"/>
  </rdf:Description>
  <rdf:Description rdf:about="http://xmlns.com/foaf/0.1/Agent">
    <skos:prefLabel>foaf:Agent</skos:prefLabel>
  </rdf:Description>
  <rdf:Description rdf:about="http://xmlns.com/foaf/0.1/Organisation">
    <rdf:type rdf:resource="http://www.w3.org/2000/01/rdf-schema#Class"/>
  </rdf:Description>
  <rdf:Description rdf:about="http://xmlns.com/foaf/0.1/Organisation">
    <rdf:type rdf:resource="http://www.w3.org/2002/07/owl#Class"/>
  </rdf:Description>
  <rdf:Description rdf:about="http://xmlns.com/foaf/0.1/Organisation">
    <rdfs:isDefinedBy rdf:resource="http://hxl.humanitarianresponse.info/ns/#responseSection"/>
  </rdf:Description>
  <rdf:Description rdf:about="http://xmlns.com/foaf/0.1/Organisation">
    <skos:prefLabel>foaf:Organisation</skos:prefLabel>
  </rdf:Description>
  <rdf:Description rdf:about="http://xmlns.com/foaf/0.1/Organisation">
    <rdfs:subClassOf rdf:resource="http://xmlns.com/foaf/0.1/Agent"/>
  </rdf:Description>
  <rdf:Description rdf:about="http://xmlns.com/foaf/0.1/Group">
    <rdf:type rdf:resource="http://www.w3.org/2000/01/rdf-schema#Class"/>
  </rdf:Description>
  <rdf:Description rdf:about="http://xmlns.com/foaf/0.1/Group">
    <rdf:type rdf:resource="http://www.w3.org/2002/07/owl#Class"/>
  </rdf:Description>
  <rdf:Description rdf:about="http://xmlns.com/foaf/0.1/Group">
    <rdfs:isDefinedBy rdf:resource="http://hxl.humanitarianresponse.info/ns/#situationSection"/>
  </rdf:Description>
  <rdf:Description rdf:about="http://xmlns.com/foaf/0.1/Group">
    <skos:prefLabel>foaf:Group</skos:prefLabel>
  </rdf:Description>
  <rdf:Description rdf:about="http://xmlns.com/foaf/0.1/Group">
    <rdfs:subClassOf rdf:resource="http://xmlns.com/foaf/0.1/Agent"/>
  </rdf:Description>
  <rdf:Description rdf:about="http://hxl.humanitarianresponse.info/ns/#featureName">
    <rdf:type rdf:resource="http://www.w3.org/1999/02/22-rdf-syntax-ns#Property"/>
  </rdf:Description>
  <rdf:Description rdf:about="http://hxl.humanitarianresponse.info/ns/#featureName">
    <rdf:type rdf:resource="http://www.w3.org/2002/07/owl#DataProperty"/>
  </rdf:Description>
  <rdf:Description rdf:about="http://hxl.humanitarianresponse.info/ns/#featureName">
    <rdfs:isDefinedBy rdf:resource="http://hxl.humanitarianresponse.info/ns/#geolocationSection"/>
  </rdf:Description>
  <rdf:Description rdf:about="http://hxl.humanitarianresponse.info/ns/#featureName">
    <rdfs:subPropertyOf rdf:resource="http://hxl.humanitarianresponse.info/ns/#Title"/>
  </rdf:Description>
  <rdf:Description rdf:about="http://hxl.humanitarianresponse.info/ns/#featureName">
    <skos:prefLabel xml:lang="en">feature name</skos:prefLabel>
  </rdf:Description>
  <rdf:Description rdf:about="http://hxl.humanitarianresponse.info/ns/#featureName">
    <rdfs:comment xml:lang="en">The common name of the feature.  This is the accepted spelling of the name for the humanitarian community at the time of this version of the dataset.</rdfs:comment>
  </rdf:Description>
  <rdf:Description rdf:about="http://hxl.humanitarianresponse.info/ns/#featureName">
    <rdfs:domain rdf:resource="http://www.opengis.net/geosparql#Feature"/>
  </rdf:Description>
  <rdf:Description rdf:about="http://hxl.humanitarianresponse.info/ns/#featureName">
    <rdfs:range rdf:resource="http://www.w3.org/2000/01/rdf-schema#Literal"/>
  </rdf:Description>
  <rdf:Description rdf:about="http://hxl.humanitarianresponse.info/ns/#featureAltName">
    <rdf:type rdf:resource="http://www.w3.org/1999/02/22-rdf-syntax-ns#Property"/>
  </rdf:Description>
  <rdf:Description rdf:about="http://hxl.humanitarianresponse.info/ns/#featureAltName">
    <rdf:type rdf:resource="http://www.w3.org/2002/07/owl#DataProperty"/>
  </rdf:Description>
  <rdf:Description rdf:about="http://hxl.humanitarianresponse.info/ns/#featureAltName">
    <rdfs:isDefinedBy rdf:resource="http://hxl.humanitarianresponse.info/ns/#geolocationSection"/>
  </rdf:Description>
  <rdf:Description rdf:about="http://hxl.humanitarianresponse.info/ns/#featureAltName">
    <rdfs:subPropertyOf rdf:resource="http://hxl.humanitarianresponse.info/ns/#Title"/>
  </rdf:Description>
  <rdf:Description rdf:about="http://hxl.humanitarianresponse.info/ns/#featureAltName">
    <skos:prefLabel xml:lang="en">feature alternate name</skos:prefLabel>
  </rdf:Description>
  <rdf:Description rdf:about="http://hxl.humanitarianresponse.info/ns/#featureAltName">
    <rdfs:comment xml:lang="en">An alternative spelling of the feature.  This is not the accepted spelling of the name for the humanitarian community and should be avoided.</rdfs:comment>
  </rdf:Description>
  <rdf:Description rdf:about="http://hxl.humanitarianresponse.info/ns/#featureAltName">
    <rdfs:domain rdf:resource="http://www.opengis.net/geosparql#Feature"/>
  </rdf:Description>
  <rdf:Description rdf:about="http://hxl.humanitarianresponse.info/ns/#featureAltName">
    <rdfs:range rdf:resource="http://www.w3.org/2000/01/rdf-schema#Literal"/>
  </rdf:Description>
  <rdf:Description rdf:about="http://hxl.humanitarianresponse.info/ns/#featureRefName">
    <rdf:type rdf:resource="http://www.w3.org/1999/02/22-rdf-syntax-ns#Property"/>
  </rdf:Description>
  <rdf:Description rdf:about="http://hxl.humanitarianresponse.info/ns/#featureRefName">
    <rdf:type rdf:resource="http://www.w3.org/2002/07/owl#DataProperty"/>
  </rdf:Description>
  <rdf:Description rdf:about="http://hxl.humanitarianresponse.info/ns/#featureRefName">
    <rdfs:isDefinedBy rdf:resource="http://hxl.humanitarianresponse.info/ns/#geolocationSection"/>
  </rdf:Description>
  <rdf:Description rdf:about="http://hxl.humanitarianresponse.info/ns/#featureRefName">
    <rdfs:subPropertyOf rdf:resource="http://hxl.humanitarianresponse.info/ns/#Title"/>
  </rdf:Description>
  <rdf:Description rdf:about="http://hxl.humanitarianresponse.info/ns/#featureRefName">
    <skos:prefLabel xml:lang="en">feature reference name</skos:prefLabel>
  </rdf:Description>
  <rdf:Description rdf:about="http://hxl.humanitarianresponse.info/ns/#featureRefName">
    <rdfs:comment xml:lang="en">A version of the feature name in proper case without accented characters or apostrophes.  Spaces and hyphens are allowed.</rdfs:comment>
  </rdf:Description>
  <rdf:Description rdf:about="http://hxl.humanitarianresponse.info/ns/#featureRefName">
    <rdfs:domain rdf:resource="http://www.opengis.net/geosparql#Feature"/>
  </rdf:Description>
  <rdf:Description rdf:about="http://hxl.humanitarianresponse.info/ns/#featureRefName">
    <rdfs:range rdf:resource="http://www.w3.org/2000/01/rdf-schema#Literal"/>
  </rdf:Description>
  <rdf:Description rdf:about="http://hxl.humanitarianresponse.info/ns/#pcode">
    <rdf:type rdf:resource="http://www.w3.org/1999/02/22-rdf-syntax-ns#Property"/>
  </rdf:Description>
  <rdf:Description rdf:about="http://hxl.humanitarianresponse.info/ns/#pcode">
    <rdf:type rdf:resource="http://www.w3.org/2002/07/owl#DataProperty"/>
  </rdf:Description>
  <rdf:Description rdf:about="http://hxl.humanitarianresponse.info/ns/#pcode">
    <rdfs:isDefinedBy rdf:resource="http://hxl.humanitarianresponse.info/ns/#geolocationSection"/>
  </rdf:Description>
  <rdf:Description rdf:about="http://hxl.humanitarianresponse.info/ns/#pcode">
    <skos:prefLabel xml:lang="en">p-code</skos:prefLabel>
  </rdf:Description>
  <rdf:Description rdf:about="http://hxl.humanitarianresponse.info/ns/#pcode">
    <rdfs:comment xml:lang="en">Specifies the unique identifier for an administrative unit or populated place.  This is the preferred way of referencing these geographic features.</rdfs:comment>
  </rdf:Description>
  <rdf:Description rdf:about="http://hxl.humanitarianresponse.info/ns/#pcode">
    <rdfs:domain rdf:resource="http://www.opengis.net/geosparql#Feature"/>
  </rdf:Description>
  <rdf:Description rdf:about="http://hxl.humanitarianresponse.info/ns/#pcode">
    <rdfs:range rdf:resource="http://www.w3.org/2000/01/rdf-schema#Literal"/>
  </rdf:Description>
  <rdf:Description rdf:about="http://hxl.humanitarianresponse.info/ns/#sexCategory">
    <rdf:type rdf:resource="http://www.w3.org/1999/02/22-rdf-syntax-ns#Property"/>
  </rdf:Description>
  <rdf:Description rdf:about="http://hxl.humanitarianresponse.info/ns/#sexCategory">
    <rdf:type rdf:resource="http://www.w3.org/2002/07/owl#ObjectProperty"/>
  </rdf:Description>
  <rdf:Description rdf:about="http://hxl.humanitarianresponse.info/ns/#sexCategory">
    <rdfs:isDefinedBy rdf:resource="http://hxl.humanitarianresponse.info/ns/#humanitarianProfileSection"/>
  </rdf:Description>
  <rdf:Description rdf:about="http://hxl.humanitarianresponse.info/ns/#sexCategory">
    <skos:prefLabel>sex category</skos:prefLabel>
  </rdf:Description>
  <rdf:Description rdf:about="http://hxl.humanitarianresponse.info/ns/#sexCategory">
    <rdfs:comment>Specifies the sex of the population.</rdfs:comment>
  </rdf:Description>
  <rdf:Description rdf:about="http://hxl.humanitarianresponse.info/ns/#sexCategory">
    <rdfs:domain rdf:resource="http://hxl.humanitarianresponse.info/ns/#Population"/>
  </rdf:Description>
  <rdf:Description rdf:about="http://hxl.humanitarianresponse.info/ns/#sexCategory">
    <rdfs:range rdf:resource="http://hxl.humanitarianresponse.info/ns/#SexCategory"/>
  </rdf:Description>
  <rdf:Description rdf:about="http://hxl.humanitarianresponse.info/ns/#sexCategoryOf">
    <owl:inverseOf rdf:resource="http://hxl.humanitarianresponse.info/ns/#sexCategory"/>
  </rdf:Description>
  <rdf:Description rdf:about="http://hxl.humanitarianresponse.info/ns/#ageGroup">
    <rdf:type rdf:resource="http://www.w3.org/1999/02/22-rdf-syntax-ns#Property"/>
  </rdf:Description>
  <rdf:Description rdf:about="http://hxl.humanitarianresponse.info/ns/#ageGroup">
    <rdf:type rdf:resource="http://www.w3.org/2002/07/owl#ObjectProperty"/>
  </rdf:Description>
  <rdf:Description rdf:about="http://hxl.humanitarianresponse.info/ns/#ageGroup">
    <rdfs:isDefinedBy rdf:resource="http://hxl.humanitarianresponse.info/ns/#humanitarianProfileSection"/>
  </rdf:Description>
  <rdf:Description rdf:about="http://hxl.humanitarianresponse.info/ns/#ageGroup">
    <skos:prefLabel>age group</skos:prefLabel>
  </rdf:Description>
  <rdf:Description rdf:about="http://hxl.humanitarianresponse.info/ns/#ageGroup">
    <rdfs:comment>Specifies the age group of the population.</rdfs:comment>
  </rdf:Description>
  <rdf:Description rdf:about="http://hxl.humanitarianresponse.info/ns/#ageGroup">
    <rdfs:domain rdf:resource="http://hxl.humanitarianresponse.info/ns/#Population"/>
  </rdf:Description>
  <rdf:Description rdf:about="http://hxl.humanitarianresponse.info/ns/#ageGroup">
    <rdfs:range rdf:resource="http://hxl.humanitarianresponse.info/ns/#AgeGroup"/>
  </rdf:Description>
  <rdf:Description rdf:about="http://hxl.humanitarianresponse.info/ns/#ageGroupOf">
    <owl:inverseOf rdf:resource="http://hxl.humanitarianresponse.info/ns/#ageGroup"/>
  </rdf:Description>
  <rdf:Description rdf:about="http://hxl.humanitarianresponse.info/ns/#AgeGroup">
    <rdf:type rdf:resource="http://www.w3.org/2000/01/rdf-schema#Class"/>
  </rdf:Description>
  <rdf:Description rdf:about="http://hxl.humanitarianresponse.info/ns/#AgeGroup">
    <rdfs:subClassOf rdf:resource="http://hxl.humanitarianresponse.info/ns/#BaseClass"/>
  </rdf:Description>
  <rdf:Description rdf:about="http://hxl.humanitarianresponse.info/ns/#AgeGroup">
    <rdfs:isDefinedBy rdf:resource="http://hxl.humanitarianresponse.info/ns/#humanitarianProfileSection"/>
  </rdf:Description>
  <rdf:Description rdf:about="http://hxl.humanitarianresponse.info/ns/#AgeGroup">
    <skos:prefLabel xml:lang="en">Age Group</skos:prefLabel>
  </rdf:Description>
  <rdf:Description rdf:about="http://hxl.humanitarianresponse.info/ns/#AgeGroup">
    <label:plural xml:lang="en">Age Groups</label:plural>
  </rdf:Description>
  <rdf:Description rdf:about="http://hxl.humanitarianresponse.info/ns/#AgeGroup">
    <rdfs:comment>Generic class for age groups; instances should be created for actual age groups and must have an identifier that does not start with a number. Example: &lt;em&gt;Children under 5&lt;/em&gt;. Each AgeGroup should be added to at least one &lt;a href='#AgeGroupSet'&gt;AgeGroupSet&lt;/a&gt; following the conventions of &lt;a href='http://www.w3.org/TR/rdf-schema/#ch_member'&gt;rdfs:member&lt;/a&gt;.</rdfs:comment>
  </rdf:Description>
  <rdf:Description rdf:about="http://hxl.humanitarianresponse.info/ns/#AgeGroupSet">
    <rdf:type rdf:resource="http://www.w3.org/2000/01/rdf-schema#Class"/>
  </rdf:Description>
  <rdf:Description rdf:about="http://hxl.humanitarianresponse.info/ns/#AgeGroupSet">
    <rdfs:subClassOf rdf:resource="http://hxl.humanitarianresponse.info/ns/#BaseClass"/>
  </rdf:Description>
  <rdf:Description rdf:about="http://hxl.humanitarianresponse.info/ns/#AgeGroupSet">
    <rdfs:subClassOf rdf:resource="http://www.w3.org/1999/02/22-rdf-syntax-ns#Bag"/>
  </rdf:Description>
  <rdf:Description rdf:about="http://hxl.humanitarianresponse.info/ns/#AgeGroupSet">
    <rdfs:isDefinedBy rdf:resource="http://hxl.humanitarianresponse.info/ns/#humanitarianProfileSection"/>
  </rdf:Description>
  <rdf:Description rdf:about="http://hxl.humanitarianresponse.info/ns/#AgeGroupSet">
    <skos:prefLabel xml:lang="en">Age Group Set</skos:prefLabel>
  </rdf:Description>
  <rdf:Description rdf:about="http://hxl.humanitarianresponse.info/ns/#AgeGroupSet">
    <label:plural xml:lang="en">Age Group Sets</label:plural>
  </rdf:Description>
  <rdf:Description rdf:about="http://hxl.humanitarianresponse.info/ns/#AgeGroupSet">
    <rdfs:comment xml:lang="en">Contains a set of bracketed age groups, usually defined as a standard by some authority. &lt;a href='#AgeGroup'&gt;AgeGroups&lt;/a&gt; should be added to an AgeGroupSet following the conventions of &lt;a href='http://www.w3.org/TR/rdf-schema/#ch_member'&gt;rdfs:member&lt;/a&gt;.</rdfs:comment>
  </rdf:Description>
  <rdf:Description rdf:about="http://hxl.humanitarianresponse.info/ns/#displacedLocationType">
    <rdf:type rdf:resource="http://www.w3.org/1999/02/22-rdf-syntax-ns#Property"/>
  </rdf:Description>
  <rdf:Description rdf:about="http://hxl.humanitarianresponse.info/ns/#displacedLocationType">
    <rdf:type rdf:resource="http://www.w3.org/2002/07/owl#ObjectProperty"/>
  </rdf:Description>
  <rdf:Description rdf:about="http://hxl.humanitarianresponse.info/ns/#displacedLocationType">
    <rdfs:isDefinedBy rdf:resource="http://hxl.humanitarianresponse.info/ns/#geolocationSection"/>
  </rdf:Description>
  <rdf:Description rdf:about="http://hxl.humanitarianresponse.info/ns/#displacedLocationType">
    <skos:prefLabel xml:lang="en">displaced location type</skos:prefLabel>
  </rdf:Description>
  <rdf:Description rdf:about="http://hxl.humanitarianresponse.info/ns/#displacedLocationType">
    <rdfs:comment xml:lang="en">Specifies the type of living situation in which a population is living.</rdfs:comment>
  </rdf:Description>
  <rdf:Description rdf:about="http://hxl.humanitarianresponse.info/ns/#displacedLocationType">
    <rdfs:domain rdf:resource="http://hxl.humanitarianresponse.info/ns/#APL"/>
  </rdf:Description>
  <rdf:Description rdf:about="http://hxl.humanitarianresponse.info/ns/#displacedLocationType">
    <rdfs:range rdf:resource="http://hxl.humanitarianresponse.info/ns/#DisplacedLocationType"/>
  </rdf:Description>
  <rdf:Description rdf:about="http://hxl.humanitarianresponse.info/ns/#displacedLocationTypeOf">
    <owl:inverseOf rdf:resource="http://hxl.humanitarianresponse.info/ns/#displacedLocationType"/>
  </rdf:Description>
  <rdf:Description rdf:about="http://hxl.humanitarianresponse.info/ns/#DisplacedLocationType">
    <rdf:type rdf:resource="http://www.w3.org/2000/01/rdf-schema#Class"/>
  </rdf:Description>
  <rdf:Description rdf:about="http://hxl.humanitarianresponse.info/ns/#DisplacedLocationType">
    <rdfs:subClassOf rdf:resource="http://hxl.humanitarianresponse.info/ns/#BaseClass"/>
  </rdf:Description>
  <rdf:Description rdf:about="http://hxl.humanitarianresponse.info/ns/#DisplacedLocationType">
    <rdfs:isDefinedBy rdf:resource="http://hxl.humanitarianresponse.info/ns/#geolocationSection"/>
  </rdf:Description>
  <rdf:Description rdf:about="http://hxl.humanitarianresponse.info/ns/#DisplacedLocationType">
    <skos:prefLabel xml:lang="en">Displaced Location Type</skos:prefLabel>
  </rdf:Description>
  <rdf:Description rdf:about="http://hxl.humanitarianresponse.info/ns/#DisplacedLocationType">
    <label:plural xml:lang="en">Displaced Location Types</label:plural>
  </rdf:Description>
  <rdf:Description rdf:about="http://hxl.humanitarianresponse.info/ns/#DisplacedLocationType">
    <rdfs:comment xml:lang="en">Generic class for types of displaced locations; instances should be created for actual displaced location types and must have identifiers that do not start with a number. Examples: &lt;em&gt;self-settled camp&lt;/em&gt; or &lt;em&gt;collective centre&lt;/em&gt;. Each DisplacedLocationType should be added to at least one &lt;a href='#DisplacedLocationTypeSet'&gt;DisplacedLocationTypeSet&lt;/a&gt; following the conventions of &lt;a href='http://www.w3.org/TR/rdf-schema/#ch_member'&gt;rdfs:member&lt;/a&gt;.</rdfs:comment>
  </rdf:Description>
  <rdf:Description rdf:about="http://hxl.humanitarianresponse.info/ns/#DisplacedLocationTypeSet">
    <rdf:type rdf:resource="http://www.w3.org/2000/01/rdf-schema#Class"/>
  </rdf:Description>
  <rdf:Description rdf:about="http://hxl.humanitarianresponse.info/ns/#DisplacedLocationTypeSet">
    <rdfs:subClassOf rdf:resource="http://hxl.humanitarianresponse.info/ns/#BaseClass"/>
  </rdf:Description>
  <rdf:Description rdf:about="http://hxl.humanitarianresponse.info/ns/#DisplacedLocationTypeSet">
    <rdfs:subClassOf rdf:resource="http://www.w3.org/1999/02/22-rdf-syntax-ns#Bag"/>
  </rdf:Description>
  <rdf:Description rdf:about="http://hxl.humanitarianresponse.info/ns/#DisplacedLocationTypeSet">
    <rdfs:isDefinedBy rdf:resource="http://hxl.humanitarianresponse.info/ns/#geolocationSection"/>
  </rdf:Description>
  <rdf:Description rdf:about="http://hxl.humanitarianresponse.info/ns/#DisplacedLocationTypeSet">
    <skos:prefLabel xml:lang="en">Displaced Persons Location Type Set</skos:prefLabel>
  </rdf:Description>
  <rdf:Description rdf:about="http://hxl.humanitarianresponse.info/ns/#DisplacedLocationTypeSet">
    <rdfs:comment xml:lang="en">Generic class for classes describing the housing situation in which a displaced population is living. Subclasses of this class represent a coherent set of these location types which may vary from emergency to emergency.  The individual types are instances of the subclass. &lt;a href='#DisplacedLocationType'&gt;DisplacedLocationTypes&lt;/a&gt; should be added to a DisplacedLocationTypeSet following the conventions of &lt;a href='http://www.w3.org/TR/rdf-schema/#ch_member'&gt;rdfs:member&lt;/a&gt;.</rdfs:comment>
  </rdf:Description>
  <rdf:Description rdf:about="http://hxl.humanitarianresponse.info/ns/#ReportCategorySet">
    <rdf:type rdf:resource="http://www.w3.org/2000/01/rdf-schema#Class"/>
  </rdf:Description>
  <rdf:Description rdf:about="http://hxl.humanitarianresponse.info/ns/#ReportCategorySet">
    <rdfs:subClassOf rdf:resource="http://hxl.humanitarianresponse.info/ns/#BaseClass"/>
  </rdf:Description>
  <rdf:Description rdf:about="http://hxl.humanitarianresponse.info/ns/#ReportCategorySet">
    <rdfs:subClassOf rdf:resource="http://www.w3.org/1999/02/22-rdf-syntax-ns#Bag"/>
  </rdf:Description>
  <rdf:Description rdf:about="http://hxl.humanitarianresponse.info/ns/#ReportCategorySet">
    <rdfs:isDefinedBy rdf:resource="http://hxl.humanitarianresponse.info/ns/#metadataSection"/>
  </rdf:Description>
  <rdf:Description rdf:about="http://hxl.humanitarianresponse.info/ns/#ReportCategorySet">
    <skos:prefLabel xml:lang="en">Report Category Set</skos:prefLabel>
  </rdf:Description>
  <rdf:Description rdf:about="http://hxl.humanitarianresponse.info/ns/#ReportCategorySet">
    <rdfs:comment xml:lang="en">A set of report categories that may be specific to an emergency. &lt;a href='#ReportCategory'&gt;ReportCategories&lt;/a&gt; should be added to a ReportCategorySet following the conventions of &lt;a href='http://www.w3.org/TR/rdf-schema/#ch_member'&gt;rdfs:member&lt;/a&gt;</rdfs:comment>
  </rdf:Description>
  <rdf:Description rdf:about="http://hxl.humanitarianresponse.info/ns/#ReportCategory">
    <rdf:type rdf:resource="http://www.w3.org/2000/01/rdf-schema#Class"/>
  </rdf:Description>
  <rdf:Description rdf:about="http://hxl.humanitarianresponse.info/ns/#ReportCategory">
    <rdfs:subClassOf rdf:resource="http://hxl.humanitarianresponse.info/ns/#BaseClass"/>
  </rdf:Description>
  <rdf:Description rdf:about="http://hxl.humanitarianresponse.info/ns/#ReportCategory">
    <rdfs:isDefinedBy rdf:resource="http://hxl.humanitarianresponse.info/ns/#metadataSection"/>
  </rdf:Description>
  <rdf:Description rdf:about="http://hxl.humanitarianresponse.info/ns/#ReportCategory">
    <skos:prefLabel xml:lang="en">Report Category</skos:prefLabel>
  </rdf:Description>
  <rdf:Description rdf:about="http://hxl.humanitarianresponse.info/ns/#ReportCategory">
    <rdfs:comment xml:lang="en">Instances of this class are specific report categories such as &lt;em&gt;humanitrian profile&lt;/em&gt;, &lt;em&gt;shelter&lt;/em&gt; or &lt;em&gt;security&lt;/em&gt;. Each ReportCategory should be added to at least one &lt;a href='#ReportCategorySet'&gt;ReportCategorySet&lt;/a&gt; following the conventions of &lt;a href='http://www.w3.org/TR/rdf-schema/#ch_member'&gt;rdfs:member&lt;/a&gt;.</rdfs:comment>
  </rdf:Description>
  <rdf:Description rdf:about="http://hxl.humanitarianresponse.info/ns/#reportCategory">
    <rdf:type rdf:resource="http://www.w3.org/1999/02/22-rdf-syntax-ns#Property"/>
  </rdf:Description>
  <rdf:Description rdf:about="http://hxl.humanitarianresponse.info/ns/#reportCategory">
    <rdf:type rdf:resource="http://www.w3.org/2002/07/owl#ObjectProperty"/>
  </rdf:Description>
  <rdf:Description rdf:about="http://hxl.humanitarianresponse.info/ns/#reportCategory">
    <rdfs:isDefinedBy rdf:resource="http://hxl.humanitarianresponse.info/ns/#metadataSection"/>
  </rdf:Description>
  <rdf:Description rdf:about="http://hxl.humanitarianresponse.info/ns/#reportCategory">
    <skos:prefLabel>report category</skos:prefLabel>
  </rdf:Description>
  <rdf:Description rdf:about="http://hxl.humanitarianresponse.info/ns/#reportCategory">
    <rdfs:comment>Specifies the ReportCategory of a DataContainer.</rdfs:comment>
  </rdf:Description>
  <rdf:Description rdf:about="http://hxl.humanitarianresponse.info/ns/#reportCategory">
    <rdfs:domain rdf:resource="http://hxl.humanitarianresponse.info/ns/#DataContainer"/>
  </rdf:Description>
  <rdf:Description rdf:about="http://hxl.humanitarianresponse.info/ns/#reportCategory">
    <rdfs:range rdf:resource="http://hxl.humanitarianresponse.info/ns/#ReportCategory"/>
  </rdf:Description>
  <rdf:Description rdf:about="http://hxl.humanitarianresponse.info/ns/#reportCategoryOf">
    <owl:inverseOf rdf:resource="http://hxl.humanitarianresponse.info/ns/#reportCategory"/>
  </rdf:Description>
</rdf:RDF>
